@prefix          rdf: <http://www.w3.org/1999/02/22-rdf-syntax-ns#> .
@prefix         rdfs: <http://www.w3.org/2000/01/rdf-schema#> .
@prefix          xsd: <http://www.w3.org/2001/XMLSchema#> .
@prefix          owl: <http://www.w3.org/2002/07/owl#> .
@prefix             : <http://iec.ch/TC57/CIM-generic#> .
@prefix          cim: <https://cim.ucaiug.io/ns#> .
@prefix           md: <http://iec.ch/TC57/61970-552/ModelDescription/1#> .
@prefix        model: <http://iec.ch/TC57/61970-552/ModelDescription/1#> .
@prefix         next: <http://der.edf.fr/mire/MSite-v3.1.a#> .
@prefix        next2: <http://edf.fr/draft/cim17-ext#> .
@prefix        next3: <http://edf.fr/draft/cim17-info#> .
@prefix          uml: <http://iec.ch/TC57/NonStandard/UML#> .

<http://iec.ch/TC57/CIM-generic> a owl:Ontology .

:ModelingAuthority a owl:Class ;
  rdfs:label "ModelingAuthority" ;
  rdfs:comment "A Modeling Authority is an entity responsible for supplying and maintaining the data defining a specific set of objects in a network model."@en ;
  rdfs:isDefinedBy :Package_ModelAuthority ;
  uml:id "EAID_C2D644C3_20C1_408d_86F0_738AD512C121" .

:ModelingAuthoritySet a owl:Class ;
  rdfs:label "ModelingAuthoritySet" ;
  rdfs:comment """A Modeling Authority Set is a group of objects in a network model where the data is supplied and maintained by the same Modeling Authority.
      This class is typically not included in instance data exchange as this information is tracked by other mechanisms in the exchange."""@en ;
  rdfs:isDefinedBy :Package_ModelAuthority ;
  uml:id "EAID_6D6E62ED_DCB6_4e54_9159_8469729C9828" .

:PowerSystemProjectSchedule a owl:Class ;
  rdfs:label "PowerSystemProjectSchedule" ;
  rdfs:isDefinedBy :Package_PowerSystemProject ;
  uml:id "EAID_7DC6B4C8_C974_401f_939A_39C1DD101122" .

:PowerSystemSubProject a owl:Class ;
  rdfs:label "PowerSystemSubProject" ;
  rdfs:comment "A collection of dependent projects."@en ;
  rdfs:isDefinedBy :Package_PowerSystemProject ;
  uml:id "EAID_42771878_2F05_4bc6_BC00_E9068AA3EDD3" .

:ProjectStep a owl:Class ;
  rdfs:label "ProjectStep" ;
  rdfs:comment "The ProjectSteps are ordered by the actualStart and actualEnds so that  a dependent ProjectStep will have a actualStart after an actualEnd."@en ;
  rdfs:isDefinedBy :Package_PowerSystemProject ;
  uml:id "EAID_7CD8163C_EE75_49cd_9305_8882E4110723" .

:ProjectStepStatusKind a owl:Class ;
  rdfs:label "ProjectStepStatusKind" ;
  rdfs:isDefinedBy :Package_PowerSystemProject ;
  uml:hasStereotype uml:enum, uml:enumeration ;
  uml:id "EAID_9A16A0EF_917D_4824_BA55_8833EB4D8E0E" .

:StepKind a owl:Class ;
  rdfs:label "StepKind" ;
  rdfs:comment "First phase investigation and planning."@en, "Project is approved for realisation and the construction is starting, under construction or in the state of being realist."@en, "State of the project"@en, "The project is commissioned and added to the network model."@en ;
  rdfs:isDefinedBy :Package_PowerSystemProject ;
  uml:hasStereotype uml:enum, uml:enumeration ;
  uml:id "EAID_E73576D6_ABD2_4dde_B7AB_71996C8B33A2" .

cim:AssetInfo a owl:Class ;
  rdfs:label "AssetInfo" ;
  rdfs:comment """Set of attributes of an asset, representing typical data-sheet information of a physical device, that can be instantiated and shared in different data exchange contexts:
      - as attributes of an asset instance (installed or in stock)
      - as attributes of an asset model (product by a manufacturer)
      - as attributes of a type asset (generic type of an asset as used in designs/extension planning)."""@en ;
  rdfs:isDefinedBy :Package_Standard ;
  rdfs:subClassOf cim:IdentifiedObject ;
  uml:id "EAID_30FBF45B_74C6_4e74_B7D5_772D51971E33" .

cim:AssetModelUsageKind a owl:Class ;
  rdfs:label "AssetModelUsageKind" ;
  rdfs:comment "Usage for an asset model."@en ;
  rdfs:isDefinedBy :Package_CIMEnumerations ;
  uml:hasStereotype uml:enumeration ;
  uml:id "EAID_95C22779_AD14_4e7b_875E_E85E8EACEC42" .

cim:AsynchronousMachineKind a owl:Class ;
  rdfs:label "AsynchronousMachineKind" ;
  rdfs:comment "Kind of Asynchronous Machine."@en ;
  rdfs:isDefinedBy :Package_CIMEnumerations ;
  uml:hasStereotype uml:enumeration ;
  uml:id "EAID_C2395579_2094_4bc6_B96D_56E185200EB1" .

cim:BusbarSectionInfo a owl:Class ;
  rdfs:label "BusbarSectionInfo" ;
  rdfs:comment "Busbar section data."@en ;
  rdfs:isDefinedBy :Package_Standard ;
  rdfs:subClassOf cim:AssetInfo ;
  uml:id "EAID_D910C856_BDEE_45c7_BF2E_96B9561F2570" .

cim:CDPSMVersion a owl:Class ;
  rdfs:label "CDPSMVersion" ;
  rdfs:comment "CDPSM profiles set version details."@en ;
  rdfs:isDefinedBy :Package_Extensions ;
  uml:hasStereotype uml:cdpsm ;
  uml:id "EAID_0D2BEBD3_B3EF_46c6_B7C8_533F3340D673" .

cim:CableConstructionKind a owl:Class ;
  rdfs:label "CableConstructionKind" ;
  rdfs:comment "Kind of cable construction."@en ;
  rdfs:isDefinedBy :Package_CIMEnumerations ;
  uml:hasStereotype uml:enumeration ;
  uml:id "EAID_A57A40AC_EA8E_400f_BA03_164E85900253" .

cim:CableInfo a owl:Class ;
  rdfs:label "CableInfo" ;
  rdfs:comment "Cable data."@en ;
  rdfs:isDefinedBy :Package_Standard ;
  rdfs:subClassOf cim:WireInfo ;
  uml:id "EAID_2B65C7CD_A660_4dbc_A5F5_29F437FE1D7A" .

cim:CableOuterJacketKind a owl:Class ;
  rdfs:label "CableOuterJacketKind" ;
  rdfs:comment "Kind of cable outer jacket."@en ;
  rdfs:isDefinedBy :Package_CIMEnumerations ;
  uml:hasStereotype uml:enumeration ;
  uml:id "EAID_A507A747_6AAE_4791_A8EB_C551C6F5C249" .

cim:CableShieldMaterialKind a owl:Class ;
  rdfs:label "CableShieldMaterialKind" ;
  rdfs:comment "Kind of cable shield material."@en ;
  rdfs:isDefinedBy :Package_CIMEnumerations ;
  uml:hasStereotype uml:enumeration ;
  uml:id "EAID_8D834724_2F83_44b1_9CF6_81476C3CC028" .

cim:CatalogAssetType a owl:Class ;
  rdfs:label "CatalogAssetType" ;
  rdfs:comment "assets that may be used for planning, work or design purposes."@en ;
  rdfs:isDefinedBy :Package_Standard ;
  rdfs:subClassOf cim:IdentifiedObject ;
  uml:id "EAID_3F51F3FA_94E9_4caa_A77D_53EA9C5F69C9" .

cim:CurveStyle a owl:Class ;
  rdfs:label "CurveStyle" ;
  rdfs:comment "Style or shape of curve."@en ;
  rdfs:isDefinedBy :Package_CIMEnumerations ;
  uml:hasStereotype uml:enumeration ;
  uml:id "EAID_581AD431_AA05_4773_9693_5BD5767AA1F2" .

cim:DateTimeInterval a owl:Class ;
  rdfs:label "DateTimeInterval" ;
  rdfs:comment "Interval between two date and time points."@en ;
  rdfs:isDefinedBy :Package_CompoundTypes ;
  uml:hasStereotype uml:compound ;
  uml:id "EAID_6941208A_3F6F_434f_A7D1_DD3484409331" .

cim:EndDeviceInfo a owl:Class ;
  rdfs:label "EndDeviceInfo" ;
  rdfs:comment "End device data."@en ;
  rdfs:isDefinedBy :Package_Standard ;
  rdfs:subClassOf cim:AssetInfo ;
  uml:id "EAID_E86CD1A7_D7C9_40ec_8CEE_2A12482F441A" .

cim:GeneratorControlSource a owl:Class ;
  rdfs:label "GeneratorControlSource" ;
  rdfs:comment "The source of controls for a generating unit."@en ;
  rdfs:isDefinedBy :Package_CIMEnumerations ;
  uml:hasStereotype uml:enumeration ;
  uml:id "EAID_30E66CA1_5BEA_4df6_B147_E3BA6C8CCAB7" .

cim:HydroPlantStorageKind a owl:Class ;
  rdfs:label "HydroPlantStorageKind" ;
  rdfs:comment "The type of hydro power plant."@en ;
  rdfs:isDefinedBy :Package_CIMEnumerations ;
  uml:hasStereotype uml:enumeration ;
  uml:id "EAID_A93B398E_56F0_466c_B0DE_0F907EBB3614" .

cim:IEC61968CIMVersion a owl:Class ;
  rdfs:label "IEC61968CIMVersion" ;
  rdfs:comment "IEC 61968 version number assigned to this UML model."@en ;
  rdfs:isDefinedBy :Package_CDPSM2015_Versions ;
  uml:id "EAID_E46C312C_2296_448b_BD8F_889A26BE4A04" .

cim:IEC61970CIMVersion a owl:Class ;
  rdfs:label "IEC61970CIMVersion" ;
  rdfs:comment "This is the IEC 61970 CIM version number assigned to this UML model."@en ;
  rdfs:isDefinedBy :Package_CDPSM2015_Versions ;
  uml:id "EAID_D7DB6F76_F0D2_4df0_ADBA_8450E821106F" .

cim:IdentifiedObject a owl:Class ;
  rdfs:label "IdentifiedObject" ;
  rdfs:comment "This is a root class to provide common identification for all classes needing identification and naming attributes"@en ;
  rdfs:isDefinedBy :Package_Standard ;
  uml:id "EAID_1E5E1F43_54EA_41f7_B60C_B71DB9A5F522" .

cim:LifecycleDate a owl:Class ;
  rdfs:label "LifecycleDate" ;
  rdfs:comment "Dates for lifecycle events of an asset."@en ;
  rdfs:isDefinedBy :Package_CompoundTypes ;
  uml:hasStereotype uml:compound ;
  uml:id "EAID_071DD356_C080_45a8_8665_642A87AE1C75" .

cim:LimitTypeKind a owl:Class ;
  rdfs:label "LimitTypeKind" ;
  rdfs:comment "The enumeration defines the kinds of the limit types."@en ;
  rdfs:isDefinedBy :Package_EntsoeExtensions ;
  uml:hasStereotype uml:entsoe, uml:enumeration ;
  uml:id "EAID_F74847DE_6251_4d32_A07F_F0B465A31CB1" .

cim:Manufacturer a owl:Class ;
  rdfs:label "Manufacturer" ;
  rdfs:comment "Organisation that manufactures asset products."@en ;
  rdfs:isDefinedBy :Package_Standard ;
  rdfs:subClassOf cim:OrganisationRole ;
  uml:id "EAID_0B0A35C0_2194_4e45_831A_292AE8DB46BA" .

cim:Name a owl:Class ;
  rdfs:label "Name" ;
  rdfs:comment "The Name class provides the means to define any number of human readable  names for an object. A name is <b>not</b> to be used for defining inter-object relationships. For inter-object relationships instead use the object identification 'mRID'."@en ;
  rdfs:isDefinedBy :Package_Standard ;
  uml:id "EAID_C947EB48_D33D_4033_A6A1_F23B1ACB95D6" .

cim:NameType a owl:Class ;
  rdfs:label "NameType" ;
  rdfs:comment """Type of name. Possible values for attribute 'name' are implementation dependent but standard profiles may specify types. An enterprise may have multiple IT systems each having its own local name for the same object, e.g. a planning system may have different names from an EMS. An object may also have different names within the same IT system, e.g. localName and aliasName as defined in CIM version 14. Their definitions from CIM14 are
      The localName is a human readable name of the object. It is only used with objects organized in a naming hierarchy. localName: A free text name local to a node in a naming hierarchy similar to a file directory structure. A power system related naming hierarchy may be: Substation, VoltageLevel, Equipment etc. Children of the same parent in such a hierarchy have names that typically are unique among them.
      aliasName: A free text alternate name typically used in tabular reports where the column width is limited."""@en ;
  rdfs:isDefinedBy :Package_Standard ;
  uml:id "EAID_01966DF3_6311_4695_918E_CEADEC6CBD62" .

cim:NameTypeAuthority a owl:Class ;
  rdfs:label "NameTypeAuthority" ;
  rdfs:comment "Authority responsible for creation and management of names of a given type; typically an organization or an enterprise system."@en ;
  rdfs:isDefinedBy :Package_Standard ;
  uml:id "EAID_1EF26656_130D_42b3_8941_2B7A369524C1" .

cim:NoLoadTest a owl:Class ;
  rdfs:label "NoLoadTest" ;
  rdfs:comment """No-load test results determine core admittance parameters. They include exciting current and core loss measurements from applying voltage to one winding.  The excitation may be positive sequence or zero
      sequence.  The test may be repeated at different voltages to measure saturation."""@en ;
  rdfs:isDefinedBy :Package_Standard ;
  rdfs:subClassOf cim:TransformerTest ;
  uml:id "EAID_F97BFB9F_4C97_4cea_BDEB_3FF5633F1360" .

cim:OperatingParticipant a owl:Class ;
  rdfs:label "OperatingParticipant" ;
  rdfs:comment "An operator of multiple power system resource objects. Note multple operating participants may operate the same power system resource object.   This can be used for modeling jointly owned units where each owner operates as a contractual share."@en ;
  rdfs:isDefinedBy :Package_Standard ;
  rdfs:subClassOf next2:OrganisationRoleEx ;
  uml:id "EAID_95EF5F86_52DD_457f_9556_D313D07C3003" .

cim:OperationalLimitDirectionKind a owl:Class ;
  rdfs:label "OperationalLimitDirectionKind" ;
  rdfs:comment "The direction attribute describes the side of  a limit that is a violation."@en ;
  rdfs:isDefinedBy :Package_CIMEnumerations ;
  uml:hasStereotype uml:enumeration ;
  uml:id "EAID_851C85E6_4C7C_4fa1_ADC6_85BD43EBEE2D" .

cim:Organisation a owl:Class ;
  rdfs:label "Organisation" ;
  rdfs:comment "Organisation that might have roles as utility, contractor, supplier, manufacturer, customer, etc."@en ;
  rdfs:isDefinedBy :Package_Standard ;
  rdfs:subClassOf cim:IdentifiedObject ;
  uml:id "EAID_495178C9_ECFA_47a9_A809_76793E46AF8C" .

cim:OrganisationRole a owl:Class ;
  rdfs:label "OrganisationRole" ;
  rdfs:comment "Identifies a way in which an organisation may participate in the utility enterprise (e.g., customer, manufacturer, etc)."@en ;
  rdfs:isDefinedBy :Package_Standard ;
  rdfs:subClassOf cim:IdentifiedObject ;
  uml:id "EAID_C2DFBC9E_FE40_468e_B6FE_2C6EC0B2F6B0" .

cim:OrientationKind a owl:Class ;
  rdfs:label "OrientationKind" ;
  rdfs:comment "The orientation of the coordinate system with respect to top, left, and the coordinate number system."@en ;
  rdfs:isDefinedBy :Package_CIMEnumerations ;
  uml:hasStereotype uml:enumeration ;
  uml:id "EAID_D1EF0087_BDE5_4b00_8462_DF7B5DD2CA29" .

cim:OverheadWireInfo a owl:Class ;
  rdfs:label "OverheadWireInfo" ;
  rdfs:comment "Overhead wire data."@en ;
  rdfs:isDefinedBy :Package_Standard ;
  rdfs:subClassOf cim:WireInfo ;
  uml:id "EAID_1D6B7F4B_00BA_4016_8B40_9DE87ADF6AA5" .

cim:PSREventKind a owl:Class ;
  rdfs:label "PSREventKind" ;
  rdfs:comment "Kind of power system resource event."@en ;
  rdfs:isDefinedBy :Package_CIMEnumerations ;
  uml:hasStereotype uml:enumeration ;
  uml:id "EAID_72380D15_60A8_4a30_8311_256442CAA6EA" .

cim:ParentOrganization a owl:Class ;
  rdfs:label "ParentOrganization" ;
  rdfs:isDefinedBy :Package_Standard ;
  rdfs:subClassOf cim:Organisation ;
  uml:id "EAID_993DDC75_6EEB_4c2e_909F_D344D6D169CB" .

cim:PerLengthImpedance a owl:Class ;
  rdfs:label "PerLengthImpedance" ;
  rdfs:comment "Common type for per-length impedance electrical catalogues."@en ;
  rdfs:isDefinedBy :Package_Standard ;
  rdfs:subClassOf cim:PerLengthLineParameter ;
  uml:id "EAID_B108607B_974D_4ad8_AFCC_05762EE79112" .

cim:PerLengthLineParameter a owl:Class ;
  rdfs:label "PerLengthLineParameter" ;
  rdfs:comment "Common type for per-length electrical catalogues describing line parameters."@en ;
  rdfs:isDefinedBy :Package_Standard ;
  rdfs:subClassOf cim:IdentifiedObject ;
  uml:id "EAID_F021874E_E30A_4ecf_8EF6_0063C8013FCE" .

cim:PerLengthPhaseImpedance a owl:Class ;
  rdfs:label "PerLengthPhaseImpedance" ;
  rdfs:comment "Impedance and admittance parameters per unit length for n-wire unbalanced lines, in matrix form."@en ;
  rdfs:isDefinedBy :Package_Standard ;
  rdfs:subClassOf cim:PerLengthImpedance ;
  uml:id "EAID_AE50C888_C180_429e_B726_F99C09A42AB2" .

cim:PerLengthSequenceImpedance a owl:Class ;
  rdfs:label "PerLengthSequenceImpedance" ;
  rdfs:comment "Sequence impedance and admittance parameters per unit length, for transposed lines of 1, 2, or 3 phases. For 1-phase lines, define x=x0=xself. For 2-phase lines, define x=xs-xm and x0=xs+xm."@en ;
  rdfs:isDefinedBy :Package_Standard ;
  rdfs:subClassOf cim:PerLengthImpedance ;
  uml:id "EAID_62811080_C3DC_4119_BCFC_BB75BD1AF996" .

cim:PhaseCode a owl:Class ;
  rdfs:label "PhaseCode" ;
  rdfs:comment """Enumeration of phase identifiers. Allows designation of phases for both transmission and distribution equipment, circuits and loads.
      Residential and small commercial loads are often served from single-phase, or split-phase, secondary circuits. Phases 1 and 2 refer to hot wires that are 180 degrees out of phase, while N refers to the neutral wire. Through single-phase transformer connections, these secondary circuits may be served from one or two of the primary phases A, B, and C. For three-phase loads, use the A, B, C phase codes instead of s12N."""@en ;
  rdfs:isDefinedBy :Package_CIMEnumerations ;
  uml:hasStereotype uml:enumeration ;
  uml:id "EAID_4725DEF0_D125_4768_99B3_4AC3649D5D11" .

cim:PhaseImpedanceData a owl:Class ;
  rdfs:label "PhaseImpedanceData" ;
  rdfs:comment "Triplet of resistance, reactance, and susceptance matrix element values."@en ;
  rdfs:isDefinedBy :Package_Standard ;
  uml:id "EAID_1AB60DC8_B4D0_42ac_AB35_9B517E0470BA" .

cim:PowerTransformerInfo a owl:Class ;
  rdfs:label "PowerTransformerInfo" ;
  rdfs:comment "Set of power transformer data, from an equipment library."@en ;
  rdfs:isDefinedBy :Package_Standard ;
  rdfs:subClassOf next:PowerTransformerInfoEx ;
  uml:id "EAID_A23CE505_160C_48f7_9E91_957FFC5B0D27" .

cim:ProductAssetModel a owl:Class ;
  rdfs:label "ProductAssetModel" ;
  rdfs:comment "Asset model by a specific manufacturer."@en ;
  rdfs:isDefinedBy :Package_Standard ;
  rdfs:subClassOf cim:IdentifiedObject ;
  uml:id "EAID_2EA6E6E2_6DD6_4634_B6E1_B1035C7F8712" .

cim:RE_UnitMultiplier a owl:Class ;
  rdfs:label "RE_UnitMultiplier" ;
  rdfs:comment "The unit multipliers defined for the CIM"@en ;
  rdfs:isDefinedBy :Package_CIMEnumerations ;
  uml:hasStereotype uml:enumeration ;
  uml:id "EAID_CCD2B42A_2923_46e8_8908_ABA4A853B758" .

cim:RE_UnitSymbol a owl:Class ;
  rdfs:label "RE_UnitSymbol" ;
  rdfs:comment "The units defiend for usage in the CIM"@en ;
  rdfs:isDefinedBy :Package_CIMEnumerations ;
  uml:hasStereotype uml:enumeration ;
  uml:id "EAID_82CF8971_5F46_440c_88F3_A1B5783F9EA7" .

cim:RegulatingControlModeKind a owl:Class ;
  rdfs:label "RegulatingControlModeKind" ;
  rdfs:comment "The kind of regulation model.   For example regulating voltage, reactive power, active power, etc."@en ;
  rdfs:isDefinedBy :Package_CIMEnumerations ;
  uml:hasStereotype uml:enumeration ;
  uml:id "EAID_69E37D4A_38E7_4ba8_8F1B_2E0DC8735AAD" .

cim:ShortCircuitTest a owl:Class ;
  rdfs:label "ShortCircuitTest" ;
  rdfs:comment "Short-circuit test results determine mesh impedance parameters. They include load losses and leakage impedances.  For three-phase windings, the excitation can be positive sequence (the default) or zero sequence. There must be at least one grounded winding."@en ;
  rdfs:isDefinedBy :Package_Standard ;
  rdfs:subClassOf cim:TransformerTest ;
  uml:id "EAID_124F00C1_D9A6_42f1_A6F4_629206316507" .

cim:ShuntCompensatorInfo a owl:Class ;
  rdfs:label "ShuntCompensatorInfo" ;
  rdfs:comment "Properties of shunt capacitor, shunt reactor or switchable bank of shunt capacitor or reactor assets."@en ;
  rdfs:isDefinedBy :Package_Standard ;
  rdfs:subClassOf cim:AssetInfo ;
  uml:id "EAID_2F9AE477_C9C3_4af9_8CBE_73B4476A8ACF" .

cim:SinglePhaseKind a owl:Class ;
  rdfs:label "SinglePhaseKind" ;
  rdfs:comment "Enumeration of single phase identifiers. Allows designation of single phases for both transmission and distribution equipment, circuits and loads."@en ;
  rdfs:isDefinedBy :Package_CIMEnumerations ;
  uml:hasStereotype uml:enumeration ;
  uml:id "EAID_F2284250_7D26_434c_BF35_98EA18648856" .

cim:Source a owl:Class ;
  rdfs:label "Source" ;
  rdfs:comment "Source gives information related to the origin of a value."@en ;
  rdfs:isDefinedBy :Package_CIMEnumerations ;
  uml:hasStereotype uml:enumeration ;
  uml:id "EAID_7CF6775C_176F_4790_9985_E2A403F01F15" .

cim:Status a owl:Class ;
  rdfs:label "Status" ;
  rdfs:comment "Current status information relevant to an entity."@en ;
  rdfs:isDefinedBy :Package_CompoundTypes ;
  uml:hasStereotype uml:compound ;
  uml:id "EAID_C289C1B8_B2A7_44dc_9539_6FF6A864D9A7" .

cim:StreetAddress a owl:Class ;
  rdfs:label "StreetAddress" ;
  rdfs:comment "General purpose street address information."@en ;
  rdfs:isDefinedBy :Package_CompoundTypes ;
  uml:hasStereotype uml:compound ;
  uml:id "EAID_4E00C826_D63A_4b62_A6AA_D3C86C1D8D9A" .

cim:StreetDetail a owl:Class ;
  rdfs:label "StreetDetail" ;
  rdfs:comment "Street details, in the context of address."@en ;
  rdfs:isDefinedBy :Package_CompoundTypes ;
  uml:hasStereotype uml:compound ;
  uml:id "EAID_2896C068_81B3_4338_8314_BF55C9D20652" .

cim:SwitchInfo a owl:Class ;
  rdfs:label "SwitchInfo" ;
  rdfs:comment "Switch data."@en ;
  rdfs:isDefinedBy :Package_Standard ;
  rdfs:subClassOf cim:AssetInfo ;
  uml:id "EAID_EC1BB432_7139_435d_B872_F0FFB942DDCA" .

cim:SynchronousMachineKind a owl:Class ;
  rdfs:label "SynchronousMachineKind" ;
  rdfs:comment "Synchronous machine type."@en ;
  rdfs:isDefinedBy :Package_CIMEnumerations ;
  uml:hasStereotype uml:enumeration ;
  uml:id "EAID_0271C369_418B_4753_97E7_8F46A0235E90" .

cim:SynchronousMachineOperatingMode a owl:Class ;
  rdfs:label "SynchronousMachineOperatingMode" ;
  rdfs:comment "Synchronous machine operating mode."@en ;
  rdfs:isDefinedBy :Package_CIMEnumerations ;
  uml:hasStereotype uml:enumeration ;
  uml:id "EAID_9E79D1F1_41A0_49fe_85FD_4B4E849646A4" .

cim:TapChangerInfo a owl:Class ;
  rdfs:label "TapChangerInfo" ;
  rdfs:comment "Tap changer data."@en ;
  rdfs:isDefinedBy :Package_Standard ;
  rdfs:subClassOf cim:AssetInfo ;
  uml:id "EAID_063AAC4D_7539_40bf_918C_54C7C509104B" .

cim:TownDetail a owl:Class ;
  rdfs:label "TownDetail" ;
  rdfs:comment "Town details, in the context of address."@en ;
  rdfs:isDefinedBy :Package_CompoundTypes ;
  uml:hasStereotype uml:compound ;
  uml:id "EAID_F6B511C6_7BF1_4322_9D5A_CECDA55A1F3F" .

cim:TransformerControlMode a owl:Class ;
  rdfs:label "TransformerControlMode" ;
  rdfs:comment "Control modes for a transformer."@en ;
  rdfs:isDefinedBy :Package_CIMEnumerations ;
  uml:hasStereotype uml:enumeration ;
  uml:id "EAID_30994180_C510_4a68_9CF1_36A25A1F79B5" .

cim:TransformerEndInfo a owl:Class ;
  rdfs:label "TransformerEndInfo" ;
  rdfs:comment "Transformer end data."@en ;
  rdfs:isDefinedBy :Package_Standard ;
  rdfs:subClassOf cim:AssetInfo ;
  uml:id "EAID_6121FF50_58BB_4854_A8EC_6B82CD512C1E" .

cim:TransformerTankInfo a owl:Class ;
  rdfs:label "TransformerTankInfo" ;
  rdfs:comment "Set of transformer tank data, from an equipment library."@en ;
  rdfs:isDefinedBy :Package_Standard ;
  rdfs:subClassOf cim:AssetInfo ;
  uml:id "EAID_A83B2E46_DC61_4017_8D97_E05E99078582" .

cim:TransformerTest a owl:Class ;
  rdfs:label "TransformerTest" ;
  rdfs:comment "Test result for transformer ends, such as short-circuit, open-circuit (excitation) or no-load test."@en ;
  rdfs:isDefinedBy :Package_Standard ;
  rdfs:subClassOf cim:IdentifiedObject ;
  uml:id "EAID_9545B21B_1178_4e07_A433_DAC4731130E2" .

cim:UnitMultiplier a owl:Class ;
  rdfs:label "UnitMultiplier" ;
  rdfs:comment "The unit multipliers defined for the CIM"@en ;
  rdfs:isDefinedBy :Package_CIMEnumerations ;
  uml:hasStereotype uml:enumeration ;
  uml:id "EAID_64CEA0C6_6C26_41bd_B02E_00CF2F02A294" .

cim:UnitSymbol a owl:Class ;
  rdfs:label "UnitSymbol" ;
  rdfs:comment "The units defined for usage in the CIM."@en ;
  rdfs:isDefinedBy :Package_CIMEnumerations ;
  uml:hasStereotype uml:enumeration ;
  uml:id "EAID_0A91C126_5421_4ec9_868D_FAA0E1B091A9" .

cim:WindGenUnitKind a owl:Class ;
  rdfs:label "WindGenUnitKind" ;
  rdfs:comment "Kind of wind generating unit."@en ;
  rdfs:isDefinedBy :Package_CIMEnumerations ;
  uml:hasStereotype uml:enumeration ;
  uml:id "EAID_E7574EE8_C9C2_4466_B309_787007D5DA32" .

cim:WindingConnection a owl:Class ;
  rdfs:label "WindingConnection" ;
  rdfs:comment "Winding connection type."@en ;
  rdfs:isDefinedBy :Package_CIMEnumerations ;
  uml:hasStereotype uml:enumeration ;
  uml:id "EAID_2079870A_25A3_4d77_98C3_B142C2FD391D" .

cim:WireAssemblyInfo a owl:Class ;
  rdfs:label "WireAssemblyInfo" ;
  rdfs:isDefinedBy :Package_Standard ;
  rdfs:subClassOf cim:AssetInfo ;
  uml:id "EAID_8E4CA764_FCF9_4d7b_ADB0_1462ED8D8EAA" .

cim:WireInfo a owl:Class ;
  rdfs:label "WireInfo" ;
  rdfs:comment "Wire data that can be specified per line segment phase, or for the line segment as a whole in case its phases all have the same wire characteristics."@en ;
  rdfs:isDefinedBy :Package_Standard ;
  rdfs:subClassOf next:WireInfoEx ;
  uml:id "EAID_86C395AF_F55A_473e_AA74_F8A41B5ABBDF" .

cim:WireInsulationKind a owl:Class ;
  rdfs:label "WireInsulationKind" ;
  rdfs:comment "Kind of wire insulation."@en ;
  rdfs:isDefinedBy :Package_CIMEnumerations ;
  uml:hasStereotype uml:enumeration ;
  uml:id "EAID_9C1C15AB_1FB5_4bd8_90AA_79939AC0A9F6" .

cim:WireMaterialKind a owl:Class ;
  rdfs:label "WireMaterialKind" ;
  rdfs:comment "Kind of wire material."@en ;
  rdfs:isDefinedBy :Package_CIMEnumerations ;
  uml:hasStereotype uml:enumeration ;
  uml:id "EAID_1F6368A6_BE59_418c_8DA4_DA1ACCA7A850" .

cim:WirePhaseInfo a owl:Class ;
  rdfs:label "WirePhaseInfo" ;
  rdfs:isDefinedBy :Package_Standard ;
  uml:id "EAID_826E3BB3_C218_42da_9FA8_E161C4202D2B" .

cim:WirePosition a owl:Class ;
  rdfs:label "WirePosition" ;
  rdfs:comment "Identification, spacing and configuration of the wires of a conductor with respect to a structure."@en ;
  rdfs:isDefinedBy :Package_Standard ;
  rdfs:subClassOf cim:IdentifiedObject ;
  uml:id "EAID_AFE916CC_C901_41ff_850C_0F77B9496B9D" .

cim:WireSpacing a owl:Class ;
  rdfs:label "WireSpacing" ;
  rdfs:comment "Wire spacing data that associates multiple wire positions with the line segment, and allows to calculate line segment impedances. Number of phases can be derived from the number of associated wire positions whose phase is not neutral."@en ;
  rdfs:isDefinedBy :Package_Standard ;
  rdfs:subClassOf cim:AssetInfo ;
  uml:id "EAID_B91EA4FE_F4A2_4492_939F_D6C57F9E06E5" .

cim:WireUsageKind a owl:Class ;
  rdfs:label "WireUsageKind" ;
  rdfs:comment "Kind of wire usage."@en ;
  rdfs:isDefinedBy :Package_CIMEnumerations ;
  uml:hasStereotype uml:enumeration ;
  uml:id "EAID_3307BFA5_45D7_4cf5_91BD_0AA72AB03138" .

md:Description a owl:Class ;
  rdfs:label "Description" ;
  rdfs:comment "Identity contain comon descriptive information."@en ;
  rdfs:isDefinedBy :Package_ModelDescription ;
  uml:hasStereotype uml:deprecated ;
  uml:id "EAID_EA6429C5_DBE5_4667_A4E7_9B691DCB27C7" .

md:DescriptionID a owl:Class ;
  rdfs:label "DescriptionID" ;
  rdfs:isDefinedBy :Package_ModelDescription ;
  rdfs:subClassOf md:Description ;
  uml:hasStereotype uml:deprecated ;
  uml:id "EAID_11C3E838_F554_495b_9C57_BF88D3E00C11" .

md:DifferenceModel a owl:Class ;
  rdfs:label "DifferenceModel" ;
  rdfs:isDefinedBy :Package_ModelDescription ;
  rdfs:subClassOf md:Model ;
  uml:id "EAID_96A36E86_5379_448d_9604_56095A1905CE" .

md:FullModel a owl:Class ;
  rdfs:label "FullModel" ;
  rdfs:isDefinedBy :Package_ModelDescription ;
  rdfs:subClassOf md:Model ;
  uml:id "EAID_66403EF1_5399_499b_9023_9A568B9EDE41" .

md:FullModelDocumentElement a owl:Class ;
  rdfs:label "FullModelDocumentElement" ;
  rdfs:isDefinedBy :Package_ModelDescription ;
  uml:hasStereotype uml:deprecated ;
  uml:id "EAID_7D924A77_DD88_4aca_9D53_3285248B856D" .

md:Model a owl:Class ;
  rdfs:label "Model" ;
  rdfs:isDefinedBy :Package_ModelDescription ;
  uml:id "EAID_B6CC60A3_3A7C_4d1e_B87B_34B75E586359" .

md:ModelDescriptionCIMVersion a owl:Class ;
  rdfs:label "ModelDescriptionCIMVersion" ;
  rdfs:isDefinedBy :Package_ModelDescription ;
  uml:id "EAID_E5EE368A_4650_44ad_BE63_43EE2D9DFF2B" .

md:Statements a owl:Class ;
  rdfs:label "Statements" ;
  rdfs:isDefinedBy :Package_ModelDescription ;
  rdfs:subClassOf md:FullModelDocumentElement ;
  uml:id "EAID_1DF18623_9167_4901_9EA6_33DE8A0733D5" .

next2:OrganisationRoleEx a owl:Class ;
  rdfs:label "OrganisationRoleEx" ;
  rdfs:comment """Extension defined to add ROle Link to Organisation for classes that should be a specialisation of OrganisationRole and for which this is missing.
      Example: OperatingParticipant."""@en ;
  rdfs:isDefinedBy :Package_CIMExtensions ;
  rdfs:subClassOf cim:IdentifiedObject ;
  uml:hasStereotype uml:extension ;
  uml:id "EAID_68357F3A_653B_427a_A631_09504CB6DECA" .

next3:ShuntCompensatorControl a owl:Class ;
  rdfs:label "ShuntCompensatorControl" ;
  rdfs:comment "Distribution capacitor bank control settings."@en ;
  rdfs:isDefinedBy :Package_InfIEC61968 ;
  rdfs:subClassOf cim:IdentifiedObject ;
  uml:id "EAID_A25E4B55_FF9B_4ada_AD40_93D33258241F" .

next3:TypeAssetCatalogue a owl:Class ;
  rdfs:label "TypeAssetCatalogue" ;
  rdfs:comment "Catalogue of generic types of assets (TypeAsset) that may be used for design purposes. It is not associated with a particular manufacturer."@en ;
  rdfs:isDefinedBy :Package_InfIEC61968 ;
  rdfs:subClassOf cim:IdentifiedObject ;
  uml:id "EAID_A845114A_E466_4532_876D_9EA46E87E675" .

next:PowerTransformerInfoEx a owl:Class ;
  rdfs:label "PowerTransformerInfoEx" ;
  rdfs:isDefinedBy :Package_EDFExtensions ;
  rdfs:subClassOf cim:AssetInfo ;
  uml:hasStereotype uml:extension ;
  uml:id "EAID_690022EE_5B16_41e9_8A0D_4DAC4F6F9DDD" .

next:WireInfoEx a owl:Class ;
  rdfs:label "WireInfo" ;
  rdfs:comment "Voltage level the wire is intended for."@en ;
  rdfs:isDefinedBy :Package_EDFExtensions ;
  rdfs:subClassOf cim:AssetInfo ;
  uml:hasStereotype uml:extension ;
  uml:id "EAID_5BD59EAC_A29B_4571_AB39_6AE01B959202" .

uml:Package a owl:Class .

uml:Stereotype a owl:Class .

:ModelingAuthority.ModelingAuthoritySets a owl:ObjectProperty, owl:InverseFunctionalProperty ;
  rdfs:label "ModelingAuthoritySets" ;
  rdfs:comment "A Modeling Authority set supplies and maintains the data for the objects in a Modeling Authority Set."@en ;
  owl:inverseOf :ModelingAuthoritySet.ModelingAuthority ;
  rdfs:domain :ModelingAuthority ;
  rdfs:isDefinedBy :Package_ModelAuthority ;
  rdfs:range :ModelingAuthoritySet ;
  uml:id "EAID_DD1413D0_73ED_4d90_8ADB_E87B483F7D14-A" .

:ModelingAuthoritySet.ModelingAuthority a owl:ObjectProperty, owl:FunctionalProperty ;
  rdfs:label "ModelingAuthority" ;
  rdfs:comment "A Modeling Authority set supplies and maintains the data for the objects in a Modeling Authority Set."@en ;
  owl:inverseOf :ModelingAuthority.ModelingAuthoritySets ;
  rdfs:domain :ModelingAuthoritySet ;
  rdfs:isDefinedBy :Package_ModelAuthority ;
  rdfs:range :ModelingAuthority ;
  uml:id "EAID_DD1413D0_73ED_4d90_8ADB_E87B483F7D14-B" .

:PowerSystemProjectSchedule.status a owl:ObjectProperty, owl:FunctionalProperty ;
  rdfs:label "status" ;
  rdfs:domain :PowerSystemProjectSchedule ;
  rdfs:isDefinedBy :Package_PowerSystemProject ;
  rdfs:range :ProjectStepStatusKind ;
  uml:hasStereotype uml:attribute ;
  uml:id "EAID_A2782127_6316_4c7a_8FD3_0BAFF34696EA" .

:PowerSystemProjectSchedule.stepType a owl:ObjectProperty, owl:FunctionalProperty ;
  rdfs:label "stepType" ;
  rdfs:domain :PowerSystemProjectSchedule ;
  rdfs:isDefinedBy :Package_PowerSystemProject ;
  rdfs:range :StepKind ;
  uml:hasStereotype uml:attribute ;
  uml:id "EAID_E5F56033_237D_4136_B67F_992E49D34D4C" .

:ProjectStep.status a owl:ObjectProperty, owl:FunctionalProperty ;
  rdfs:label "status" ;
  rdfs:domain :ProjectStep ;
  rdfs:isDefinedBy :Package_PowerSystemProject ;
  rdfs:range :ProjectStepStatusKind ;
  uml:hasStereotype uml:attribute ;
  uml:id "EAID_066625C1_EB9A_4637_A571_09C23BB3A0ED" .

:ProjectStep.stepType a owl:ObjectProperty, owl:FunctionalProperty ;
  rdfs:label "stepType" ;
  rdfs:domain :ProjectStep ;
  rdfs:isDefinedBy :Package_PowerSystemProject ;
  rdfs:range :StepKind ;
  uml:hasStereotype uml:attribute ;
  uml:id "EAID_949103D0_A373_4f5d_BC2A_8CE9427856FA" .

cim:AssetInfo.CatalogAssetType a owl:ObjectProperty, owl:FunctionalProperty, owl:InverseFunctionalProperty ;
  rdfs:label "CatalogAssetType" ;
  owl:inverseOf cim:CatalogAssetType.AssetInfo ;
  rdfs:domain cim:AssetInfo ;
  rdfs:isDefinedBy :Package_Standard ;
  rdfs:range cim:CatalogAssetType ;
  uml:id "EAID_7327A8D8_F544_48a5_9933_747268D5F7DD-B" .

cim:AssetInfo.ProductAssetModel a owl:ObjectProperty, owl:FunctionalProperty, owl:InverseFunctionalProperty ;
  rdfs:label "ProductAssetModel" ;
  owl:inverseOf cim:ProductAssetModel.AssetInfo ;
  rdfs:domain cim:AssetInfo ;
  rdfs:isDefinedBy :Package_Standard ;
  rdfs:range cim:ProductAssetModel ;
  uml:id "EAID_CCB697D1_E4FE_424f_8CCF_56E8AF800314-B" .

cim:BusbarSectionInfo.ratedCurrent a owl:ObjectProperty, owl:DatatypeProperty, owl:FunctionalProperty ;
  rdfs:label "ratedCurrent" ;
  rdfs:comment "Rated current."@en ;
  rdfs:domain cim:BusbarSectionInfo ;
  rdfs:isDefinedBy :Package_Standard ;
  rdfs:range cim:CurrentFlow ;
  uml:hasStereotype uml:attribute ;
  uml:id "EAID_28464C19_18C8_4c00_B90D_23584DC607CA" .

cim:BusbarSectionInfo.ratedVoltage a owl:ObjectProperty, owl:DatatypeProperty, owl:FunctionalProperty ;
  rdfs:label "ratedVoltage" ;
  rdfs:comment "Rated voltage."@en ;
  rdfs:domain cim:BusbarSectionInfo ;
  rdfs:isDefinedBy :Package_Standard ;
  rdfs:range cim:Voltage ;
  uml:hasStereotype uml:attribute ;
  uml:id "EAID_6BA735F6_E26C_4332_9527_3E6588740C58" .

cim:CableInfo.constructionKind a owl:ObjectProperty, owl:FunctionalProperty ;
  rdfs:label "constructionKind" ;
  rdfs:comment "Kind of construction of this cable."@en ;
  rdfs:domain cim:CableInfo ;
  rdfs:isDefinedBy :Package_Standard ;
  rdfs:range cim:CableConstructionKind ;
  uml:hasStereotype uml:attribute ;
  uml:id "EAID_7E46F832_C0A1_438d_9A81_33D8BB2B30DE" .

cim:CatalogAssetType.AssetInfo a owl:ObjectProperty, owl:FunctionalProperty, owl:InverseFunctionalProperty ;
  rdfs:label "AssetInfo" ;
  owl:inverseOf cim:AssetInfo.CatalogAssetType ;
  rdfs:domain cim:CatalogAssetType ;
  rdfs:isDefinedBy :Package_Standard ;
  rdfs:range cim:AssetInfo ;
  uml:id "EAID_7327A8D8_F544_48a5_9933_747268D5F7DD-A" .

cim:EndDeviceInfo.ratedCurrent a owl:ObjectProperty, owl:DatatypeProperty, owl:FunctionalProperty ;
  rdfs:label "ratedCurrent" ;
  rdfs:comment "Rated current."@en ;
  rdfs:domain cim:EndDeviceInfo ;
  rdfs:isDefinedBy :Package_Standard ;
  rdfs:range cim:CurrentFlow ;
  uml:hasStereotype uml:attribute ;
  uml:id "EAID_A5C6D8A4_BCB0_4f8d_B302_044630250D4E" .

cim:EndDeviceInfo.ratedVoltage a owl:ObjectProperty, owl:DatatypeProperty, owl:FunctionalProperty ;
  rdfs:label "ratedVoltage" ;
  rdfs:comment "Rated voltage."@en ;
  rdfs:domain cim:EndDeviceInfo ;
  rdfs:isDefinedBy :Package_Standard ;
  rdfs:range cim:Voltage ;
  uml:hasStereotype uml:attribute ;
  uml:id "EAID_19E62125_0FB5_4163_A49E_78C6038A1190" .

cim:IdentifiedObject.Names a owl:ObjectProperty, owl:InverseFunctionalProperty ;
  rdfs:label "Names" ;
  rdfs:comment "All names of this identified object."@en ;
  owl:inverseOf cim:Name.IdentifiedObject ;
  rdfs:domain cim:IdentifiedObject ;
  rdfs:isDefinedBy :Package_Standard ;
  rdfs:range cim:Name ;
  uml:id "EAID_4DC1EF2E_B36F_4630_BD70_70A716EF48C8-B" .

cim:Manufacturer.ProductAssetModel a owl:ObjectProperty, owl:InverseFunctionalProperty ;
  rdfs:label "ProductAssetModel" ;
  rdfs:comment "All asset models by this manufacturer."@en ;
  owl:inverseOf cim:ProductAssetModel.Manufacturer ;
  rdfs:domain cim:Manufacturer ;
  rdfs:isDefinedBy :Package_Standard ;
  rdfs:range cim:ProductAssetModel ;
  uml:id "EAID_9413325B_DAA3_4fea_A516_89BBF10173DF-B" .

cim:Name.IdentifiedObject a owl:ObjectProperty, owl:FunctionalProperty ;
  rdfs:label "IdentifiedObject" ;
  rdfs:comment "Identified object that this name designates."@en ;
  owl:inverseOf cim:IdentifiedObject.Names ;
  rdfs:domain cim:Name ;
  rdfs:isDefinedBy :Package_Standard ;
  rdfs:range cim:IdentifiedObject ;
  uml:id "EAID_4DC1EF2E_B36F_4630_BD70_70A716EF48C8-A" .

cim:Name.NameType a owl:ObjectProperty, owl:FunctionalProperty ;
  rdfs:label "NameType" ;
  rdfs:comment "Type of this name."@en ;
  owl:inverseOf cim:NameType.Names ;
  rdfs:domain cim:Name ;
  rdfs:isDefinedBy :Package_Standard ;
  rdfs:range cim:NameType ;
  uml:id "EAID_C9CA7E15_2CD6_4880_A3C3_16D37A697A25-B" .

cim:NameType.NameTypeAuthority a owl:ObjectProperty, owl:FunctionalProperty ;
  rdfs:label "NameTypeAuthority" ;
  rdfs:comment "Authority responsible for managing names of this type."@en ;
  owl:inverseOf cim:NameTypeAuthority.NameTypes ;
  rdfs:domain cim:NameType ;
  rdfs:isDefinedBy :Package_Standard ;
  rdfs:range cim:NameTypeAuthority ;
  uml:id "EAID_4D45DB20_10E5_4f35_8516_E9A0FC9B44DC-A" .

cim:NameType.Names a owl:ObjectProperty, owl:InverseFunctionalProperty ;
  rdfs:label "Names" ;
  rdfs:comment "All names of this type."@en ;
  owl:inverseOf cim:Name.NameType ;
  rdfs:domain cim:NameType ;
  rdfs:isDefinedBy :Package_Standard ;
  rdfs:range cim:Name ;
  uml:id "EAID_C9CA7E15_2CD6_4880_A3C3_16D37A697A25-A" .

cim:NameTypeAuthority.NameTypes a owl:ObjectProperty, owl:InverseFunctionalProperty ;
  rdfs:label "NameTypes" ;
  rdfs:comment "All name types managed by this authority."@en ;
  owl:inverseOf cim:NameType.NameTypeAuthority ;
  rdfs:domain cim:NameTypeAuthority ;
  rdfs:isDefinedBy :Package_Standard ;
  rdfs:range cim:NameType ;
  uml:id "EAID_4D45DB20_10E5_4f35_8516_E9A0FC9B44DC-B" .

cim:NoLoadTest.EnergisedEnd a owl:ObjectProperty, owl:FunctionalProperty ;
  rdfs:label "EnergisedEnd" ;
  rdfs:comment "Transformer end that current is applied to in this no-load test."@en ;
  owl:inverseOf cim:TransformerEndInfo.EnergisedEndNoLoadTest ;
  rdfs:domain cim:NoLoadTest ;
  rdfs:isDefinedBy :Package_Standard ;
  rdfs:range cim:TransformerEndInfo ;
  uml:id "EAID_D9249600_6545_48c5_BB01_F3AC06385B23-A" .

cim:NoLoadTest.loss a owl:ObjectProperty, owl:DatatypeProperty, owl:FunctionalProperty ;
  rdfs:label "loss" ;
  rdfs:comment "Losses measured from a positive-sequence or single-phase excitation test."@en ;
  rdfs:domain cim:NoLoadTest ;
  rdfs:isDefinedBy :Package_Standard ;
  rdfs:range cim:KiloActivePower ;
  uml:hasStereotype uml:attribute ;
  uml:id "EAID_2D5C6EC9_7CDA_4324_B65B_24377EF0730E" .

cim:Organisation.ParentOrganisation a owl:ObjectProperty, owl:FunctionalProperty ;
  rdfs:label "ParentOrganisation" ;
  rdfs:comment "Parent organisation of this organisation."@en ;
  owl:inverseOf cim:ParentOrganization.Organisation ;
  rdfs:domain cim:Organisation ;
  rdfs:isDefinedBy :Package_Standard ;
  rdfs:range cim:ParentOrganization ;
  uml:id "EAID_0407A64E_5A0E_47bb_A6E0_A89797DFF73A-B" .

cim:OrganisationRole.Organisation a owl:ObjectProperty, owl:FunctionalProperty ;
  rdfs:label "Organisation" ;
  rdfs:comment "Organisation having this role."@en ;
  rdfs:domain cim:OrganisationRole ;
  rdfs:isDefinedBy :Package_Standard ;
  rdfs:range cim:Organisation ;
  uml:id "EAID_E8277819_0C96_46eb_A4CC_07181A2C2300-A" .

cim:ParentOrganization.Organisation a owl:ObjectProperty, owl:InverseFunctionalProperty ;
  rdfs:label "Organisation" ;
  rdfs:comment "Organisation that is part of this parent organisation."@en ;
  owl:inverseOf cim:Organisation.ParentOrganisation ;
  rdfs:domain cim:ParentOrganization ;
  rdfs:isDefinedBy :Package_Standard ;
  rdfs:range cim:Organisation ;
  uml:id "EAID_0407A64E_5A0E_47bb_A6E0_A89797DFF73A-A" .

cim:PerLengthLineParameter.WireAssemblyInfo a owl:ObjectProperty, owl:FunctionalProperty ;
  rdfs:label "WireAssemblyInfo" ;
  rdfs:comment "A WireAssemblyInfo is used to compute the PerLengthParameter data in the Wires package"@en ;
  owl:inverseOf cim:WireAssemblyInfo.PerLengthLineParameter ;
  rdfs:domain cim:PerLengthLineParameter ;
  rdfs:isDefinedBy :Package_Standard ;
  rdfs:range cim:WireAssemblyInfo ;
  uml:id "EAID_98CE9D77_13DF_4983_93BD_7E438547A4BE-B" .

cim:PerLengthPhaseImpedance.PhaseImpedanceData a owl:ObjectProperty, owl:InverseFunctionalProperty ;
  rdfs:label "PhaseImpedanceData" ;
  rdfs:comment "All data that belong to this conductor phase impedance."@en ;
  owl:inverseOf cim:PhaseImpedanceData.PhaseImpedance ;
  rdfs:domain cim:PerLengthPhaseImpedance ;
  rdfs:isDefinedBy :Package_Standard ;
  rdfs:range cim:PhaseImpedanceData ;
  uml:id "EAID_918A88CD_E0A4_4abb_A371_853D33F0CA98-B" .

cim:PerLengthSequenceImpedance.b0ch a owl:ObjectProperty, owl:DatatypeProperty, owl:FunctionalProperty ;
  rdfs:label "b0ch" ;
  rdfs:comment "Zero sequence shunt (charging) susceptance, per unit of length."@en ;
  rdfs:domain cim:PerLengthSequenceImpedance ;
  rdfs:isDefinedBy :Package_Standard ;
  rdfs:range cim:SusceptancePerLength ;
  uml:hasStereotype uml:attribute ;
  uml:id "EAID_2CBFC123_60BB_4778_83BB_D7DC67F47AB4" .

cim:PerLengthSequenceImpedance.bch a owl:ObjectProperty, owl:DatatypeProperty, owl:FunctionalProperty ;
  rdfs:label "bch" ;
  rdfs:comment "Positive sequence shunt (charging) susceptance, per unit of length."@en ;
  rdfs:domain cim:PerLengthSequenceImpedance ;
  rdfs:isDefinedBy :Package_Standard ;
  rdfs:range cim:SusceptancePerLength ;
  uml:hasStereotype uml:attribute ;
  uml:id "EAID_B2B74726_086F_4b5a_A223_EB38E25EE5F5" .

cim:PerLengthSequenceImpedance.g0ch a owl:ObjectProperty, owl:DatatypeProperty, owl:FunctionalProperty ;
  rdfs:label "g0ch" ;
  rdfs:comment "Zero sequence shunt (charging) conductance, per unit of length."@en ;
  rdfs:domain cim:PerLengthSequenceImpedance ;
  rdfs:isDefinedBy :Package_Standard ;
  rdfs:range cim:ConductancePerLength ;
  uml:hasStereotype uml:attribute ;
  uml:id "EAID_EE085440_7095_4562_A152_AE761E9451B3" .

cim:PerLengthSequenceImpedance.gch a owl:ObjectProperty, owl:DatatypeProperty, owl:FunctionalProperty ;
  rdfs:label "gch" ;
  rdfs:comment "Positive sequence shunt (charging) conductance, per unit of length."@en ;
  rdfs:domain cim:PerLengthSequenceImpedance ;
  rdfs:isDefinedBy :Package_Standard ;
  rdfs:range cim:ConductancePerLength ;
  uml:hasStereotype uml:attribute ;
  uml:id "EAID_9D47983F_BB5D_4670_846A_A6A5216E59FE" .

cim:PerLengthSequenceImpedance.r a owl:ObjectProperty, owl:DatatypeProperty, owl:FunctionalProperty ;
  rdfs:label "r" ;
  rdfs:comment "Positive sequence series resistance, per unit of length."@en ;
  rdfs:domain cim:PerLengthSequenceImpedance ;
  rdfs:isDefinedBy :Package_Standard ;
  rdfs:range cim:ResistancePerLength ;
  uml:hasStereotype uml:attribute ;
  uml:id "EAID_8FE892E4_453B_4599_8F05_21A684D989C4" .

cim:PerLengthSequenceImpedance.r0 a owl:ObjectProperty, owl:DatatypeProperty, owl:FunctionalProperty ;
  rdfs:label "r0" ;
  rdfs:comment "Zero sequence series resistance, per unit of length."@en ;
  rdfs:domain cim:PerLengthSequenceImpedance ;
  rdfs:isDefinedBy :Package_Standard ;
  rdfs:range cim:ResistancePerLength ;
  uml:hasStereotype uml:attribute ;
  uml:id "EAID_A112C7DC_968B_45e8_B850_6B201779C80A" .

cim:PerLengthSequenceImpedance.x a owl:ObjectProperty, owl:DatatypeProperty, owl:FunctionalProperty ;
  rdfs:label "x" ;
  rdfs:comment "Positive sequence series reactance, per unit of length."@en ;
  rdfs:domain cim:PerLengthSequenceImpedance ;
  rdfs:isDefinedBy :Package_Standard ;
  rdfs:range cim:ReactancePerLength ;
  uml:hasStereotype uml:attribute ;
  uml:id "EAID_31976830_1AA2_4fdb_9D0C_4AD1FB1355E9" .

cim:PerLengthSequenceImpedance.x0 a owl:ObjectProperty, owl:DatatypeProperty, owl:FunctionalProperty ;
  rdfs:label "x0" ;
  rdfs:comment "Zero sequence series reactance, per unit of length."@en ;
  rdfs:domain cim:PerLengthSequenceImpedance ;
  rdfs:isDefinedBy :Package_Standard ;
  rdfs:range cim:ReactancePerLength ;
  uml:hasStereotype uml:attribute ;
  uml:id "EAID_43CB9D7B_35BF_4c59_804A_9B64B6FD13F8" .

cim:PhaseImpedanceData.PhaseImpedance a owl:ObjectProperty, owl:FunctionalProperty ;
  rdfs:label "PhaseImpedance" ;
  rdfs:comment "Conductor phase impedance to which this data belongs."@en ;
  owl:inverseOf cim:PerLengthPhaseImpedance.PhaseImpedanceData ;
  rdfs:domain cim:PhaseImpedanceData ;
  rdfs:isDefinedBy :Package_Standard ;
  rdfs:range cim:PerLengthPhaseImpedance ;
  uml:id "EAID_918A88CD_E0A4_4abb_A371_853D33F0CA98-A" .

cim:PhaseImpedanceData.b a owl:ObjectProperty, owl:DatatypeProperty, owl:FunctionalProperty ;
  rdfs:label "b" ;
  rdfs:comment "Susceptance matrix element value, per length of unit."@en ;
  rdfs:domain cim:PhaseImpedanceData ;
  rdfs:isDefinedBy :Package_Standard ;
  rdfs:range cim:SusceptancePerLength ;
  uml:hasStereotype uml:attribute ;
  uml:id "EAID_93BDDE71_8D80_4a96_871D_CDD17E8F9C67" .

cim:PhaseImpedanceData.fromPhase a owl:ObjectProperty, owl:FunctionalProperty ;
  rdfs:label "fromPhase" ;
  rdfs:comment "Refer to the class description."@en ;
  rdfs:domain cim:PhaseImpedanceData ;
  rdfs:isDefinedBy :Package_Standard ;
  rdfs:range cim:SinglePhaseKind ;
  uml:hasStereotype uml:attribute ;
  uml:id "EAID_5AEB6B27_2AF8_404d_871C_260A76428503" .

cim:PhaseImpedanceData.g a owl:ObjectProperty, owl:DatatypeProperty, owl:FunctionalProperty ;
  rdfs:label "g" ;
  rdfs:comment "Conductance matrix element value, per length of unit."@en ;
  rdfs:domain cim:PhaseImpedanceData ;
  rdfs:isDefinedBy :Package_Standard ;
  rdfs:range cim:ConductancePerLength ;
  uml:hasStereotype uml:attribute ;
  uml:id "EAID_422A0F0A_C078_471a_BC18_3A7CC033ACAB" .

cim:PhaseImpedanceData.r a owl:ObjectProperty, owl:DatatypeProperty, owl:FunctionalProperty ;
  rdfs:label "r" ;
  rdfs:comment "Resistance matrix element value, per length of unit."@en ;
  rdfs:domain cim:PhaseImpedanceData ;
  rdfs:isDefinedBy :Package_Standard ;
  rdfs:range cim:ResistancePerLength ;
  uml:hasStereotype uml:attribute ;
  uml:id "EAID_989CB9D5_8FEC_4ab0_8698_7CB4D45183F6" .

cim:PhaseImpedanceData.toPhase a owl:ObjectProperty, owl:FunctionalProperty ;
  rdfs:label "toPhase" ;
  rdfs:comment "Refer to the class description."@en ;
  rdfs:domain cim:PhaseImpedanceData ;
  rdfs:isDefinedBy :Package_Standard ;
  rdfs:range cim:SinglePhaseKind ;
  uml:hasStereotype uml:attribute ;
  uml:id "EAID_E831AB7A_1AD3_4b93_B207_AE38ABC8E10E" .

cim:PhaseImpedanceData.x a owl:ObjectProperty, owl:DatatypeProperty, owl:FunctionalProperty ;
  rdfs:label "x" ;
  rdfs:comment "Reactance matrix element value, per length of unit."@en ;
  rdfs:domain cim:PhaseImpedanceData ;
  rdfs:isDefinedBy :Package_Standard ;
  rdfs:range cim:ReactancePerLength ;
  uml:hasStereotype uml:attribute ;
  uml:id "EAID_A99E11BB_AAA8_45b8_8C1E_3A12A6C39999" .

cim:PowerTransformerInfo.TransformerTankInfos a owl:ObjectProperty, owl:InverseFunctionalProperty ;
  rdfs:label "TransformerTankInfos" ;
  rdfs:comment "Data for all the tanks described by this power transformer data."@en ;
  owl:inverseOf cim:TransformerTankInfo.PowerTransformerInfo ;
  rdfs:domain cim:PowerTransformerInfo ;
  rdfs:isDefinedBy :Package_Standard ;
  rdfs:range cim:TransformerTankInfo ;
  uml:id "EAID_C277C451_16BA_451f_8357_29ACD116F6FA-B" .

cim:ProductAssetModel.AssetInfo a owl:ObjectProperty, owl:FunctionalProperty, owl:InverseFunctionalProperty ;
  rdfs:label "AssetInfo" ;
  owl:inverseOf cim:AssetInfo.ProductAssetModel ;
  rdfs:domain cim:ProductAssetModel ;
  rdfs:isDefinedBy :Package_Standard ;
  rdfs:range cim:AssetInfo ;
  uml:id "EAID_CCB697D1_E4FE_424f_8CCF_56E8AF800314-A" .

cim:ProductAssetModel.Manufacturer a owl:ObjectProperty, owl:FunctionalProperty ;
  rdfs:label "Manufacturer" ;
  rdfs:comment "Manufacturer of this asset model."@en ;
  owl:inverseOf cim:Manufacturer.ProductAssetModel ;
  rdfs:domain cim:ProductAssetModel ;
  rdfs:isDefinedBy :Package_Standard ;
  rdfs:range cim:Manufacturer ;
  uml:id "EAID_9413325B_DAA3_4fea_A516_89BBF10173DF-A" .

cim:ProductAssetModel.usageKind a owl:ObjectProperty, owl:FunctionalProperty ;
  rdfs:label "usageKind" ;
  rdfs:comment "Intended usage for this asset model."@en ;
  rdfs:domain cim:ProductAssetModel ;
  rdfs:isDefinedBy :Package_Standard ;
  rdfs:range cim:AssetModelUsageKind ;
  uml:hasStereotype uml:attribute ;
  uml:id "EAID_E6EFD948_8862_49e7_8839_D499DFE57DA7" .

cim:ShortCircuitTest.EnergisedEnd a owl:ObjectProperty, owl:FunctionalProperty ;
  rdfs:label "EnergisedEnd" ;
  rdfs:comment "Transformer end that voltage is applied to in this short-circuit test. The test voltage is chosen to induce rated current in the energised end."@en ;
  rdfs:domain cim:ShortCircuitTest ;
  rdfs:isDefinedBy :Package_Standard ;
  rdfs:range cim:TransformerEndInfo ;
  uml:id "EAID_F4CC6936_487F_4f4d_8120_368DE1C89C5A-A" .

cim:ShortCircuitTest.GroundedEnds a owl:ObjectProperty ;
  rdfs:label "GroundedEnds" ;
  rdfs:comment "All ends short-circuited in this short-circuit test."@en ;
  rdfs:domain cim:ShortCircuitTest ;
  rdfs:isDefinedBy :Package_Standard ;
  rdfs:range cim:TransformerEndInfo ;
  uml:id "EAID_0CA30326_4F64_4c91_BA06_69480DD1C0F0-A" .

cim:ShortCircuitTest.loss a owl:ObjectProperty, owl:DatatypeProperty, owl:FunctionalProperty ;
  rdfs:label "loss" ;
  rdfs:comment "Load losses from a positive-sequence or single-phase short-circuit test."@en ;
  rdfs:domain cim:ShortCircuitTest ;
  rdfs:isDefinedBy :Package_Standard ;
  rdfs:range cim:KiloActivePower ;
  uml:hasStereotype uml:attribute ;
  uml:id "EAID_8B8CB54A_C059_46c0_AE7F_7FDD39807AA1" .

cim:ShuntCompensatorInfo.ratedReactivePower a owl:ObjectProperty, owl:DatatypeProperty, owl:FunctionalProperty ;
  rdfs:label "ratedReactivePower" ;
  rdfs:comment "Rated reactive power."@en ;
  rdfs:domain cim:ShuntCompensatorInfo ;
  rdfs:isDefinedBy :Package_Standard ;
  rdfs:range cim:ReactivePower ;
  uml:hasStereotype uml:attribute ;
  uml:id "EAID_D0513C8E_4C8F_484b_8474_14FB37BE0BB5" .

cim:ShuntCompensatorInfo.ratedVoltage a owl:ObjectProperty, owl:DatatypeProperty, owl:FunctionalProperty ;
  rdfs:label "ratedVoltage" ;
  rdfs:comment "Rated voltage."@en ;
  rdfs:domain cim:ShuntCompensatorInfo ;
  rdfs:isDefinedBy :Package_Standard ;
  rdfs:range cim:Voltage ;
  uml:hasStereotype uml:attribute ;
  uml:id "EAID_18A7154A_6D7B_42c3_A489_62E4955C8691" .

cim:StreetAddress.streetDetail a owl:ObjectProperty, owl:FunctionalProperty ;
  rdfs:label "streetDetail" ;
  rdfs:comment "Street detail."@en ;
  rdfs:domain cim:StreetAddress ;
  rdfs:isDefinedBy :Package_CompoundTypes ;
  rdfs:range cim:StreetDetail ;
  uml:hasStereotype uml:attribute ;
  uml:id "EAID_FE7C53E0_21C7_42cd_82C0_B199179621BD" .

cim:StreetAddress.townDetail a owl:ObjectProperty, owl:FunctionalProperty ;
  rdfs:label "townDetail" ;
  rdfs:comment "Town detail."@en ;
  rdfs:domain cim:StreetAddress ;
  rdfs:isDefinedBy :Package_CompoundTypes ;
  rdfs:range cim:TownDetail ;
  uml:hasStereotype uml:attribute ;
  uml:id "EAID_3EA71AA6_ED5C_4f67_BCA2_3A6FB26C45AA" .

cim:SwitchInfo.breakingCapacity a owl:ObjectProperty, owl:DatatypeProperty, owl:FunctionalProperty ;
  rdfs:label "breakingCapacity" ;
  rdfs:comment "The maximum fault current a breaking device can break safely under prescribed conditions of use."@en ;
  rdfs:domain cim:SwitchInfo ;
  rdfs:isDefinedBy :Package_Standard ;
  rdfs:range cim:CurrentFlow ;
  uml:hasStereotype uml:attribute ;
  uml:id "EAID_021BF3BF_5E65_4acf_8993_94608A9B3F48" .

cim:SwitchInfo.ratedCurrent a owl:ObjectProperty, owl:DatatypeProperty, owl:FunctionalProperty ;
  rdfs:label "ratedCurrent" ;
  rdfs:comment "Rated current."@en ;
  rdfs:domain cim:SwitchInfo ;
  rdfs:isDefinedBy :Package_Standard ;
  rdfs:range cim:CurrentFlow ;
  uml:hasStereotype uml:attribute ;
  uml:id "EAID_0E3D0A4C_27B8_47a9_B4B9_828CA5C7E979" .

cim:SwitchInfo.ratedVoltage a owl:ObjectProperty, owl:DatatypeProperty, owl:FunctionalProperty ;
  rdfs:label "ratedVoltage" ;
  rdfs:comment "Rated voltage."@en ;
  rdfs:domain cim:SwitchInfo ;
  rdfs:isDefinedBy :Package_Standard ;
  rdfs:range cim:Voltage ;
  uml:hasStereotype uml:attribute ;
  uml:id "EAID_D93D2EF1_F7B6_44df_9878_104B915FA5E5" .

cim:TapChangerInfo.neutralU a owl:ObjectProperty, owl:DatatypeProperty, owl:FunctionalProperty ;
  rdfs:label "neutralU" ;
  rdfs:comment "Voltage at which the winding operates at the neutral tap setting."@en ;
  rdfs:domain cim:TapChangerInfo ;
  rdfs:isDefinedBy :Package_Standard ;
  rdfs:range cim:Voltage ;
  uml:hasStereotype uml:attribute ;
  uml:id "EAID_C46776FB_4B12_4339_A572_40F74B9FC2B1" .

cim:TapChangerInfo.ratedVoltage a owl:ObjectProperty, owl:DatatypeProperty, owl:FunctionalProperty ;
  rdfs:label "ratedVoltage" ;
  rdfs:comment "Rated voltage."@en ;
  rdfs:domain cim:TapChangerInfo ;
  rdfs:isDefinedBy :Package_Standard ;
  rdfs:range cim:Voltage ;
  uml:hasStereotype uml:attribute ;
  uml:id "EAID_C0D85BFE_8ECE_449a_8689_255E212C433D" .

cim:TapChangerInfo.stepVoltageIncrement a owl:ObjectProperty, owl:DatatypeProperty, owl:FunctionalProperty ;
  rdfs:label "stepVoltageIncrement" ;
  rdfs:comment "Tap step increment, in per cent of rated voltage, per step position."@en ;
  rdfs:domain cim:TapChangerInfo ;
  rdfs:isDefinedBy :Package_Standard ;
  rdfs:range cim:PerCent ;
  uml:hasStereotype uml:attribute ;
  uml:id "EAID_2B051AF4_DD1E_4d4e_ADA9_528FA2439004" .

cim:TransformerEndInfo.EnergisedEndNoLoadTest a owl:ObjectProperty, owl:InverseFunctionalProperty ;
  rdfs:label "EnergisedEndNoLoadTest" ;
  rdfs:comment "All no-load test measurements in which this transformer end was energised."@en ;
  owl:inverseOf cim:NoLoadTest.EnergisedEnd ;
  rdfs:domain cim:TransformerEndInfo ;
  rdfs:isDefinedBy :Package_Standard ;
  rdfs:range cim:NoLoadTest ;
  uml:id "EAID_D9249600_6545_48c5_BB01_F3AC06385B23-B" .

cim:TransformerEndInfo.TransformerTankInfo a owl:ObjectProperty, owl:FunctionalProperty ;
  rdfs:label "TransformerTankInfo" ;
  rdfs:comment "Transformer tank data that this end description is part of."@en ;
  owl:inverseOf cim:TransformerTankInfo.TransformerEndInfos ;
  rdfs:domain cim:TransformerEndInfo ;
  rdfs:isDefinedBy :Package_Standard ;
  rdfs:range cim:TransformerTankInfo ;
  uml:id "EAID_01B0907C_7429_4ad1_A4AC_32AA17C81164-A" .

cim:TransformerEndInfo.connectionKind a owl:ObjectProperty, owl:FunctionalProperty ;
  rdfs:label "connectionKind" ;
  rdfs:comment "Kind of connection."@en ;
  rdfs:domain cim:TransformerEndInfo ;
  rdfs:isDefinedBy :Package_Standard ;
  rdfs:range cim:WindingConnection ;
  uml:hasStereotype uml:attribute ;
  uml:id "EAID_F5D39242_6C65_4151_805C_28BA230569F1" .

cim:TransformerEndInfo.r a owl:ObjectProperty, owl:DatatypeProperty, owl:FunctionalProperty ;
  rdfs:label "r" ;
  rdfs:comment "DC resistance."@en ;
  rdfs:domain cim:TransformerEndInfo ;
  rdfs:isDefinedBy :Package_Standard ;
  rdfs:range cim:Resistance ;
  uml:hasStereotype uml:attribute ;
  uml:id "EAID_DB7EC136_7215_4b74_AD30_5C67AB6DEFF8" .

cim:TransformerEndInfo.ratedS a owl:ObjectProperty, owl:DatatypeProperty, owl:FunctionalProperty ;
  rdfs:label "ratedS" ;
  rdfs:comment "Normal apparent power rating."@en ;
  rdfs:domain cim:TransformerEndInfo ;
  rdfs:isDefinedBy :Package_Standard ;
  rdfs:range cim:ApparentPower ;
  uml:hasStereotype uml:attribute ;
  uml:id "EAID_B0C2308F_7D8D_4042_AD56_76C943CDF8A4" .

cim:TransformerEndInfo.ratedU a owl:ObjectProperty, owl:DatatypeProperty, owl:FunctionalProperty ;
  rdfs:label "ratedU" ;
  rdfs:comment "Rated voltage: phase-phase for three-phase windings, and either phase-phase or phase-neutral for single-phase windings."@en ;
  rdfs:domain cim:TransformerEndInfo ;
  rdfs:isDefinedBy :Package_Standard ;
  rdfs:range cim:Voltage ;
  uml:hasStereotype uml:attribute ;
  uml:id "EAID_615FE2AB_C13E_41eb_B1C1_D07CD9AE256A" .

cim:TransformerTankInfo.PowerTransformerInfo a owl:ObjectProperty, owl:FunctionalProperty ;
  rdfs:label "PowerTransformerInfo" ;
  rdfs:comment "Power transformer data that this tank description is part of."@en ;
  owl:inverseOf cim:PowerTransformerInfo.TransformerTankInfos ;
  rdfs:domain cim:TransformerTankInfo ;
  rdfs:isDefinedBy :Package_Standard ;
  rdfs:range cim:PowerTransformerInfo ;
  uml:id "EAID_C277C451_16BA_451f_8357_29ACD116F6FA-A" .

cim:TransformerTankInfo.TransformerEndInfos a owl:ObjectProperty, owl:InverseFunctionalProperty ;
  rdfs:label "TransformerEndInfos" ;
  rdfs:comment "Data for all the ends described by this transformer tank data."@en ;
  owl:inverseOf cim:TransformerEndInfo.TransformerTankInfo ;
  rdfs:domain cim:TransformerTankInfo ;
  rdfs:isDefinedBy :Package_Standard ;
  rdfs:range cim:TransformerEndInfo ;
  uml:id "EAID_01B0907C_7429_4ad1_A4AC_32AA17C81164-B" .

cim:TransformerTest.basePower a owl:ObjectProperty, owl:DatatypeProperty, owl:FunctionalProperty ;
  rdfs:label "basePower" ;
  rdfs:comment "Base power at which the tests are conducted, usually equal to the rateds of one of the involved transformer ends."@en ;
  rdfs:domain cim:TransformerTest ;
  rdfs:isDefinedBy :Package_Standard ;
  rdfs:range cim:ApparentPower ;
  uml:hasStereotype uml:attribute ;
  uml:id "EAID_C1517EB5_B868_4ae5_A410_5EEBE2756D97" .

cim:WireAssemblyInfo.PerLengthLineParameter a owl:ObjectProperty, owl:InverseFunctionalProperty ;
  rdfs:label "PerLengthLineParameter" ;
  rdfs:comment "A WireAssemblyInfo is used to compute the PerLengthParameter data in the Wires package"@en ;
  owl:inverseOf cim:PerLengthLineParameter.WireAssemblyInfo ;
  rdfs:domain cim:WireAssemblyInfo ;
  rdfs:isDefinedBy :Package_Standard ;
  rdfs:range cim:PerLengthLineParameter ;
  uml:id "EAID_98CE9D77_13DF_4983_93BD_7E438547A4BE-A" .

cim:WireAssemblyInfo.WirePhaseInfo a owl:ObjectProperty, owl:InverseFunctionalProperty ;
  rdfs:label "WirePhaseInfo" ;
  owl:inverseOf cim:WirePhaseInfo.WireAssemblyInfo ;
  rdfs:domain cim:WireAssemblyInfo ;
  rdfs:isDefinedBy :Package_Standard ;
  rdfs:range cim:WirePhaseInfo ;
  uml:id "EAID_7CA6758B_7DAB_46c5_87C3_10AFEABC60A1-A" .

cim:WireInfo.WirePhaseInfo a owl:ObjectProperty, owl:InverseFunctionalProperty ;
  rdfs:label "WirePhaseInfo" ;
  owl:inverseOf cim:WirePhaseInfo.WireInfo ;
  rdfs:domain cim:WireInfo ;
  rdfs:isDefinedBy :Package_Standard ;
  rdfs:range cim:WirePhaseInfo ;
  uml:id "EAID_CFE876A4_DF6A_4c0e_B278_E09296D58CF8-B" .

cim:WireInfo.insulationMaterial a owl:ObjectProperty, owl:FunctionalProperty ;
  rdfs:label "insulationMaterial" ;
  rdfs:comment "(if insulated conductor) Material used for insulation."@en ;
  rdfs:domain cim:WireInfo ;
  rdfs:isDefinedBy :Package_Standard ;
  rdfs:range cim:WireInsulationKind ;
  uml:hasStereotype uml:attribute ;
  uml:id "EAID_3FE372EC_1C5A_49c1_9F89_A11284254BA5" .

cim:WireInfo.material a owl:ObjectProperty, owl:FunctionalProperty ;
  rdfs:label "material" ;
  rdfs:comment "Conductor material."@en ;
  rdfs:domain cim:WireInfo ;
  rdfs:isDefinedBy :Package_Standard ;
  rdfs:range cim:WireMaterialKind ;
  uml:hasStereotype uml:attribute ;
  uml:id "EAID_986B1BF1_2CEE_4bcb_B91C_BDF900B68364" .

cim:WireInfo.radius a owl:ObjectProperty, owl:DatatypeProperty, owl:FunctionalProperty ;
  rdfs:label "radius" ;
  rdfs:comment "Outside radius of the wire."@en ;
  rdfs:domain cim:WireInfo ;
  rdfs:isDefinedBy :Package_Standard ;
  rdfs:range cim:Length ;
  uml:hasStereotype uml:attribute ;
  uml:id "EAID_B7D8C060_1737_41ac_BACB_39404B5411FB" .

cim:WireInfo.ratedCurrent a owl:ObjectProperty, owl:DatatypeProperty, owl:FunctionalProperty ;
  rdfs:label "ratedCurrent" ;
  rdfs:comment "Current carrying capacity of the wire under stated thermal conditions."@en ;
  rdfs:domain cim:WireInfo ;
  rdfs:isDefinedBy :Package_Standard ;
  rdfs:range cim:CurrentFlow ;
  uml:hasStereotype uml:attribute ;
  uml:id "EAID_5C1F3562_D4C6_433c_B8EA_058A604A0513" .

cim:WirePhaseInfo.WireAssemblyInfo a owl:ObjectProperty, owl:FunctionalProperty ;
  rdfs:label "WireAssemblyInfo" ;
  owl:inverseOf cim:WireAssemblyInfo.WirePhaseInfo ;
  rdfs:domain cim:WirePhaseInfo ;
  rdfs:isDefinedBy :Package_Standard ;
  rdfs:range cim:WireAssemblyInfo ;
  uml:id "EAID_7CA6758B_7DAB_46c5_87C3_10AFEABC60A1-B" .

cim:WirePhaseInfo.WireInfo a owl:ObjectProperty, owl:FunctionalProperty ;
  rdfs:label "WireInfo" ;
  owl:inverseOf cim:WireInfo.WirePhaseInfo ;
  rdfs:domain cim:WirePhaseInfo ;
  rdfs:isDefinedBy :Package_Standard ;
  rdfs:range cim:WireInfo ;
  uml:id "EAID_CFE876A4_DF6A_4c0e_B278_E09296D58CF8-A" .

cim:WirePhaseInfo.WirePosition a owl:ObjectProperty, owl:FunctionalProperty ;
  rdfs:label "WirePosition" ;
  owl:inverseOf cim:WirePosition.WirePhaseInfo ;
  rdfs:domain cim:WirePhaseInfo ;
  rdfs:isDefinedBy :Package_Standard ;
  rdfs:range cim:WirePosition ;
  uml:id "EAID_EF1B8B6A_6D78_43c1_818B_8F70517C4849-A" .

cim:WirePhaseInfo.phaseInfo a owl:ObjectProperty, owl:FunctionalProperty ;
  rdfs:label "phaseInfo" ;
  rdfs:domain cim:WirePhaseInfo ;
  rdfs:isDefinedBy :Package_Standard ;
  rdfs:range cim:SinglePhaseKind ;
  uml:hasStereotype uml:attribute ;
  uml:id "EAID_5F6C386A_55B1_45e6_8155_CF2D5B9F2C10" .

cim:WirePosition.WirePhaseInfo a owl:ObjectProperty, owl:InverseFunctionalProperty ;
  rdfs:label "WirePhaseInfo" ;
  owl:inverseOf cim:WirePhaseInfo.WirePosition ;
  rdfs:domain cim:WirePosition ;
  rdfs:isDefinedBy :Package_Standard ;
  rdfs:range cim:WirePhaseInfo ;
  uml:id "EAID_EF1B8B6A_6D78_43c1_818B_8F70517C4849-B" .

cim:WirePosition.WireSpacingInfo a owl:ObjectProperty, owl:FunctionalProperty ;
  rdfs:label "WireSpacingInfo" ;
  rdfs:comment "Wire spacing data this wire position belongs to."@en ;
  owl:inverseOf cim:WireSpacing.WirePosition ;
  rdfs:domain cim:WirePosition ;
  rdfs:isDefinedBy :Package_Standard ;
  rdfs:range cim:WireSpacing ;
  uml:id "EAID_56D78854_A2BC_4502_8273_C1C1208A55F3-A" .

cim:WirePosition.xCoord a owl:ObjectProperty, owl:DatatypeProperty, owl:FunctionalProperty ;
  rdfs:label "xCoord" ;
  rdfs:comment "Signed horizontal distance from the wire at this position to a common reference point."@en ;
  rdfs:domain cim:WirePosition ;
  rdfs:isDefinedBy :Package_Standard ;
  rdfs:range cim:Displacement ;
  uml:hasStereotype uml:attribute ;
  uml:id "EAID_9A48273A_E3AB_4fc0_98FE_079E588FE89E" .

cim:WirePosition.yCoord a owl:ObjectProperty, owl:DatatypeProperty, owl:FunctionalProperty ;
  rdfs:label "yCoord" ;
  rdfs:comment "Signed vertical distance from the wire at this position: above ground (positive value) or burial depth below ground (negative value)."@en ;
  rdfs:domain cim:WirePosition ;
  rdfs:isDefinedBy :Package_Standard ;
  rdfs:range cim:Displacement ;
  uml:hasStereotype uml:attribute ;
  uml:id "EAID_3F994542_429C_48ba_B978_7D3641E12E9C" .

cim:WireSpacing.WirePosition a owl:ObjectProperty, owl:InverseFunctionalProperty ;
  rdfs:label "WirePosition" ;
  rdfs:comment "All positions of single wires (phase or neutral) making the conductor."@en ;
  owl:inverseOf cim:WirePosition.WireSpacingInfo ;
  rdfs:domain cim:WireSpacing ;
  rdfs:isDefinedBy :Package_Standard ;
  rdfs:range cim:WirePosition ;
  uml:id "EAID_56D78854_A2BC_4502_8273_C1C1208A55F3-B" .

cim:WireSpacing.phaseWireSpacing a owl:ObjectProperty, owl:DatatypeProperty, owl:FunctionalProperty ;
  rdfs:label "phaseWireSpacing" ;
  rdfs:comment "Distance between wire sub-conductors in a symmetrical bundle."@en ;
  rdfs:domain cim:WireSpacing ;
  rdfs:isDefinedBy :Package_Standard ;
  rdfs:range cim:Length ;
  uml:hasStereotype uml:attribute ;
  uml:id "EAID_A200C8F2_6675_422b_B94B_14AE950272FD" .

cim:WireSpacing.usage a owl:ObjectProperty, owl:FunctionalProperty ;
  rdfs:label "usage" ;
  rdfs:domain cim:WireSpacing ;
  rdfs:isDefinedBy :Package_Standard ;
  rdfs:range cim:WireUsageKind ;
  uml:hasStereotype uml:attribute ;
  uml:id "EAID_43C13EF5_5580_4d03_8D6A_E31336FF9DF0" .

md:DifferenceModel.forwardDifferences a owl:ObjectProperty, owl:FunctionalProperty ;
  rdfs:label "forwardDifferences" ;
  rdfs:domain md:DifferenceModel ;
  rdfs:isDefinedBy :Package_ModelDescription ;
  rdfs:range md:Statements ;
  uml:id "EAID_4F33C8FB_FF1D_42aa_918E_407C825CC412-B" .

md:DifferenceModel.reverseDifferences a owl:ObjectProperty, owl:FunctionalProperty ;
  rdfs:label "reverseDifferences" ;
  rdfs:domain md:DifferenceModel ;
  rdfs:isDefinedBy :Package_ModelDescription ;
  rdfs:range md:Statements ;
  uml:id "EAID_84439CAF_AF31_4da5_9D0F_EA6311EF9054-B" .

md:Model.DependentOn a owl:ObjectProperty ;
  rdfs:label "DependentOn" ;
  owl:inverseOf md:Model.Depending ;
  rdfs:domain md:Model ;
  rdfs:isDefinedBy :Package_ModelDescription ;
  rdfs:range md:Model ;
  uml:id "EAID_151476FC_7E20_41d2_AE3F_224B91D88006-B" .

md:Model.Depending a owl:ObjectProperty ;
  rdfs:label "Depending" ;
  owl:inverseOf md:Model.DependentOn ;
  rdfs:domain md:Model ;
  rdfs:isDefinedBy :Package_ModelDescription ;
  rdfs:range md:Model ;
  uml:id "EAID_151476FC_7E20_41d2_AE3F_224B91D88006-A" .

md:Model.SupersededBy a owl:ObjectProperty ;
  rdfs:label "SupersededBy" ;
  owl:inverseOf md:Model.Supersedes ;
  rdfs:domain md:Model ;
  rdfs:isDefinedBy :Package_ModelDescription ;
  rdfs:range md:Model ;
  uml:id "EAID_DDBEB57C_03E6_4aab_B8A4_E5A2E2C2E3CF-A" .

md:Model.Supersedes a owl:ObjectProperty ;
  rdfs:label "Supersedes" ;
  owl:inverseOf md:Model.SupersededBy ;
  rdfs:domain md:Model ;
  rdfs:isDefinedBy :Package_ModelDescription ;
  rdfs:range md:Model ;
  uml:id "EAID_DDBEB57C_03E6_4aab_B8A4_E5A2E2C2E3CF-B" .

md:Model.modelingAuthoritySet a owl:ObjectProperty, owl:DatatypeProperty, owl:FunctionalProperty ;
  rdfs:label "modelingAuthoritySet" ;
  rdfs:domain md:Model ;
  rdfs:isDefinedBy :Package_ModelDescription ;
  rdfs:range :URI ;
  uml:hasStereotype uml:attribute ;
  uml:id "EAID_933B0F39_959D_4fe4_B6EF_D25BF8CDA8CC" .

md:Model.profile a owl:ObjectProperty, owl:DatatypeProperty, owl:FunctionalProperty ;
  rdfs:label "profile" ;
  rdfs:domain md:Model ;
  rdfs:isDefinedBy :Package_ModelDescription ;
  rdfs:range :URI ;
  uml:hasStereotype uml:attribute ;
  uml:id "EAID_5FC10413_4CB8_4041_A5C5_39DBCE569A80" .

next2:Organisation.RolesEx a owl:ObjectProperty, owl:InverseFunctionalProperty ;
  rdfs:label "Roles" ;
  rdfs:comment "All roles of this organisation."@en ;
  owl:inverseOf next2:OrganisationRoleEx.Organisation ;
  rdfs:domain cim:Organisation ;
  rdfs:isDefinedBy :Package_CIMExtensions ;
  rdfs:range next2:OrganisationRoleEx ;
  uml:id "EAID_5276F20A_6106_4add_AFF5_435E575B8751-B" .

next2:OrganisationRoleEx.Organisation a owl:ObjectProperty, owl:FunctionalProperty ;
  rdfs:label "Organisation" ;
  rdfs:comment "Organisation having this role."@en ;
  owl:inverseOf next2:Organisation.RolesEx ;
  rdfs:domain next2:OrganisationRoleEx ;
  rdfs:isDefinedBy :Package_CIMExtensions ;
  rdfs:range cim:Organisation ;
  uml:id "EAID_5276F20A_6106_4add_AFF5_435E575B8751-A" .

next3:CatalogAssetType.TypeAssetCatalogue a owl:ObjectProperty, owl:FunctionalProperty ;
  rdfs:label "TypeAssetCatalogue" ;
  owl:inverseOf next3:TypeAssetCatalogue.TypeAssets ;
  rdfs:domain cim:CatalogAssetType ;
  rdfs:isDefinedBy :Package_InfIEC61968 ;
  rdfs:range next3:TypeAssetCatalogue ;
  uml:id "EAID_A591ED48_AB76_461f_92B6_DBF7738B306D-B" .

next3:ShuntCompensatorControl.ShuntCompensatorInfo a owl:ObjectProperty, owl:FunctionalProperty, owl:InverseFunctionalProperty ;
  rdfs:label "ShuntCompensatorInfo" ;
  owl:inverseOf next3:ShuntCompensatorInfo.ShuntCompensatorControl ;
  rdfs:domain next3:ShuntCompensatorControl ;
  rdfs:isDefinedBy :Package_InfIEC61968 ;
  rdfs:range cim:ShuntCompensatorInfo ;
  uml:id "EAID_7241F032_F58B_4c83_9506_5A1E11436B82-B" .

next3:ShuntCompensatorControl.cellSize a owl:ObjectProperty, owl:DatatypeProperty, owl:FunctionalProperty ;
  rdfs:label "cellSize" ;
  rdfs:comment "The size of the individual units that make up the bank."@en ;
  rdfs:domain next3:ShuntCompensatorControl ;
  rdfs:isDefinedBy :Package_InfIEC61968 ;
  rdfs:range cim:ReactivePower ;
  uml:hasStereotype uml:attribute ;
  uml:id "EAID_50481FCE_1EE9_477a_932E_2FD188AC1E24" .

next3:ShuntCompensatorInfo.ShuntCompensatorControl a owl:ObjectProperty, owl:FunctionalProperty, owl:InverseFunctionalProperty ;
  rdfs:label "ShuntCompensatorControl" ;
  owl:inverseOf next3:ShuntCompensatorControl.ShuntCompensatorInfo ;
  rdfs:domain cim:ShuntCompensatorInfo ;
  rdfs:isDefinedBy :Package_InfIEC61968 ;
  rdfs:range next3:ShuntCompensatorControl ;
  uml:id "EAID_7241F032_F58B_4c83_9506_5A1E11436B82-A" .

next3:TypeAssetCatalogue.TypeAssets a owl:ObjectProperty, owl:InverseFunctionalProperty ;
  rdfs:label "TypeAssets" ;
  owl:inverseOf next3:CatalogAssetType.TypeAssetCatalogue ;
  rdfs:domain next3:TypeAssetCatalogue ;
  rdfs:isDefinedBy :Package_InfIEC61968 ;
  rdfs:range cim:CatalogAssetType ;
  uml:id "EAID_A591ED48_AB76_461f_92B6_DBF7738B306D-A" .

next:WireInfoEx.ratedVoltage a owl:ObjectProperty, owl:DatatypeProperty, owl:FunctionalProperty ;
  rdfs:label "ratedVoltage" ;
  rdfs:domain next:WireInfoEx ;
  rdfs:isDefinedBy :Package_EDFExtensions ;
  rdfs:range cim:Voltage ;
  uml:hasStereotype uml:attribute ;
  uml:id "EAID_C3CD4E8C_BF29_4b94_83F9_AE2AF65C168A" .

:PowerSystemProjectSchedule.actualEnd a owl:DatatypeProperty, owl:FunctionalProperty ;
  rdfs:label "actualEnd" ;
  rdfs:comment "Actual date and time for when the project is commissioned and committed to the network model."@en ;
  rdfs:domain :PowerSystemProjectSchedule ;
  rdfs:isDefinedBy :Package_PowerSystemProject ;
  rdfs:range xsd:dateTime ;
  uml:hasStereotype uml:attribute ;
  uml:id "EAID_33C0A687_BB3C_4e0b_B2B3_82D4C137641B" .

:PowerSystemProjectSchedule.actualStart a owl:DatatypeProperty, owl:FunctionalProperty ;
  rdfs:label "actualStart" ;
  rdfs:comment "Actual date and time for when the project is commissioned and committed to the network model."@en ;
  rdfs:domain :PowerSystemProjectSchedule ;
  rdfs:isDefinedBy :Package_PowerSystemProject ;
  rdfs:range xsd:dateTime ;
  uml:hasStereotype uml:attribute ;
  uml:id "EAID_4EDBCAA8_AF79_4b4c_B36A_B3003FC9689D" .

:PowerSystemProjectSchedule.scheduledEnd a owl:DatatypeProperty, owl:FunctionalProperty ;
  rdfs:label "scheduledEnd" ;
  rdfs:comment "Estimated date and time for when the project will be commissioned and committed to the network model."@en ;
  rdfs:domain :PowerSystemProjectSchedule ;
  rdfs:isDefinedBy :Package_PowerSystemProject ;
  rdfs:range xsd:dateTime ;
  uml:hasStereotype uml:attribute ;
  uml:id "EAID_62039392_12EC_47c9_AC63_22F9A0CEA639" .

:PowerSystemProjectSchedule.scheduledStart a owl:DatatypeProperty, owl:FunctionalProperty ;
  rdfs:label "scheduledStart" ;
  rdfs:comment "Estimated date and time for when the project will be commissioned and committed to the network model."@en ;
  rdfs:domain :PowerSystemProjectSchedule ;
  rdfs:isDefinedBy :Package_PowerSystemProject ;
  rdfs:range xsd:dateTime ;
  uml:hasStereotype uml:attribute ;
  uml:id "EAID_60AFA573_DE21_4205_A33F_0FF74871E407" .

:ProjectStep.actualEnd a owl:DatatypeProperty, owl:FunctionalProperty ;
  rdfs:label "actualEnd" ;
  rdfs:comment "Actual date and time for when the project is commissioned and committed to the network model."@en ;
  rdfs:domain :ProjectStep ;
  rdfs:isDefinedBy :Package_PowerSystemProject ;
  rdfs:range xsd:dateTime ;
  uml:hasStereotype uml:attribute ;
  uml:id "EAID_EC8B0A80_0258_479a_9B0D_F35BBCFDE375" .

:ProjectStep.actualStart a owl:DatatypeProperty, owl:FunctionalProperty ;
  rdfs:label "actualStart" ;
  rdfs:comment "Actual date and time for when the project is commissioned and committed to the network model."@en ;
  rdfs:domain :ProjectStep ;
  rdfs:isDefinedBy :Package_PowerSystemProject ;
  rdfs:range xsd:dateTime ;
  uml:hasStereotype uml:attribute ;
  uml:id "EAID_DBF1A91C_4DE8_4424_A85C_B910C938A7C7" .

:ProjectStep.scheduledEnd a owl:DatatypeProperty, owl:FunctionalProperty ;
  rdfs:label "scheduledEnd" ;
  rdfs:comment "Estimated date and time for when the project will be commissioned and committed to the network model."@en ;
  rdfs:domain :ProjectStep ;
  rdfs:isDefinedBy :Package_PowerSystemProject ;
  rdfs:range xsd:dateTime ;
  uml:hasStereotype uml:attribute ;
  uml:id "EAID_F82A3F17_7783_4cde_8D47_EE8AF38A6BF6" .

:ProjectStep.scheduledStart a owl:DatatypeProperty, owl:FunctionalProperty ;
  rdfs:label "scheduledStart" ;
  rdfs:comment "Estimated date and time for when the project will be commissioned and committed to the network model."@en ;
  rdfs:domain :ProjectStep ;
  rdfs:isDefinedBy :Package_PowerSystemProject ;
  rdfs:range xsd:dateTime ;
  uml:hasStereotype uml:attribute ;
  uml:id "EAID_F7E1A2ED_891A_4649_9389_B2BA5C2B4AC9" .

cim:CDPSMVersion.baseIec61968 a owl:DatatypeProperty, owl:FunctionalProperty ;
  rdfs:label "baseIec61968" ;
  rdfs:comment "Base UML provided by CIM model manager, submodel 61968."@en ;
  rdfs:domain cim:CDPSMVersion ;
  rdfs:isDefinedBy :Package_Extensions ;
  rdfs:range xsd:string ;
  uml:hasInitialValue "iec61968cim13v09" ;
  uml:hasStereotype uml:attribute ;
  uml:id "EAID_1970E2C0_DACC_4a56_93E0_64EFD94A9EAE" .

cim:CDPSMVersion.baseIec61970 a owl:DatatypeProperty, owl:FunctionalProperty ;
  rdfs:label "baseIec61970" ;
  rdfs:comment "Base UML provided by CIM model manager, submodel 61970."@en ;
  rdfs:domain cim:CDPSMVersion ;
  rdfs:isDefinedBy :Package_Extensions ;
  rdfs:range xsd:string ;
  uml:hasInitialValue "iec61970cim17v19" ;
  uml:hasStereotype uml:attribute ;
  uml:id "EAID_A840C944_510F_46d8_8CFE_FEB825CA3494" .

cim:CDPSMVersion.baseURI a owl:DatatypeProperty, owl:FunctionalProperty ;
  rdfs:label "baseURI" ;
  rdfs:comment "Profile URI used in the Model Exchange header and defined in IEC standards.  It uniquely identifies the Profile and its version. It is given for information only and to identify the closest IEC profile to which this CGMES profile is based on."@en ;
  rdfs:domain cim:CDPSMVersion ;
  rdfs:isDefinedBy :Package_Extensions ;
  rdfs:range xsd:string ;
  uml:hasInitialValue "none" ;
  uml:hasStereotype uml:attribute ;
  uml:id "EAID_D8A307FA_4BAA_4f07_8F0A_8B5C3D86C6A1" .

cim:CDPSMVersion.date a owl:DatatypeProperty, owl:FunctionalProperty ;
  rdfs:label "date" ;
  rdfs:comment """Profile creation date
      Form is YYYY-MM-DD for example for January 5, 2009 it is 2009-01-05."""@en ;
  rdfs:domain cim:CDPSMVersion ;
  rdfs:isDefinedBy :Package_Extensions ;
  rdfs:range xsd:date ;
  uml:hasInitialValue "2017-05-15" ;
  uml:hasStereotype uml:attribute ;
  uml:id "EAID_DF772018_A2E0_4d6c_9BB4_C3E163783425" .

cim:CDPSMVersion.differenceModelURI a owl:DatatypeProperty, owl:FunctionalProperty ;
  rdfs:label "differenceModelURI" ;
  rdfs:comment "Difference model URI defined by IEC 61970-552."@en ;
  rdfs:domain cim:CDPSMVersion ;
  rdfs:isDefinedBy :Package_Extensions ;
  rdfs:range xsd:string ;
  uml:hasInitialValue "none" ;
  uml:hasStereotype uml:attribute ;
  uml:id "EAID_DB86C423_0254_438b_B485_F7737ED12D7A" .

cim:CDPSMVersion.namespaceRDF a owl:DatatypeProperty, owl:FunctionalProperty ;
  rdfs:label "namespaceRDF" ;
  rdfs:comment "RDF namespace."@en ;
  rdfs:domain cim:CDPSMVersion ;
  rdfs:isDefinedBy :Package_Extensions ;
  rdfs:range xsd:string ;
  uml:hasInitialValue "http://www.w3.org/1999/02/22-rdf-syntax-ns#" ;
  uml:hasStereotype uml:attribute ;
  uml:id "EAID_DFA95D2C_8997_4791_B719_FA6E6F31AEF5" .

cim:CDPSMVersion.namespace_CDPSM_UML a owl:DatatypeProperty, owl:FunctionalProperty ;
  rdfs:label "namespace_CDPSM_UML" ;
  rdfs:comment "UML extensions version (format cdpsm_vXX) (obsolete namespace)"@en ;
  rdfs:domain cim:CDPSMVersion ;
  rdfs:isDefinedBy :Package_Extensions ;
  rdfs:range xsd:string ;
  uml:hasInitialValue "http://edf.fr/CDPSM/2016/cdpsm2015#" ;
  uml:hasStereotype uml:attribute ;
  uml:id "EAID_56D65BBE_EB99_4585_8CAE_CC4B9BE0B5D5" .

cim:CDPSMVersion.namespace_CIMEXT_UML a owl:DatatypeProperty, owl:FunctionalProperty ;
  rdfs:label "namespace_CIMEXT_UML" ;
  rdfs:comment "namespace for components extensions to CIM, used in CDPSM (not defined in CIM but used by CDPSM should be added to CIM in a next release)"@en ;
  rdfs:domain cim:CDPSMVersion ;
  rdfs:isDefinedBy :Package_Extensions ;
  rdfs:range xsd:string ;
  uml:hasInitialValue "http://edf.fr/draft/cim17-ext#" ;
  uml:hasStereotype uml:attribute ;
  uml:id "EAID_A54C4F1D_4EA1_42d8_8986_CA3254221EA9" .

cim:CDPSMVersion.namespace_CIMINFO_UML a owl:DatatypeProperty, owl:FunctionalProperty ;
  rdfs:label "namespace_CIMINFO_UML" ;
  rdfs:comment "namespace for CIM informative components used in CDPSM (defined in CIM but not considered stabilized and noty part of the standard)"@en ;
  rdfs:domain cim:CDPSMVersion ;
  rdfs:isDefinedBy :Package_Extensions ;
  rdfs:range xsd:string ;
  uml:hasInitialValue "http://edf.fr/draft/cim17-info#" ;
  uml:hasStereotype uml:attribute ;
  uml:id "EAID_A454E13E_854C_4928_AF86_D20C5DE7912D" .

cim:CDPSMVersion.namespace_CIM_UML a owl:DatatypeProperty, owl:FunctionalProperty ;
  rdfs:label "namespace_CIM_UML" ;
  rdfs:comment "CIM UML namespace.  for elements considered as standard (not informative or extension)."@en ;
  rdfs:domain cim:CDPSMVersion ;
  rdfs:isDefinedBy :Package_Extensions ;
  rdfs:range xsd:string ;
  uml:hasInitialValue "https://cim.ucaiug.io/ns#" ;
  uml:hasStereotype uml:attribute ;
  uml:id "EAID_2431B278_EAB3_409d_8EDF_31CF3B06EBB6" .

cim:CDPSMVersion.namespace_EDFEXT_UML a owl:DatatypeProperty, owl:FunctionalProperty ;
  rdfs:label "namespace_EDFEXT_UML" ;
  rdfs:comment "namespace for components extensions to CIM, used in CDPSM (not defined in CIM but used by CDPSM should be added to CIM in a next release)"@en ;
  rdfs:domain cim:CDPSMVersion ;
  rdfs:isDefinedBy :Package_Extensions ;
  rdfs:range xsd:string ;
  uml:hasInitialValue "http://der.edf.fr/mire/MSite-v3.1.a#" ;
  uml:hasStereotype uml:attribute ;
  uml:id "EAID_71A33F21_3B47_40c5_B402_5759D2AD459C" .

cim:CDPSMVersion.namespace_ENTSOE_UML a owl:DatatypeProperty, owl:FunctionalProperty ;
  rdfs:label "namespace_ENTSOE_UML" ;
  rdfs:comment "namespace for components extensions to CIM, used in CGMES and CDPSM"@en ;
  rdfs:domain cim:CDPSMVersion ;
  rdfs:isDefinedBy :Package_Extensions ;
  rdfs:range xsd:string ;
  uml:hasInitialValue "http://entsoe.eu/CIM/SchemaExtension/3/1#" ;
  uml:hasStereotype uml:attribute ;
  uml:id "EAID_AD939A3B_164A_4ef1_A322_9B323EAC9AC7" .

cim:CDPSMVersion.version a owl:DatatypeProperty, owl:FunctionalProperty ;
  rdfs:label "version" ;
  rdfs:comment "working in progress to construct profiles."@en ;
  rdfs:domain cim:CDPSMVersion ;
  rdfs:isDefinedBy :Package_Extensions ;
  rdfs:range xsd:string ;
  uml:hasInitialValue "cdpsm2015 v1.2.5" ;
  uml:hasStereotype uml:attribute ;
  uml:id "EAID_58C81E00_5CD5_4ea2_AFA9_D97052FBA0ED" .

cim:CatalogAssetType.type a owl:DatatypeProperty, owl:FunctionalProperty ;
  rdfs:label "type" ;
  rdfs:domain cim:CatalogAssetType ;
  rdfs:isDefinedBy :Package_Standard ;
  rdfs:range xsd:string ;
  uml:hasStereotype uml:attribute ;
  uml:id "EAID_62F113CC_123F_4e5a_9C29_2E44010B2873" .

cim:DateTimeInterval.end a owl:DatatypeProperty, owl:FunctionalProperty ;
  rdfs:label "end" ;
  rdfs:comment "End date and time of this interval."@en ;
  rdfs:domain cim:DateTimeInterval ;
  rdfs:isDefinedBy :Package_CompoundTypes ;
  rdfs:range xsd:dateTime ;
  uml:hasStereotype uml:attribute ;
  uml:id "EAID_0ABC99C4_CBB4_45f5_8A37_418A0411A32D" .

cim:DateTimeInterval.start a owl:DatatypeProperty, owl:FunctionalProperty ;
  rdfs:label "start" ;
  rdfs:comment "Start date and time of this interval."@en ;
  rdfs:domain cim:DateTimeInterval ;
  rdfs:isDefinedBy :Package_CompoundTypes ;
  rdfs:range xsd:dateTime ;
  uml:hasStereotype uml:attribute ;
  uml:id "EAID_1541ACE8_204E_4f8c_ADED_0C21681F617D" .

cim:EndDeviceInfo.phaseCount a owl:DatatypeProperty, owl:FunctionalProperty ;
  rdfs:label "phaseCount" ;
  rdfs:comment "Number of potential phases the end device supports, typically 0, 1 or 3."@en ;
  rdfs:domain cim:EndDeviceInfo ;
  rdfs:isDefinedBy :Package_Standard ;
  rdfs:range xsd:integer ;
  uml:hasStereotype uml:attribute ;
  uml:id "EAID_7714DC56_9EDF_4e07_8336_54F44307B570" .

cim:IEC61968CIMVersion.date a owl:DatatypeProperty, owl:FunctionalProperty ;
  rdfs:label "date" ;
  rdfs:comment "Form is YYYY-MM-DD for example for January 5, 2009 it is 2009-01-05."@en ;
  rdfs:domain cim:IEC61968CIMVersion ;
  rdfs:isDefinedBy :Package_CDPSM2015_Versions ;
  rdfs:range xsd:date ;
  uml:hasInitialValue "2016-06-22" ;
  uml:hasStereotype uml:attribute ;
  uml:id "EAID_41AEDCC5_85BE_4aa8_9858_AFA1476927C0" .

cim:IEC61968CIMVersion.version a owl:DatatypeProperty, owl:FunctionalProperty ;
  rdfs:label "version" ;
  rdfs:comment "Form is IEC61968CIMXXvYY where XX is the major CIM package version and the YY is the minor version. For example IEC61968CIM10v17."@en ;
  rdfs:domain cim:IEC61968CIMVersion ;
  rdfs:isDefinedBy :Package_CDPSM2015_Versions ;
  rdfs:range xsd:string ;
  uml:hasInitialValue "IEC61968CIM13v09" ;
  uml:hasStereotype uml:attribute ;
  uml:id "EAID_856CD9B1_8D25_409e_9443_BC7BD9970C40" .

cim:IEC61970CIMVersion.date a owl:DatatypeProperty, owl:FunctionalProperty ;
  rdfs:label "date" ;
  rdfs:comment "Form is YYYY-MM-DD for example for January 5, 2009 it is 2009-01-05."@en ;
  rdfs:domain cim:IEC61970CIMVersion ;
  rdfs:isDefinedBy :Package_CDPSM2015_Versions ;
  rdfs:range xsd:date ;
  uml:hasInitialValue "2016-10-28" ;
  uml:hasStereotype uml:attribute ;
  uml:id "EAID_73319DDD_3044_4b10_BF3F_B98F7D4335FB" .

cim:IEC61970CIMVersion.version a owl:DatatypeProperty, owl:FunctionalProperty ;
  rdfs:label "version" ;
  rdfs:comment "Form is IEC61970CIMXXvYY where XX is the major CIM package version and the YY is the minor version. For example IEC61970CIM13v18."@en ;
  rdfs:domain cim:IEC61970CIMVersion ;
  rdfs:isDefinedBy :Package_CDPSM2015_Versions ;
  rdfs:range xsd:string ;
  uml:hasInitialValue "IEC61970CIM17v19" ;
  uml:hasStereotype uml:attribute ;
  uml:id "EAID_A34E3511_2B8B_47f5_83E6_23564E48933C" .

cim:IdentifiedObject.aliasName a owl:DatatypeProperty, owl:FunctionalProperty ;
  rdfs:label "aliasName" ;
  rdfs:comment """The aliasName is free text human readable name of the object alternative to IdentifiedObject.name. It may be non unique and may not correlate to a naming hierarchy.
      The attribute aliasName is retained because of backwards compatibility between CIM relases. It is however recommended to replace aliasName with the Name class as aliasName is planned for retirement at a future time."""@en ;
  rdfs:domain cim:IdentifiedObject ;
  rdfs:isDefinedBy :Package_Standard ;
  rdfs:range xsd:string ;
  uml:hasStereotype uml:attribute ;
  uml:id "EAID_D438165D_4D23_4019_88C8_0155C4FC1F5E" .

cim:IdentifiedObject.description a owl:DatatypeProperty, owl:FunctionalProperty ;
  rdfs:label "description" ;
  rdfs:comment "The description is a free human readable text describing or naming the object. It may be non unique and may not correlate to a naming hierarchy."@en ;
  rdfs:domain cim:IdentifiedObject ;
  rdfs:isDefinedBy :Package_Standard ;
  rdfs:range xsd:string ;
  uml:hasStereotype uml:attribute ;
  uml:id "EAID_EC34D7A0_366D_49c8_BF54_5F6A6B31AB7B" .

cim:IdentifiedObject.mRID a owl:DatatypeProperty, owl:FunctionalProperty ;
  rdfs:label "mRID" ;
  rdfs:comment """Master resource identifier issued by a model authority. The mRID is globally unique within an exchange context. Global uniqueness is easily achieved by using a UUID,  as specified in RFC 4122, for the mRID.  The use of UUID is strongly recommended.
      For CIMXML data files in RDF syntax conforming to IEC 61970-552 Edition 1, the mRID is mapped to rdf:ID or rdf:about attributes that identify CIM object elements."""@en ;
  rdfs:domain cim:IdentifiedObject ;
  rdfs:isDefinedBy :Package_Standard ;
  rdfs:range xsd:string ;
  uml:hasStereotype uml:attribute ;
  uml:id "EAID_BCB02C75_7925_4562_B5C7_3AA33942648E" .

cim:IdentifiedObject.name a owl:DatatypeProperty, owl:FunctionalProperty ;
  rdfs:label "name" ;
  rdfs:comment "The name is any free human readable and possibly non unique text naming the object."@en ;
  rdfs:domain cim:IdentifiedObject ;
  rdfs:isDefinedBy :Package_Standard ;
  rdfs:range xsd:string ;
  uml:hasStereotype uml:attribute ;
  uml:id "EAID_A99A1C3D_D4F0_4921_8FCD_FF8F7C570208" .

cim:LifecycleDate.installationDate a owl:DatatypeProperty, owl:FunctionalProperty ;
  rdfs:label "installationDate" ;
  rdfs:comment "(if applicable) Date current installation was completed, which may not be the same as the in-service date. Asset may have been installed at other locations previously. Ignored if asset is (1) not currently installed (e.g., stored in a depot) or (2) not intended to be installed (e.g., vehicle, tool)."@en ;
  rdfs:domain cim:LifecycleDate ;
  rdfs:isDefinedBy :Package_CompoundTypes ;
  rdfs:range xsd:date ;
  uml:hasStereotype uml:attribute ;
  uml:id "EAID_F217E2B7_A6EF_4ac2_BBD4_43C83B8B995E" .

cim:LifecycleDate.manufacturedDate a owl:DatatypeProperty, owl:FunctionalProperty ;
  rdfs:label "manufacturedDate" ;
  rdfs:comment "Date the asset was manufactured."@en ;
  rdfs:domain cim:LifecycleDate ;
  rdfs:isDefinedBy :Package_CompoundTypes ;
  rdfs:range xsd:date ;
  uml:hasStereotype uml:attribute ;
  uml:id "EAID_FB93BCF2_1C59_4f75_A5BF_EA1A77E2DDA2" .

cim:LifecycleDate.purchaseDate a owl:DatatypeProperty, owl:FunctionalProperty ;
  rdfs:label "purchaseDate" ;
  rdfs:comment "Date the asset was purchased. Note that even though an asset may have been purchased, it may not have been received into inventory at the time of purchase."@en ;
  rdfs:domain cim:LifecycleDate ;
  rdfs:isDefinedBy :Package_CompoundTypes ;
  rdfs:range xsd:date ;
  uml:hasStereotype uml:attribute ;
  uml:id "EAID_67A99AE2_0EC4_4726_AA84_6932D5342E0F" .

cim:LifecycleDate.receivedDate a owl:DatatypeProperty, owl:FunctionalProperty ;
  rdfs:label "receivedDate" ;
  rdfs:comment "Date the asset was received and first placed into inventory."@en ;
  rdfs:domain cim:LifecycleDate ;
  rdfs:isDefinedBy :Package_CompoundTypes ;
  rdfs:range xsd:date ;
  uml:hasStereotype uml:attribute ;
  uml:id "EAID_4AC4E0C8_145C_4ea3_AC43_59DD55DC0B76" .

cim:LifecycleDate.removalDate a owl:DatatypeProperty, owl:FunctionalProperty ;
  rdfs:label "removalDate" ;
  rdfs:comment "(if applicable) Date when the asset was last removed from service. Ignored if (1) not intended to be in service, or (2) currently in service."@en ;
  rdfs:domain cim:LifecycleDate ;
  rdfs:isDefinedBy :Package_CompoundTypes ;
  rdfs:range xsd:date ;
  uml:hasStereotype uml:attribute ;
  uml:id "EAID_DA08E6B4_43FF_4bb1_87C6_267E1E2E8257" .

cim:LifecycleDate.retiredDate a owl:DatatypeProperty, owl:FunctionalProperty ;
  rdfs:label "retiredDate" ;
  rdfs:comment "(if applicable) Date the asset is permanently retired from service and may be scheduled for disposal. Ignored if asset is (1) currently in service, or (2) permanently removed from service."@en ;
  rdfs:domain cim:LifecycleDate ;
  rdfs:isDefinedBy :Package_CompoundTypes ;
  rdfs:range xsd:date ;
  uml:hasStereotype uml:attribute ;
  uml:id "EAID_227AFC69_980F_45c2_A789_5ED9B056F9CA" .

cim:Name.name a owl:DatatypeProperty, owl:FunctionalProperty ;
  rdfs:label "name" ;
  rdfs:comment "Any free text that name the object."@en ;
  rdfs:domain cim:Name ;
  rdfs:isDefinedBy :Package_Standard ;
  rdfs:range xsd:string ;
  uml:hasStereotype uml:attribute ;
  uml:id "EAID_2E511BC7_4EBE_4ebc_9880_22CFF8FD877A" .

cim:NameType.description a owl:DatatypeProperty, owl:FunctionalProperty ;
  rdfs:label "description" ;
  rdfs:comment "Description of the name type."@en ;
  rdfs:domain cim:NameType ;
  rdfs:isDefinedBy :Package_Standard ;
  rdfs:range xsd:string ;
  uml:hasStereotype uml:attribute ;
  uml:id "EAID_3EA8D22E_8936_46d4_B452_9EF193F21104" .

cim:NameType.name a owl:DatatypeProperty, owl:FunctionalProperty ;
  rdfs:label "name" ;
  rdfs:comment "Name of the name type."@en ;
  rdfs:domain cim:NameType ;
  rdfs:isDefinedBy :Package_Standard ;
  rdfs:range xsd:string ;
  uml:hasStereotype uml:attribute ;
  uml:id "EAID_13DDE54F_EAAB_490e_BCF6_9C2FEBEE9819" .

cim:NameTypeAuthority.description a owl:DatatypeProperty, owl:FunctionalProperty ;
  rdfs:label "description" ;
  rdfs:comment "Description of the name type authority."@en ;
  rdfs:domain cim:NameTypeAuthority ;
  rdfs:isDefinedBy :Package_Standard ;
  rdfs:range xsd:string ;
  uml:hasStereotype uml:attribute ;
  uml:id "EAID_9AA23B4D_4A32_4184_8B9F_81376655C5D6" .

cim:NameTypeAuthority.name a owl:DatatypeProperty, owl:FunctionalProperty ;
  rdfs:label "name" ;
  rdfs:comment "Name of the name type authority."@en ;
  rdfs:domain cim:NameTypeAuthority ;
  rdfs:isDefinedBy :Package_Standard ;
  rdfs:range xsd:string ;
  uml:hasStereotype uml:attribute ;
  uml:id "EAID_6C6D55BC_5C27_4771_874C_15268AB4D9B6" .

cim:PerLengthPhaseImpedance.conductorCount a owl:DatatypeProperty, owl:FunctionalProperty ;
  rdfs:label "conductorCount" ;
  rdfs:comment "Number of phase, neutral, and other wires retained. Constrains the number of matrix elements and the phase codes that can be used with this matrix."@en ;
  rdfs:domain cim:PerLengthPhaseImpedance ;
  rdfs:isDefinedBy :Package_Standard ;
  rdfs:range xsd:integer ;
  uml:hasStereotype uml:attribute ;
  uml:id "EAID_3A14C1A4_C1AA_47fa_BF37_74DF900F6EAB" .

cim:ProductAssetModel.modelNumber a owl:DatatypeProperty, owl:FunctionalProperty ;
  rdfs:label "modelNumber" ;
  rdfs:comment "Manufacturer's model number."@en ;
  rdfs:domain cim:ProductAssetModel ;
  rdfs:isDefinedBy :Package_Standard ;
  rdfs:range xsd:string ;
  uml:hasStereotype uml:attribute ;
  uml:id "EAID_4BC6B998_6811_4ad6_AE12_F40F1D1D83FA" .

cim:ProductAssetModel.modelVersion a owl:DatatypeProperty, owl:FunctionalProperty ;
  rdfs:label "modelVersion" ;
  rdfs:comment "Version number for product model, which indicates vintage of the product."@en ;
  rdfs:domain cim:ProductAssetModel ;
  rdfs:isDefinedBy :Package_Standard ;
  rdfs:range xsd:string ;
  uml:hasStereotype uml:attribute ;
  uml:id "EAID_5CDF895C_920D_49ab_A96E_8711CA4B078D" .

cim:Status.dateTime a owl:DatatypeProperty, owl:FunctionalProperty ;
  rdfs:label "dateTime" ;
  rdfs:comment "Date and time for which status 'value' applies."@en ;
  rdfs:domain cim:Status ;
  rdfs:isDefinedBy :Package_CompoundTypes ;
  rdfs:range xsd:dateTime ;
  uml:hasStereotype uml:attribute ;
  uml:id "EAID_286829E9_8B62_471f_8507_68D03E2B9A3F" .

cim:Status.reason a owl:DatatypeProperty, owl:FunctionalProperty ;
  rdfs:label "reason" ;
  rdfs:comment "Reason code or explanation for why an object went to the current status 'value'."@en ;
  rdfs:domain cim:Status ;
  rdfs:isDefinedBy :Package_CompoundTypes ;
  rdfs:range xsd:string ;
  uml:hasStereotype uml:attribute ;
  uml:id "EAID_51E12DAD_FC37_4dfe_A8E4_A273F0EFD65C" .

cim:Status.remark a owl:DatatypeProperty, owl:FunctionalProperty ;
  rdfs:label "remark" ;
  rdfs:comment "Pertinent information regarding the current 'value', as free form text."@en ;
  rdfs:domain cim:Status ;
  rdfs:isDefinedBy :Package_CompoundTypes ;
  rdfs:range xsd:string ;
  uml:hasStereotype uml:attribute ;
  uml:id "EAID_8B7584AD_FB53_4d76_BBFE_72EE31608485" .

cim:Status.value a owl:DatatypeProperty, owl:FunctionalProperty ;
  rdfs:label "value" ;
  rdfs:comment "Status value at 'dateTime'; prior status changes may have been kept in instances of activity records associated with the object to which this status applies."@en ;
  rdfs:domain cim:Status ;
  rdfs:isDefinedBy :Package_CompoundTypes ;
  rdfs:range xsd:string ;
  uml:hasStereotype uml:attribute ;
  uml:id "EAID_0184B3DA_228D_41b3_AD2F_7C17DD4041D0" .

cim:StreetDetail.addressGeneral a owl:DatatypeProperty, owl:FunctionalProperty ;
  rdfs:label "addressGeneral" ;
  rdfs:comment "Additional address information, for example a mailstop."@en ;
  rdfs:domain cim:StreetDetail ;
  rdfs:isDefinedBy :Package_CompoundTypes ;
  rdfs:range xsd:string ;
  uml:hasStereotype uml:attribute ;
  uml:id "EAID_8A85C8D2_C0B9_4107_A0FC_B7B9EF07C4E9" .

cim:StreetDetail.name a owl:DatatypeProperty, owl:FunctionalProperty ;
  rdfs:label "name" ;
  rdfs:comment "Name of the street."@en ;
  rdfs:domain cim:StreetDetail ;
  rdfs:isDefinedBy :Package_CompoundTypes ;
  rdfs:range xsd:string ;
  uml:hasStereotype uml:attribute ;
  uml:id "EAID_947A58E8_F9CE_4429_BD6F_C705D885681C" .

cim:StreetDetail.number a owl:DatatypeProperty, owl:FunctionalProperty ;
  rdfs:label "number" ;
  rdfs:comment "Designator of the specific location on the street."@en ;
  rdfs:domain cim:StreetDetail ;
  rdfs:isDefinedBy :Package_CompoundTypes ;
  rdfs:range xsd:string ;
  uml:hasStereotype uml:attribute ;
  uml:id "EAID_64B56973_8008_434f_8AF7_03FE55395188" .

cim:StreetDetail.type a owl:DatatypeProperty, owl:FunctionalProperty ;
  rdfs:label "type" ;
  rdfs:comment "Type of street. Examples include: street, circle, boulevard, avenue, road, drive, etc."@en ;
  rdfs:domain cim:StreetDetail ;
  rdfs:isDefinedBy :Package_CompoundTypes ;
  rdfs:range xsd:string ;
  uml:hasStereotype uml:attribute ;
  uml:id "EAID_965CC979_ED3B_41f2_AAFF_3FFAE2035C15" .

cim:TapChangerInfo.highStep a owl:DatatypeProperty, owl:FunctionalProperty ;
  rdfs:label "highStep" ;
  rdfs:comment "Highest possible tap step position, advance from neutral."@en ;
  rdfs:domain cim:TapChangerInfo ;
  rdfs:isDefinedBy :Package_Standard ;
  rdfs:range xsd:integer ;
  uml:hasStereotype uml:attribute ;
  uml:id "EAID_3FAFBEA5_1188_4d93_899C_83D671CCD3AF" .

cim:TapChangerInfo.lowStep a owl:DatatypeProperty, owl:FunctionalProperty ;
  rdfs:label "lowStep" ;
  rdfs:comment "Lowest possible tap step position, retard from neutral."@en ;
  rdfs:domain cim:TapChangerInfo ;
  rdfs:isDefinedBy :Package_Standard ;
  rdfs:range xsd:integer ;
  uml:hasStereotype uml:attribute ;
  uml:id "EAID_FAEB1364_D56F_475f_AE37_4F54C30A2189" .

cim:TapChangerInfo.neutralStep a owl:DatatypeProperty, owl:FunctionalProperty ;
  rdfs:label "neutralStep" ;
  rdfs:comment "The neutral tap step position for the winding."@en ;
  rdfs:domain cim:TapChangerInfo ;
  rdfs:isDefinedBy :Package_Standard ;
  rdfs:range xsd:integer ;
  uml:hasStereotype uml:attribute ;
  uml:id "EAID_BEE5F275_7E66_45a8_BF6E_AE00976E7AE4" .

cim:TownDetail.code a owl:DatatypeProperty, owl:FunctionalProperty ;
  rdfs:label "code" ;
  rdfs:comment "Town code."@en ;
  rdfs:domain cim:TownDetail ;
  rdfs:isDefinedBy :Package_CompoundTypes ;
  rdfs:range xsd:string ;
  uml:hasStereotype uml:attribute ;
  uml:id "EAID_CA70DEEB_1A1A_4719_8887_E0397E8ED173" .

cim:TownDetail.name a owl:DatatypeProperty, owl:FunctionalProperty ;
  rdfs:label "name" ;
  rdfs:comment "Town name."@en ;
  rdfs:domain cim:TownDetail ;
  rdfs:isDefinedBy :Package_CompoundTypes ;
  rdfs:range xsd:string ;
  uml:hasStereotype uml:attribute ;
  uml:id "EAID_111467DB_41AF_40c7_8D2A_800EA073C678" .

cim:TransformerEndInfo.endNumber a owl:DatatypeProperty, owl:FunctionalProperty ;
  rdfs:label "endNumber" ;
  rdfs:comment "Number for this transformer end, corresponding to the end's order in the PowerTransformer.vectorGroup attribute. Highest voltage winding should be 1."@en ;
  rdfs:domain cim:TransformerEndInfo ;
  rdfs:isDefinedBy :Package_Standard ;
  rdfs:range xsd:integer ;
  uml:hasStereotype uml:attribute ;
  uml:id "EAID_E5A926F1_0DCF_48dd_9799_D8AE4B4CA189" .

cim:TransformerEndInfo.phaseAngleClock a owl:DatatypeProperty, owl:FunctionalProperty ;
  rdfs:label "phaseAngleClock" ;
  rdfs:comment "Winding phase angle where 360 degrees are represented with clock hours, so the valid values are {0, ..., 11}. For example, to express winding code 'Dyn11', set attributes as follows: 'connectionKind' = Yn and 'phaseAngleClock' = 11."@en ;
  rdfs:domain cim:TransformerEndInfo ;
  rdfs:isDefinedBy :Package_Standard ;
  rdfs:range xsd:integer ;
  uml:hasStereotype uml:attribute ;
  uml:id "EAID_97F04B11_9719_4c06_8E41_FE6FE22CAA4C" .

cim:WireInfo.insulated a owl:DatatypeProperty, owl:FunctionalProperty ;
  rdfs:label "insulated" ;
  rdfs:comment "True if conductor is insulated."@en ;
  rdfs:domain cim:WireInfo ;
  rdfs:isDefinedBy :Package_Standard ;
  rdfs:range xsd:boolean ;
  uml:hasStereotype uml:attribute ;
  uml:id "EAID_598D5EA7_618B_4104_B69E_E753312A1FBB" .

cim:WireInfo.sizeDescription a owl:DatatypeProperty, owl:FunctionalProperty ;
  rdfs:label "sizeDescription" ;
  rdfs:comment "Describes the wire guage or cross section (e.g., 4/0, #2, 336.5)."@en ;
  rdfs:domain cim:WireInfo ;
  rdfs:isDefinedBy :Package_Standard ;
  rdfs:range xsd:string ;
  uml:hasStereotype uml:attribute ;
  uml:id "EAID_D681D33A_56A4_43da_B43F_C20BB3E98507" .

cim:WireInfo.strandCount a owl:DatatypeProperty, owl:FunctionalProperty ;
  rdfs:label "strandCount" ;
  rdfs:comment "Number of strands in the conductor."@en ;
  rdfs:domain cim:WireInfo ;
  rdfs:isDefinedBy :Package_Standard ;
  rdfs:range xsd:integer ;
  uml:hasStereotype uml:attribute ;
  uml:id "EAID_5738ABE5_DD2F_442a_984F_6A81AFF0ABAD" .

cim:WireSpacing.isCable a owl:DatatypeProperty, owl:FunctionalProperty ;
  rdfs:label "isCable" ;
  rdfs:comment "If true, this spacing data describes a cable."@en ;
  rdfs:domain cim:WireSpacing ;
  rdfs:isDefinedBy :Package_Standard ;
  rdfs:range xsd:boolean ;
  uml:hasStereotype uml:attribute ;
  uml:id "EAID_6DE80290_0550_492e_9475_B9C043363830" .

cim:WireSpacing.phaseWireCount a owl:DatatypeProperty, owl:FunctionalProperty ;
  rdfs:label "phaseWireCount" ;
  rdfs:comment "Number of wire sub-conductors in the symmetrical bundle (typically between 1 and 4)."@en ;
  rdfs:domain cim:WireSpacing ;
  rdfs:isDefinedBy :Package_Standard ;
  rdfs:range xsd:integer ;
  uml:hasStereotype uml:attribute ;
  uml:id "EAID_C7521791_CB27_42a5_854C_C23188D51E23" .

md:Description.description a owl:DatatypeProperty, owl:FunctionalProperty ;
  rdfs:label "description" ;
  rdfs:domain md:Description ;
  rdfs:isDefinedBy :Package_ModelDescription ;
  rdfs:range xsd:string ;
  uml:hasStereotype uml:attribute ;
  uml:id "EAID_77D4EA3B_765E_4535_8798_19A334B793CD" .

md:Description.name a owl:DatatypeProperty, owl:FunctionalProperty ;
  rdfs:label "name" ;
  rdfs:domain md:Description ;
  rdfs:isDefinedBy :Package_ModelDescription ;
  rdfs:range xsd:string ;
  uml:hasStereotype uml:attribute ;
  uml:id "EAID_2112E71B_4C0E_42fe_B846_0C25245AD4AA" .

md:Description.version a owl:DatatypeProperty, owl:FunctionalProperty ;
  rdfs:label "version" ;
  rdfs:domain md:Description ;
  rdfs:isDefinedBy :Package_ModelDescription ;
  rdfs:range xsd:integer ;
  uml:hasStereotype uml:attribute ;
  uml:id "EAID_FF52CCA3_DC42_415b_B3DC_1896EDF5D285" .

md:DescriptionID.uri a owl:DatatypeProperty, owl:FunctionalProperty ;
  rdfs:label "uri" ;
  rdfs:domain md:DescriptionID ;
  rdfs:isDefinedBy :Package_ModelDescription ;
  rdfs:range xsd:string ;
  uml:hasStereotype uml:attribute ;
  uml:id "EAID_3CE77DD2_B3AC_4276_8CD1_5C88ACFD6925" .

md:Model.created a owl:DatatypeProperty, owl:FunctionalProperty ;
  rdfs:label "created" ;
  rdfs:domain md:Model ;
  rdfs:isDefinedBy :Package_ModelDescription ;
  rdfs:range xsd:dateTime ;
  uml:hasStereotype uml:attribute ;
  uml:id "EAID_D9AA16E6_6140_43bb_8AE1_6BB4690421D5" .

md:Model.description a owl:DatatypeProperty, owl:FunctionalProperty ;
  rdfs:label "description" ;
  rdfs:domain md:Model ;
  rdfs:isDefinedBy :Package_ModelDescription ;
  rdfs:range xsd:string ;
  uml:hasStereotype uml:attribute ;
  uml:id "EAID_2D2FD5B2_D2E1_4f18_B2A6_C344E4F8F056" .

md:Model.scenarioTime a owl:DatatypeProperty, owl:FunctionalProperty ;
  rdfs:label "scenarioTime" ;
  rdfs:domain md:Model ;
  rdfs:isDefinedBy :Package_ModelDescription ;
  rdfs:range xsd:dateTime ;
  uml:hasStereotype uml:attribute ;
  uml:id "EAID_93B61862_8552_4d68_982A_5988CF10A5CE" .

md:Model.version a owl:DatatypeProperty, owl:FunctionalProperty ;
  rdfs:label "version" ;
  rdfs:domain md:Model ;
  rdfs:isDefinedBy :Package_ModelDescription ;
  rdfs:range xsd:string ;
  uml:hasStereotype uml:attribute ;
  uml:id "EAID_5C9430BF_6E71_4a91_93D8_4EE62DF835AF" .

md:ModelDescriptionCIMVersion.date a owl:DatatypeProperty, owl:FunctionalProperty ;
  rdfs:label "date" ;
  rdfs:domain md:ModelDescriptionCIMVersion ;
  rdfs:isDefinedBy :Package_ModelDescription ;
  rdfs:range xsd:date ;
  uml:hasStereotype uml:attribute ;
  uml:id "EAID_3D4AE5F1_0F47_469a_88ED_6CA88FE74BAC" .

md:ModelDescriptionCIMVersion.version a owl:DatatypeProperty, owl:FunctionalProperty ;
  rdfs:label "version" ;
  rdfs:domain md:ModelDescriptionCIMVersion ;
  rdfs:isDefinedBy :Package_ModelDescription ;
  rdfs:range xsd:string ;
  uml:hasStereotype uml:attribute ;
  uml:id "EAID_E4CE2321_4D4C_4ff2_B28D_9379D107022B" .

next:PowerTransformerInfoEx.integratedFuse a owl:DatatypeProperty, owl:FunctionalProperty ;
  rdfs:label "integratedFuse" ;
  rdfs:comment "Is a fuse integrated in the transformer ?"@en ;
  rdfs:domain next:PowerTransformerInfoEx ;
  rdfs:isDefinedBy :Package_EDFExtensions ;
  rdfs:range xsd:boolean ;
  uml:hasStereotype uml:attribute ;
  uml:id "EAID_F2B8AA40_F3E7_470a_A628_066B4CBCA32E" .

rdfs:comment a owl:AnnotationProperty ;
  rdfs:label "description", "documentation" ;
  uml:id "EAID_1699E23F_8411_4351_A573_4D126B4F01CE", "EAID_8679E8D1_6606_4048_A8C3_6CD1BB41120E", "EAID_95ACFDE2_427F_4b8d_9C30_575783CB7FD0", "EAID_E647E6B9_97E3_4fa8_AC57_95A29E170D12" .

uml:baseprefix a owl:AnnotationProperty .

uml:baseuri a owl:AnnotationProperty .

uml:hasInitialValue a owl:AnnotationProperty .

uml:hasMaxCardinality a owl:AnnotationProperty .

uml:hasMinCardinality a owl:AnnotationProperty .

uml:hasMultiplier a owl:AnnotationProperty .

uml:hasStereotype a owl:AnnotationProperty .

uml:hasUnits a owl:AnnotationProperty .

uml:id a owl:AnnotationProperty .

uml:roleALabel a owl:AnnotationProperty .

uml:roleAOf a owl:AnnotationProperty .

uml:roleBLabel a owl:AnnotationProperty .

uml:roleBOf a owl:AnnotationProperty .

uml:uriHasPrefix a owl:AnnotationProperty .

:Package_CDPSM2015_Versions a uml:Package ;
  rdfs:label "CDPSM2015_Versions" ;
  uml:baseuri "https://cim.ucaiug.io/ns#" ;
  uml:id "EAPK_28BCB051_6D19_4a4c_A476_FEFCD7150943" .

:Package_CIMDataTypes a uml:Package ;
  rdfs:label "CIMDataTypes" ;
  rdfs:isDefinedBy :Package_DataTypes ;
  uml:baseuri "https://cim.ucaiug.io/ns#" ;
  uml:id "EAPK_C17AEB8B_8DB4_4c39_96D7_03E08C4E5EB1" .

:Package_CIMEnumerations a uml:Package ;
  rdfs:label "CIMEnumerations" ;
  rdfs:isDefinedBy :Package_DataTypes ;
  uml:baseuri "https://cim.ucaiug.io/ns#" ;
  uml:id "EAPK_D246256B_B69C_47df_BDD3_52D0BDB191EB" .

:Package_CIMExtensions a uml:Package ;
  rdfs:label "CIMExtensions" ;
  rdfs:isDefinedBy :Package_Catalog ;
  uml:baseuri "http://edf.fr/draft/cim17-ext#" ;
  uml:id "EAPK_0DA12261_FD7E_4713_8280_AADBB4A9B85B" .

:Package_Catalog a uml:Package ;
  rdfs:label "Catalog" ;
  uml:baseuri "https://cim.ucaiug.io/ns#" ;
  uml:id "EAPK_173EBDC8_1A5C_483b_A19A_9B5AF03FCE39" .

:Package_CompoundTypes a uml:Package ;
  rdfs:label "CompoundTypes" ;
  rdfs:isDefinedBy :Package_DataTypes ;
  uml:baseuri "https://cim.ucaiug.io/ns#" ;
  uml:id "EAPK_6F438211_9449_4fd0_AEF2_6A7898B85CE6" .

:Package_DataTypes a uml:Package ;
  rdfs:label "DataTypes" ;
  uml:baseuri "https://cim.ucaiug.io/ns#" ;
  uml:id "EAPK_4C6C1B78_A35E_4e1a_8FE7_00B567EEE34A" .

:Package_EDFExtensions a uml:Package ;
  rdfs:label "EDFExtensions" ;
  rdfs:isDefinedBy :Package_Catalog ;
  uml:baseuri "http://der.edf.fr/mire/MSite-v3.1.a#" ;
  uml:id "EAPK_660ECC23_FD6A_4439_9FB6_C6112275182E" .

:Package_EntsoeExtensions a uml:Package ;
  rdfs:label "EntsoeExtensions" ;
  rdfs:isDefinedBy :Package_DataTypes ;
  uml:baseuri "https://cim.ucaiug.io/ns#" ;
  uml:id "EAPK_5AA34A0A_7B1B_4772_96AF_359B62E14C2E" .

:Package_Extensions a uml:Package ;
  rdfs:label "Extensions" ;
  rdfs:isDefinedBy :Package_CDPSM2015_Versions ;
  uml:baseuri "https://cim.ucaiug.io/ns#" ;
  uml:id "EAPK_CA794E24_0958_4a83_B276_9765B963AE7D" .

:Package_InfIEC61968 a uml:Package ;
  rdfs:label "InfIEC61968" ;
  rdfs:isDefinedBy :Package_Catalog ;
  uml:baseuri "http://edf.fr/draft/cim17-info#" ;
  uml:id "EAPK_951F3A10_7A56_4383_BDB0_8CC44B4285A9" .

:Package_InfIEC61970 uml:baseuri "http://edf.fr/draft/cim17-info#" .

:Package_ModelAuthority a uml:Package ;
  rdfs:label "ModelAuthority" ;
  rdfs:comment "The package describes meta data for partitioning  power system models into non overlapping subsets of objects managed by a model authority."@en ;
  uml:id "EAPK_FA58BD12_D4BA_4e34_A13E_A26DB6C4EF17" .

:Package_ModelDescription a uml:Package ;
  rdfs:label "ModelDescription" ;
  rdfs:comment "The package describes meta data for the exchange of power system model data."@en ;
  uml:baseuri "http://iec.ch/TC57/61970-552/ModelDescription/1#" ;
  uml:id "EAPK_1FE6534D_F250_4ef7_9343_02B5C21DB333" .

:Package_PowerSystemProject a uml:Package ;
  rdfs:label "PowerSystemProject" ;
  rdfs:comment "The package describes how power system model data is managed and evolve over time in projects."@en ;
  uml:id "EAPK_1813910E_9451_4ae3_BA8D_4DDFC1035E40" .

:Package_PrimitiveTypes a uml:Package ;
  rdfs:label "PrimitiveTypes" ;
  rdfs:isDefinedBy :Package_DataTypes ;
  uml:baseuri "https://cim.ucaiug.io/ns#" ;
  uml:id "EAPK_7B8DB810_3F0E_4dfd_9ED4_5ABBA3E9F7E1" .

:Package_Standard a uml:Package ;
  rdfs:label "Standard" ;
  rdfs:isDefinedBy :Package_Catalog ;
  uml:baseuri "https://cim.ucaiug.io/ns#" ;
  uml:id "EAPK_451561BF_A322_4a0e_953B_B2F191B0A39B" .

:ProjectStepStatusKind.Default a :ProjectStepStatusKind ;
  rdfs:label "ProjectStepStatusKindDefault" ;
  rdfs:comment "ProjectStepStatusKindDefault"@en ;
  rdfs:isDefinedBy :Package_PowerSystemProject .

:StepKind.Default a :StepKind ;
  rdfs:label "StepKindDefault" ;
  rdfs:comment "StepKindDefault"@en ;
  rdfs:isDefinedBy :Package_PowerSystemProject .

:URI a rdfs:Datatype ;
  rdfs:label "URI" ;
  owl:equivalentClass xsd:anyURI ;
  uml:hasStereotype uml:cimdatatype ;
  uml:id "eaxmiid2" .

cim:ActivePower a rdfs:Datatype ;
  rdfs:label "ActivePower" ;
  rdfs:comment "Product of RMS value of the voltage and the RMS value of the in-phase component of the current."@en ;
  owl:equivalentClass xsd:float ;
  rdfs:isDefinedBy :Package_CIMDataTypes ;
  uml:hasMultiplier "M" ;
  uml:hasStereotype uml:cimdatatype ;
  uml:hasUnits "W" ;
  uml:id "EAID_9FDEB934_262D_4e7b_9551_75C9D20BA5C2" .

cim:ActivePowerPerCurrentFlow a rdfs:Datatype ;
  rdfs:label "ActivePowerPerCurrentFlow" ;
  owl:equivalentClass xsd:float ;
  rdfs:isDefinedBy :Package_CIMDataTypes ;
  uml:hasStereotype uml:cimdatatype ;
  uml:hasUnits "WPerA" ;
  uml:id "EAID_EF95FD0D_F934_44ee_94FC_E5318EDA6DB1" .

cim:ActivePowerPerFrequency a rdfs:Datatype ;
  rdfs:label "ActivePowerPerFrequency" ;
  rdfs:comment "Active power variation with frequency."@en ;
  owl:equivalentClass xsd:float ;
  rdfs:isDefinedBy :Package_CIMDataTypes ;
  uml:hasStereotype uml:cimdatatype ;
  uml:hasUnits "WPerHz" ;
  uml:id "EAID_3E3062AA_5BD3_43dd_9D18_3D96BCC10784" .

cim:AngleDegrees a rdfs:Datatype ;
  rdfs:label "AngleDegrees" ;
  rdfs:comment "Measurement of angle in degrees"@en ;
  owl:equivalentClass xsd:float ;
  rdfs:isDefinedBy :Package_CIMDataTypes ;
  uml:hasMultiplier "none" ;
  uml:hasStereotype uml:cimdatatype ;
  uml:hasUnits "deg" ;
  uml:id "EAID_8E77941D_A918_4ca6_B37B_2C3671D68B4D" .

cim:AngleRadians a rdfs:Datatype ;
  rdfs:label "AngleRadians" ;
  rdfs:comment "Phase angle in radians"@en ;
  owl:equivalentClass xsd:float ;
  rdfs:isDefinedBy :Package_CIMDataTypes ;
  uml:hasMultiplier "none" ;
  uml:hasStereotype uml:cimdatatype ;
  uml:hasUnits "rad" ;
  uml:id "EAID_A3F15E20_66CA_44bc_AD64_03BD90A30F48" .

cim:ApparentPower a rdfs:Datatype ;
  rdfs:label "ApparentPower" ;
  rdfs:comment "Product of the RMS value of the voltage and the RMS value of the current"@en ;
  owl:equivalentClass xsd:float ;
  rdfs:isDefinedBy :Package_CIMDataTypes ;
  uml:hasMultiplier "M" ;
  uml:hasStereotype uml:cimdatatype ;
  uml:hasUnits "VA" ;
  uml:id "EAID_42FA3B9C_DD19_4c11_B9D4_7C9BAA7BBAB0" .

cim:AssetModelUsageKind.customerSubstation a cim:AssetModelUsageKind ;
  rdfs:label "customerSubstation" ;
  rdfs:comment "Asset model is intended for use in customer substation."@en ;
  rdfs:isDefinedBy :Package_CIMEnumerations ;
  uml:id "EAID_451D749A_35B8_46d2_ACF1_0B1846EC4F16" .

cim:AssetModelUsageKind.distributionOverhead a cim:AssetModelUsageKind ;
  rdfs:label "distributionOverhead" ;
  rdfs:comment "Asset model is intended for use in distribution overhead network."@en ;
  rdfs:isDefinedBy :Package_CIMEnumerations ;
  uml:id "EAID_5400E932_09E5_49dd_85FB_51AD27E1712D" .

cim:AssetModelUsageKind.distributionUnderground a cim:AssetModelUsageKind ;
  rdfs:label "distributionUnderground" ;
  rdfs:comment "Asset model is intended for use in underground distribution network."@en ;
  rdfs:isDefinedBy :Package_CIMEnumerations ;
  uml:id "EAID_DD733D41_C7D4_4966_8072_47CB63BF3A0F" .

cim:AssetModelUsageKind.other a cim:AssetModelUsageKind ;
  rdfs:label "other" ;
  rdfs:comment "Other kind of asset model usage."@en ;
  rdfs:isDefinedBy :Package_CIMEnumerations ;
  uml:id "EAID_13EBDC0B_CF44_4b89_9BEB_85CF9D6DC67E" .

cim:AssetModelUsageKind.streetlight a cim:AssetModelUsageKind ;
  rdfs:label "streetlight" ;
  rdfs:comment "Asset model is intended for use as streetlight."@en ;
  rdfs:isDefinedBy :Package_CIMEnumerations ;
  uml:id "EAID_641028DE_403E_4bb9_8B7F_39B620D4F3FC" .

cim:AssetModelUsageKind.substation a cim:AssetModelUsageKind ;
  rdfs:label "substation" ;
  rdfs:comment "Asset model is intended for use in substation."@en ;
  rdfs:isDefinedBy :Package_CIMEnumerations ;
  uml:id "EAID_CF8F68FF_8613_469b_8A5B_A58FD4F7F700" .

cim:AssetModelUsageKind.transmission a cim:AssetModelUsageKind ;
  rdfs:label "transmission" ;
  rdfs:comment "Asset model is intended for use in transmission network."@en ;
  rdfs:isDefinedBy :Package_CIMEnumerations ;
  uml:id "EAID_64CBD772_2ABF_417b_8980_C446B73E3E04" .

cim:AssetModelUsageKind.unknown a cim:AssetModelUsageKind ;
  rdfs:label "unknown" ;
  rdfs:comment "Usage of the asset model is unknown."@en ;
  rdfs:isDefinedBy :Package_CIMEnumerations ;
  uml:id "EAID_87E82A02_3DC6_45d2_B406_BC4825202653" .

cim:AsynchronousMachineKind.generator a cim:AsynchronousMachineKind ;
  rdfs:label "generator" ;
  rdfs:comment "The Asynchronous Machine is a generator."@en ;
  rdfs:isDefinedBy :Package_CIMEnumerations ;
  uml:id "EAID_48ECF68C_AA4D_41a2_93AC_7C4AE196D72C" .

cim:AsynchronousMachineKind.motor a cim:AsynchronousMachineKind ;
  rdfs:label "motor" ;
  rdfs:comment "The Asynchronous Machine is a motor."@en ;
  rdfs:isDefinedBy :Package_CIMEnumerations ;
  uml:id "EAID_D1B93705_F30F_4184_BF0B_FC18CB4858D7" .

cim:CableConstructionKind.compacted a cim:CableConstructionKind ;
  rdfs:label "compacted" ;
  rdfs:isDefinedBy :Package_CIMEnumerations ;
  uml:id "EAID_C0717798_61AF_4496_8BA8_38D10255C7A9" .

cim:CableConstructionKind.compressed a cim:CableConstructionKind ;
  rdfs:label "compressed" ;
  rdfs:isDefinedBy :Package_CIMEnumerations ;
  uml:id "EAID_FA9CFB9A_9F62_4cbc_8C2A_81D004AAA4E4" .

cim:CableConstructionKind.other a cim:CableConstructionKind ;
  rdfs:label "other" ;
  rdfs:isDefinedBy :Package_CIMEnumerations ;
  uml:id "EAID_CEB1C1A6_B7A6_4c99_B25C_6B66983FD648" .

cim:CableConstructionKind.sector a cim:CableConstructionKind ;
  rdfs:label "sector" ;
  rdfs:isDefinedBy :Package_CIMEnumerations ;
  uml:id "EAID_99FC9376_9C9C_4bc7_8B39_E62604FCCFA7" .

cim:CableConstructionKind.segmental a cim:CableConstructionKind ;
  rdfs:label "segmental" ;
  rdfs:isDefinedBy :Package_CIMEnumerations ;
  uml:id "EAID_2E3FB6B0_CEC7_4600_92D4_A462B3FDDBFA" .

cim:CableConstructionKind.solid a cim:CableConstructionKind ;
  rdfs:label "solid" ;
  rdfs:isDefinedBy :Package_CIMEnumerations ;
  uml:id "EAID_CF90FB65_CD5F_4633_98EB_C464FD91647D" .

cim:CableConstructionKind.stranded a cim:CableConstructionKind ;
  rdfs:label "stranded" ;
  rdfs:isDefinedBy :Package_CIMEnumerations ;
  uml:id "EAID_BBCF9A7A_9F9C_45a8_9F2A_0456347BF6B5" .

cim:CableOuterJacketKind.insulating a cim:CableOuterJacketKind ;
  rdfs:label "insulating" ;
  rdfs:isDefinedBy :Package_CIMEnumerations ;
  uml:id "EAID_2BB5ADE6_DA74_4393_971F_04230E58B706" .

cim:CableOuterJacketKind.linearLowDensityPolyethylene a cim:CableOuterJacketKind ;
  rdfs:label "linearLowDensityPolyethylene" ;
  rdfs:isDefinedBy :Package_CIMEnumerations ;
  uml:id "EAID_8CD68AED_196B_4cd5_B2D0_18699B55ACC8" .

cim:CableOuterJacketKind.none a cim:CableOuterJacketKind ;
  rdfs:label "none" ;
  rdfs:isDefinedBy :Package_CIMEnumerations ;
  uml:id "EAID_348F20DD_324D_475f_A5A9_D0CA956ED5BE" .

cim:CableOuterJacketKind.other a cim:CableOuterJacketKind ;
  rdfs:label "other" ;
  rdfs:isDefinedBy :Package_CIMEnumerations ;
  uml:id "EAID_F2278A86_0174_4eab_B8F8_77A16EC9F3D4" .

cim:CableOuterJacketKind.polyethylene a cim:CableOuterJacketKind ;
  rdfs:label "polyethylene" ;
  rdfs:isDefinedBy :Package_CIMEnumerations ;
  uml:id "EAID_EBB5CF78_2E47_4b11_92AF_781E4B6C112A" .

cim:CableOuterJacketKind.pvc a cim:CableOuterJacketKind ;
  rdfs:label "pvc" ;
  rdfs:isDefinedBy :Package_CIMEnumerations ;
  uml:id "EAID_7F6A242E_80BC_43c9_B2BB_7C3C457AEC2F" .

cim:CableOuterJacketKind.semiconducting a cim:CableOuterJacketKind ;
  rdfs:label "semiconducting" ;
  rdfs:isDefinedBy :Package_CIMEnumerations ;
  uml:id "EAID_CE02D32E_12DE_4f93_AA13_529DB2C22FAD" .

cim:CableShieldMaterialKind.aluminum a cim:CableShieldMaterialKind ;
  rdfs:label "aluminum" ;
  rdfs:isDefinedBy :Package_CIMEnumerations ;
  uml:id "EAID_27223C05_A901_477e_9A43_A318054B08CD" .

cim:CableShieldMaterialKind.copper a cim:CableShieldMaterialKind ;
  rdfs:label "copper" ;
  rdfs:isDefinedBy :Package_CIMEnumerations ;
  uml:id "EAID_46872655_CF94_4810_9F51_DFE4C1E1F792" .

cim:CableShieldMaterialKind.lead a cim:CableShieldMaterialKind ;
  rdfs:label "lead" ;
  rdfs:isDefinedBy :Package_CIMEnumerations ;
  uml:id "EAID_16A14442_8C0F_44cb_B4E9_258923FC2C6E" .

cim:CableShieldMaterialKind.other a cim:CableShieldMaterialKind ;
  rdfs:label "other" ;
  rdfs:isDefinedBy :Package_CIMEnumerations ;
  uml:id "EAID_93554E7F_79B3_41e1_9550_D9375B247B4D" .

cim:CableShieldMaterialKind.steel a cim:CableShieldMaterialKind ;
  rdfs:label "steel" ;
  rdfs:isDefinedBy :Package_CIMEnumerations ;
  uml:id "EAID_BD9D47D6_7A5F_4716_9A6F_4C150CC3BB54" .

cim:Capacitance a rdfs:Datatype ;
  rdfs:label "Capacitance" ;
  rdfs:comment "Capacitive part of reactance (imaginary part of impedance), at rated frequency."@en ;
  owl:equivalentClass xsd:float ;
  rdfs:isDefinedBy :Package_CIMDataTypes ;
  uml:hasMultiplier "none" ;
  uml:hasStereotype uml:cimdatatype ;
  uml:hasUnits "F" ;
  uml:id "EAID_5C5D9592_92D6_4e93_BAD5_32AEFCC3A33E" .

cim:Conductance a rdfs:Datatype ;
  rdfs:label "Conductance" ;
  rdfs:comment "Factor by which voltage must be multiplied to give corresponding power lost from a circuit. Real part of admittance."@en ;
  owl:equivalentClass xsd:float ;
  rdfs:isDefinedBy :Package_CIMDataTypes ;
  uml:hasMultiplier "none" ;
  uml:hasStereotype uml:cimdatatype ;
  uml:hasUnits "S" ;
  uml:id "EAID_2D9C2F58_EAA8_4657_82BE_EF3D0ED215BA" .

cim:ConductancePerLength a rdfs:Datatype ;
  rdfs:label "ConductancePerLength" ;
  rdfs:comment "Real part of admittance per unit of length."@en ;
  owl:equivalentClass xsd:float ;
  rdfs:isDefinedBy :Package_CIMDataTypes ;
  uml:hasMultiplier "none" ;
  uml:hasStereotype uml:cimdatatype ;
  uml:hasUnits "SPerm" ;
  uml:id "EAID_C18C3C34_C763_4d73_8F43_E10FC386C747" .

cim:CurrentFlow a rdfs:Datatype ;
  rdfs:label "CurrentFlow" ;
  rdfs:comment "Electrical current (positive flow is out of the ConductingEquipment into the ConnectivityNode)"@en ;
  owl:equivalentClass xsd:float ;
  rdfs:isDefinedBy :Package_CIMDataTypes ;
  uml:hasMultiplier "none" ;
  uml:hasStereotype uml:cimdatatype ;
  uml:hasUnits "A" ;
  uml:id "EAID_773E16D8_9DF8_426e_BF97_853428CF78C2" .

cim:CurveStyle.constantYValue a cim:CurveStyle ;
  rdfs:label "constantYValue" ;
  rdfs:comment "The Y-axis values are assumed constant until the next curve point and prior to the first curve point."@en ;
  rdfs:isDefinedBy :Package_CIMEnumerations ;
  uml:id "EAID_FFC73338_9482_461e_9CCE_E8396F4793FB" .

cim:CurveStyle.straightLineYValues a cim:CurveStyle ;
  rdfs:label "straightLineYValues" ;
  rdfs:comment "The Y-axis values are assumed to be a straight line between values.  Also known as linear interpolation."@en ;
  rdfs:isDefinedBy :Package_CIMEnumerations ;
  uml:id "EAID_419C93CE_8818_4c89_AB63_BE01921FE30D" .

cim:Displacement a rdfs:Datatype ;
  rdfs:label "Displacement" ;
  rdfs:comment "Unit of displacement relative a reference position, hence can be negative."@en ;
  owl:equivalentClass xsd:float ;
  rdfs:isDefinedBy :Package_CIMDataTypes ;
  uml:hasMultiplier "none" ;
  uml:hasStereotype uml:cimdatatype ;
  uml:hasUnits "m" ;
  uml:id "EAID_FB005E54_4701_40e6_91DA_831E171484D9" .

cim:Frequency a rdfs:Datatype ;
  rdfs:label "Frequency" ;
  rdfs:comment "Cycles per second"@en ;
  owl:equivalentClass xsd:float ;
  rdfs:isDefinedBy :Package_CIMDataTypes ;
  uml:hasMultiplier "none" ;
  uml:hasStereotype uml:cimdatatype ;
  uml:hasUnits "Hz" ;
  uml:id "EAID_56ECB3D9_7270_43de_B868_B58829BE32E3" .

cim:GeneratorControlSource.offAGC a cim:GeneratorControlSource ;
  rdfs:label "offAGC" ;
  rdfs:isDefinedBy :Package_CIMEnumerations ;
  uml:id "EAID_9B681FE4_4EFB_4189_8B15_04468E5A4E44" .

cim:GeneratorControlSource.onAGC a cim:GeneratorControlSource ;
  rdfs:label "onAGC" ;
  rdfs:isDefinedBy :Package_CIMEnumerations ;
  uml:id "EAID_BC2966CC_CA2E_4bc9_B468_0A57C6ACB21D" .

cim:GeneratorControlSource.plantControl a cim:GeneratorControlSource ;
  rdfs:label "plantControl" ;
  rdfs:isDefinedBy :Package_CIMEnumerations ;
  uml:id "EAID_81877073_0748_4220_B78E_718AA49C7C7D" .

cim:GeneratorControlSource.unavailable a cim:GeneratorControlSource ;
  rdfs:label "unavailable" ;
  rdfs:isDefinedBy :Package_CIMEnumerations ;
  uml:id "EAID_CBE18143_8ADE_4074_906E_6157C49E8F73" .

cim:HydroPlantStorageKind.pumpedStorage a cim:HydroPlantStorageKind ;
  rdfs:label "pumpedStorage" ;
  rdfs:comment "Pumped storage."@en ;
  rdfs:isDefinedBy :Package_CIMEnumerations ;
  uml:id "EAID_02F84625_D5BF_466e_A802_4B000C3FEA03" .

cim:HydroPlantStorageKind.runOfRiver a cim:HydroPlantStorageKind ;
  rdfs:label "runOfRiver" ;
  rdfs:comment "Run of river."@en ;
  rdfs:isDefinedBy :Package_CIMEnumerations ;
  uml:id "EAID_D976AA49_42B9_456a_9FC9_4DB3058DCD4D" .

cim:HydroPlantStorageKind.storage a cim:HydroPlantStorageKind ;
  rdfs:label "storage" ;
  rdfs:comment "Storage."@en ;
  rdfs:isDefinedBy :Package_CIMEnumerations ;
  uml:id "EAID_2BE1561B_3DF2_41d7_BD06_39C870998D6E" .

cim:Impedance a rdfs:Datatype ;
  rdfs:label "Impedance" ;
  rdfs:comment "Ratio of voltage to current."@en ;
  owl:equivalentClass xsd:float ;
  rdfs:isDefinedBy :Package_CIMDataTypes ;
  uml:hasMultiplier "none" ;
  uml:hasStereotype uml:cimdatatype ;
  uml:hasUnits "ohm" ;
  uml:id "EAID_4BA91B36_C874_42f0_BC71_222AFD772FE6" .

cim:Inductance a rdfs:Datatype ;
  rdfs:label "Inductance" ;
  rdfs:comment "Inductance."@en ;
  owl:equivalentClass xsd:float ;
  rdfs:isDefinedBy :Package_CIMDataTypes ;
  uml:hasMultiplier "none" ;
  uml:hasStereotype uml:cimdatatype ;
  uml:hasUnits "H" ;
  uml:id "EAID_2DAF36DA_B9EC_4a29_AF09_6CF5F22E0F39" .

cim:KiloActivePower a rdfs:Datatype ;
  rdfs:label "KiloActivePower" ;
  rdfs:comment "Active power in kilowatts."@en ;
  owl:equivalentClass xsd:float ;
  rdfs:isDefinedBy :Package_CIMDataTypes ;
  uml:hasMultiplier "k" ;
  uml:hasStereotype uml:cimdatatype ;
  uml:hasUnits "W" ;
  uml:id "EAID_9DA985D0_F816_45e4_B16D_1C9443499FC4" .

cim:Length a rdfs:Datatype ;
  rdfs:label "Length" ;
  rdfs:comment "Unit of length."@en ;
  owl:equivalentClass xsd:float ;
  rdfs:isDefinedBy :Package_CIMDataTypes ;
  uml:hasMultiplier "none" ;
  uml:hasStereotype uml:cimdatatype ;
  uml:hasUnits "m" ;
  uml:id "EAID_3957F899_DF24_4f2b_9800_255B6433079C" .

cim:LimitTypeKind.highVoltage a cim:LimitTypeKind ;
  rdfs:label "highVoltage" ;
  rdfs:comment """Referring to the rating of the equipments, a voltage too high can lead to accelerated ageing or the destruction of the equipment.
      This limit type may or may not have duration."""@en ;
  rdfs:isDefinedBy :Package_EntsoeExtensions ;
  uml:id "EAID_A2487C52_43C7_43ca_8C3D_8118D17045FE" .

cim:LimitTypeKind.lowVoltage a cim:LimitTypeKind ;
  rdfs:label "lowVoltage" ;
  rdfs:comment """A too low voltage can disturb the normal operation of some protections and transformer equipped with on-load tap changers, electronic power devices or can affect the behaviour of the auxiliaries of generation units.
      This limit type may or may not have duration."""@en ;
  rdfs:isDefinedBy :Package_EntsoeExtensions ;
  uml:id "EAID_D8379B00_BAAB_4819_B91E_BACD2110B25C" .

cim:LimitTypeKind.patl a cim:LimitTypeKind ;
  rdfs:label "patl" ;
  rdfs:comment """The Permanent Admissible Transmission Loading (PATL) is the loading in Amps, MVA or MW that can be accepted by a network branch for an unlimited duration without any risk for the material.
      The duration attribute is not used and shall be excluded for the PATL limit type. Hence only one limit value exists for the PATL type."""@en ;
  rdfs:isDefinedBy :Package_EntsoeExtensions ;
  uml:id "EAID_516D15CE_8CA9_4d25_8FDD_F27A89E58B09" .

cim:LimitTypeKind.patlt a cim:LimitTypeKind ;
  rdfs:label "patlt" ;
  rdfs:comment "Permanent Admissible Transmission Loading Threshold  (PATLT) is a value in engineering units defined for PATL and calculated using percentage less than 100 of the PATL type intended to alert operators of an arising condition. The percentage should be given in the name of the OperationalLimitSet. The aceptableDuration is another way to express the severity of the limit."@en ;
  rdfs:isDefinedBy :Package_EntsoeExtensions ;
  uml:id "EAID_643C64D1_3C4E_49a1_B399_98811CDA33C9" .

cim:LimitTypeKind.tatl a cim:LimitTypeKind ;
  rdfs:label "tatl" ;
  rdfs:comment """Temporarily Admissible Transmission Loading (TATL) which is the loading in Amps, MVA or MW that can be accepted by a branch for a certain limited duration.
      The TATL can be defined in different ways:
      <ul>
      <li>as a fixed percentage of the PATL for a given time (for example, 115% of the PATL that can be accepted during 15 minutes),</li>
      </ul>
      <ul>
      <li>pairs of TATL type and Duration calculated for each line taking into account its particular configuration and conditions of functioning (for example, it can define a TATL acceptable during 20 minutes and another one acceptable during 10 minutes).</li>
      </ul>
      Such a definition of TATL can depend on the initial operating conditions of the network element (sag situation of a line).
      The duration attribute can be used define several TATL limit types. Hence multiple TATL limit values may exist having different durations."""@en ;
  rdfs:isDefinedBy :Package_EntsoeExtensions ;
  uml:id "EAID_372CFE1D_4098_420a_BA32_1A12D5074DD4" .

cim:LimitTypeKind.tc a cim:LimitTypeKind ;
  rdfs:label "tc" ;
  rdfs:comment """Tripping Current (TC) is the ultimate intensity without any delay. It is defined as the threshold the line will trip without any possible remedial actions.
      The tripping of the network element is ordered by protections against short circuits or by overload protections, but in any case, the activation delay of these protections is not compatible with the reaction delay of an operator (less than one minute).
      The duration is always zero and the duration attribute may be left out. Hence only one limit value exists for the TC type."""@en ;
  rdfs:isDefinedBy :Package_EntsoeExtensions ;
  uml:id "EAID_5453131E_0F2E_43ab_8AE6_76BAEAE28C73" .

cim:LimitTypeKind.tct a cim:LimitTypeKind ;
  rdfs:label "tct" ;
  rdfs:comment "Tripping Current Threshold  (TCT) is a value in engineering units defined for TC and calculated using percentage less than 100 of the TC type intended to alert operators of an arising condition. The percentage should be given in the name of the OperationalLimitSet. The aceptableDuration is another way to express the severity of the limit."@en ;
  rdfs:isDefinedBy :Package_EntsoeExtensions ;
  uml:id "EAID_BBCB79E0_9C34_4767_BB0E_DEE92D439726" .

cim:MonthDay a rdfs:Datatype ;
  rdfs:label "MonthDay" ;
  rdfs:comment "MonthDay format as \"--mm-dd\", which conforms with XSD data type gMonthDay."@en ;
  rdfs:isDefinedBy :Package_PrimitiveTypes ;
  uml:hasStereotype uml:primitive ;
  uml:id "EAID_83956FD6_B8C0_480f_AB7D_ED3C03B8124A" .

cim:OperationalLimitDirectionKind.absoluteValue a cim:OperationalLimitDirectionKind ;
  rdfs:label "absoluteValue" ;
  rdfs:comment "An absoluteValue limit means that a monitored absolute value above the limit value is a violation."@en ;
  rdfs:isDefinedBy :Package_CIMEnumerations ;
  uml:id "EAID_8E09B578_BBFF_4092_BF37_53C1F42A9429" .

cim:OperationalLimitDirectionKind.high a cim:OperationalLimitDirectionKind ;
  rdfs:label "high" ;
  rdfs:comment "High means that a monitored value above the limit value is a violation.   If applied to a terminal flow, the positive direction is into the terminal."@en ;
  rdfs:isDefinedBy :Package_CIMEnumerations ;
  uml:id "EAID_55F0B56D_2715_45fd_B494_E78450B8FE51" .

cim:OperationalLimitDirectionKind.low a cim:OperationalLimitDirectionKind ;
  rdfs:label "low" ;
  rdfs:comment "Low means a monitored value below the limit is a violation.  If applied to a terminal flow, the positive direction is into the terminal."@en ;
  rdfs:isDefinedBy :Package_CIMEnumerations ;
  uml:id "EAID_D7E34FE7_5F5F_4d22_B14A_9FB9459033A8" .

cim:OrientationKind.negative a cim:OrientationKind ;
  rdfs:label "negative" ;
  rdfs:comment "For 2D diagrams, a negative orientation gives the left-hand orientation (favoured by computer graphics displays) with X values increasing from left to right and Y values increasing from top to bottom.   This is also known as a left hand orientation."@en ;
  rdfs:isDefinedBy :Package_CIMEnumerations ;
  uml:id "EAID_83B1FCEC_F370_4286_958D_530C1B06B4A8" .

cim:OrientationKind.positive a cim:OrientationKind ;
  rdfs:label "positive" ;
  rdfs:comment "For 2D diagrams, a positive orientation will result in X values increasing from left to right and Y values increasing from bottom to top.  This is also known as a right hand orientation."@en ;
  rdfs:isDefinedBy :Package_CIMEnumerations ;
  uml:id "EAID_DE6A1FBB_1A91_41a9_8505_B6954F7E55B3" .

cim:PSREventKind.inService a cim:PSREventKind ;
  rdfs:label "inService" ;
  rdfs:comment "Power system resource state change to in service."@en ;
  rdfs:isDefinedBy :Package_CIMEnumerations ;
  uml:id "EAID_980B47DD_1501_466b_A527_889EDA30BA04" .

cim:PSREventKind.other a cim:PSREventKind ;
  rdfs:label "other" ;
  rdfs:comment "Other power system resource state change."@en ;
  rdfs:isDefinedBy :Package_CIMEnumerations ;
  uml:id "EAID_D78F1B92_633C_4d84_A16A_680AAEAC7DD4" .

cim:PSREventKind.outOfService a cim:PSREventKind ;
  rdfs:label "outOfService" ;
  rdfs:comment "Power system resource state change to out of service."@en ;
  rdfs:isDefinedBy :Package_CIMEnumerations ;
  uml:id "EAID_93ED4D01_62F2_4f61_A295_51F30E4E6350" .

cim:PSREventKind.pendingAdd a cim:PSREventKind ;
  rdfs:label "pendingAdd" ;
  rdfs:comment "Power system resource state change to pending add."@en ;
  rdfs:isDefinedBy :Package_CIMEnumerations ;
  uml:id "EAID_4F4B64B4_FE91_4811_84EE_6412E8E06917" .

cim:PSREventKind.pendingRemove a cim:PSREventKind ;
  rdfs:label "pendingRemove" ;
  rdfs:comment "Power system resource state change to pending remove."@en ;
  rdfs:isDefinedBy :Package_CIMEnumerations ;
  uml:id "EAID_0C0E4C88_6E79_459c_81B3_44111E00022C" .

cim:PSREventKind.pendingReplace a cim:PSREventKind ;
  rdfs:label "pendingReplace" ;
  rdfs:comment "Power system resource state change to pending replace."@en ;
  rdfs:isDefinedBy :Package_CIMEnumerations ;
  uml:id "EAID_9C71A044_A673_4f60_A2BE_1C5B7156E786" .

cim:PSREventKind.unknown a cim:PSREventKind ;
  rdfs:label "unknown" ;
  rdfs:comment "Unknown power system resource state change."@en ;
  rdfs:isDefinedBy :Package_CIMEnumerations ;
  uml:id "EAID_95F1E3E1_029C_458a_A504_EE84D4D543A1" .

cim:PU a rdfs:Datatype ;
  rdfs:label "PU" ;
  rdfs:comment "Per Unit - a positive or negative value referred to a defined base. Values typically range from -10 to +10."@en ;
  owl:equivalentClass xsd:float ;
  rdfs:isDefinedBy :Package_CIMDataTypes ;
  uml:hasMultiplier "none" ;
  uml:hasStereotype uml:cimdatatype ;
  uml:hasUnits "none" ;
  uml:id "EAID_B95B85BC_F780_44a7_9FA5_230945D6D405" .

cim:PerCent a rdfs:Datatype ;
  rdfs:label "PerCent" ;
  rdfs:comment "Normally 0 - 100 on a defined base"@en ;
  owl:equivalentClass xsd:float ;
  rdfs:isDefinedBy :Package_CIMDataTypes ;
  uml:hasMultiplier "none" ;
  uml:hasStereotype uml:cimdatatype ;
  uml:hasUnits "none" ;
  uml:id "EAID_7D7C80E0_6F8B_4edb_A772_B9E3A8BC10B1" .

cim:PhaseCode.A a cim:PhaseCode ;
  rdfs:label "A" ;
  rdfs:comment "Phase A."@en ;
  rdfs:isDefinedBy :Package_CIMEnumerations ;
  uml:id "EAID_DA8D8889_2672_43a0_9C5B_8B41C1685CF0" .

cim:PhaseCode.AB a cim:PhaseCode ;
  rdfs:label "AB" ;
  rdfs:comment "Phases A and B."@en ;
  rdfs:isDefinedBy :Package_CIMEnumerations ;
  uml:id "EAID_C2D378B0_1CC6_42b9_BAD1_4D0FC944338C" .

cim:PhaseCode.ABC a cim:PhaseCode ;
  rdfs:label "ABC" ;
  rdfs:comment "Phases A, B, and C."@en ;
  rdfs:isDefinedBy :Package_CIMEnumerations ;
  uml:id "EAID_1E471668_30E7_4bfa_809B_49A962CFF418" .

cim:PhaseCode.ABCN a cim:PhaseCode ;
  rdfs:label "ABCN" ;
  rdfs:comment "Phases A, B, C, and N."@en ;
  rdfs:isDefinedBy :Package_CIMEnumerations ;
  uml:id "EAID_8A6E5842_BB8C_4e01_8606_3F461DE8C5D0" .

cim:PhaseCode.ABN a cim:PhaseCode ;
  rdfs:label "ABN" ;
  rdfs:comment "Phases A, B, and neutral."@en ;
  rdfs:isDefinedBy :Package_CIMEnumerations ;
  uml:id "EAID_4B392DBC_EE18_4978_A1A7_419604B59AAD" .

cim:PhaseCode.AC a cim:PhaseCode ;
  rdfs:label "AC" ;
  rdfs:comment "Phases A and C."@en ;
  rdfs:isDefinedBy :Package_CIMEnumerations ;
  uml:id "EAID_CB0F6C14_5343_4697_91AD_586CFAF714A5" .

cim:PhaseCode.ACN a cim:PhaseCode ;
  rdfs:label "ACN" ;
  rdfs:comment "Phases A, C and neutral."@en ;
  rdfs:isDefinedBy :Package_CIMEnumerations ;
  uml:id "EAID_FABAE345_1D4E_471a_8834_6AE0B42EE2ED" .

cim:PhaseCode.AN a cim:PhaseCode ;
  rdfs:label "AN" ;
  rdfs:comment "Phases A and neutral."@en ;
  rdfs:isDefinedBy :Package_CIMEnumerations ;
  uml:id "EAID_A2322207_4C93_4111_9B2F_3AE95D68B826" .

cim:PhaseCode.B a cim:PhaseCode ;
  rdfs:label "B" ;
  rdfs:comment "Phase B."@en ;
  rdfs:isDefinedBy :Package_CIMEnumerations ;
  uml:id "EAID_FCAA2C0A_22BE_444d_BDBF_970246E69C58" .

cim:PhaseCode.BC a cim:PhaseCode ;
  rdfs:label "BC" ;
  rdfs:comment "Phases B and C."@en ;
  rdfs:isDefinedBy :Package_CIMEnumerations ;
  uml:id "EAID_D42E600C_F3C4_4230_A063_C00048897B7A" .

cim:PhaseCode.BCN a cim:PhaseCode ;
  rdfs:label "BCN" ;
  rdfs:comment "Phases B, C, and neutral."@en ;
  rdfs:isDefinedBy :Package_CIMEnumerations ;
  uml:id "EAID_FABE2547_CACC_4cd6_8351_77FA867EBE9C" .

cim:PhaseCode.BN a cim:PhaseCode ;
  rdfs:label "BN" ;
  rdfs:comment "Phases B and neutral."@en ;
  rdfs:isDefinedBy :Package_CIMEnumerations ;
  uml:id "EAID_995787A5_B742_4a0e_9466_46E63D6B5061" .

cim:PhaseCode.C a cim:PhaseCode ;
  rdfs:label "C" ;
  rdfs:comment "Phase C."@en ;
  rdfs:isDefinedBy :Package_CIMEnumerations ;
  uml:id "EAID_8611466E_A157_4815_AEC3_4AA783A3AE39" .

cim:PhaseCode.CN a cim:PhaseCode ;
  rdfs:label "CN" ;
  rdfs:comment "Phases C and neutral."@en ;
  rdfs:isDefinedBy :Package_CIMEnumerations ;
  uml:id "EAID_9B346D24_2794_4ad5_AB0F_A6807FEB2A1B" .

cim:PhaseCode.N a cim:PhaseCode ;
  rdfs:label "N" ;
  rdfs:comment "Neutral phase."@en ;
  rdfs:isDefinedBy :Package_CIMEnumerations ;
  uml:id "EAID_1CE522F3_6334_48e8_870E_ACD413EF9BC1" .

cim:PhaseCode.X a cim:PhaseCode ;
  rdfs:label "X" ;
  rdfs:comment "Unknown non-neutral phase."@en ;
  rdfs:isDefinedBy :Package_CIMEnumerations ;
  uml:id "EAID_D69AC548_42A5_4933_BA3A_92954DACD646" .

cim:PhaseCode.XN a cim:PhaseCode ;
  rdfs:label "XN" ;
  rdfs:comment "Unknown non-neutral phase plus neutral."@en ;
  rdfs:isDefinedBy :Package_CIMEnumerations ;
  uml:id "EAID_0814677D_555E_4964_BD82_04622C6CCA19" .

cim:PhaseCode.XY a cim:PhaseCode ;
  rdfs:label "XY" ;
  rdfs:comment "Two unknown non-neutral phases."@en ;
  rdfs:isDefinedBy :Package_CIMEnumerations ;
  uml:id "EAID_B223C117_334E_4d72_B952_FDB86AB35EDE" .

cim:PhaseCode.XYN a cim:PhaseCode ;
  rdfs:label "XYN" ;
  rdfs:comment "Two unknown non-neutral phases plus neutral."@en ;
  rdfs:isDefinedBy :Package_CIMEnumerations ;
  uml:id "EAID_56602A0D_B4C0_445c_B37D_E1BDA94BB926" .

cim:PhaseCode.none a cim:PhaseCode ;
  rdfs:label "none" ;
  rdfs:comment "No phases specified."@en ;
  rdfs:isDefinedBy :Package_CIMEnumerations ;
  uml:id "EAID_52D79C11_0C1C_4160_BEF7_697F7DF934C7" .

cim:PhaseCode.s1 a cim:PhaseCode ;
  rdfs:label "s1" ;
  rdfs:comment "Secondary phase 1."@en ;
  rdfs:isDefinedBy :Package_CIMEnumerations ;
  uml:id "EAID_C49EC80B_B8C4_4c15_A8DF_EBEFCA1F71E3" .

cim:PhaseCode.s12 a cim:PhaseCode ;
  rdfs:label "s12" ;
  rdfs:comment "Secondary phase 1 and 2."@en ;
  rdfs:isDefinedBy :Package_CIMEnumerations ;
  uml:id "EAID_363287F6_BC54_477b_A9B5_99C64490742C" .

cim:PhaseCode.s12N a cim:PhaseCode ;
  rdfs:label "s12N" ;
  rdfs:comment "Secondary phases 1, 2, and neutral."@en ;
  rdfs:isDefinedBy :Package_CIMEnumerations ;
  uml:id "EAID_D2B0CAFC_BDB5_413b_910B_79C398C4F267" .

cim:PhaseCode.s1N a cim:PhaseCode ;
  rdfs:label "s1N" ;
  rdfs:comment "Secondary phase 1 and neutral."@en ;
  rdfs:isDefinedBy :Package_CIMEnumerations ;
  uml:id "EAID_BF0EA903_4E83_438b_8B23_85939CB1FC35" .

cim:PhaseCode.s2 a cim:PhaseCode ;
  rdfs:label "s2" ;
  rdfs:comment "Secondary phase 2."@en ;
  rdfs:isDefinedBy :Package_CIMEnumerations ;
  uml:id "EAID_C98B6AF7_876C_462c_A09F_07F3A44EBE0D" .

cim:PhaseCode.s2N a cim:PhaseCode ;
  rdfs:label "s2N" ;
  rdfs:comment "Secondary phase 2 and neutral."@en ;
  rdfs:isDefinedBy :Package_CIMEnumerations ;
  uml:id "EAID_B859D225_16B7_4cf4_B648_30154EB4E959" .

cim:RE_UnitMultiplier.G a cim:RE_UnitMultiplier ;
  rdfs:label "G" ;
  rdfs:comment "Giga 10**9"@en ;
  rdfs:isDefinedBy :Package_CIMEnumerations ;
  uml:id "EAID_CD30195D_01AD_4731_BC64_4DAB4FEB34C2" .

cim:RE_UnitMultiplier.M a cim:RE_UnitMultiplier ;
  rdfs:label "M" ;
  rdfs:comment "Mega 10**6"@en ;
  rdfs:isDefinedBy :Package_CIMEnumerations ;
  uml:id "EAID_3D4E19C6_4FA3_417a_9A64_58F651496443" .

cim:RE_UnitMultiplier.T a cim:RE_UnitMultiplier ;
  rdfs:label "T" ;
  rdfs:comment "Tera 10**12"@en ;
  rdfs:isDefinedBy :Package_CIMEnumerations ;
  uml:id "EAID_6441E4ED_2DB7_4bf9_9947_F7BBF541CDE2" .

cim:RE_UnitMultiplier.c a cim:RE_UnitMultiplier ;
  rdfs:label "c" ;
  rdfs:comment "Centi 10**-2"@en ;
  rdfs:isDefinedBy :Package_CIMEnumerations ;
  uml:id "EAID_33523CA1_9FBB_4dda_A41F_8CCD01A705E3" .

cim:RE_UnitMultiplier.d a cim:RE_UnitMultiplier ;
  rdfs:label "d" ;
  rdfs:comment "Deci 10**-1"@en ;
  rdfs:isDefinedBy :Package_CIMEnumerations ;
  uml:id "EAID_2C6B01E8_EE7F_47b4_B17A_D52718E9FDB5" .

cim:RE_UnitMultiplier.k a cim:RE_UnitMultiplier ;
  rdfs:label "k" ;
  rdfs:comment "Kilo 10**3"@en ;
  rdfs:isDefinedBy :Package_CIMEnumerations ;
  uml:id "EAID_FC3463E2_B7B7_42df_ADC4_0DDCB4417F47" .

cim:RE_UnitMultiplier.m a cim:RE_UnitMultiplier ;
  rdfs:label "m" ;
  rdfs:comment "Milli 10**-3"@en ;
  rdfs:isDefinedBy :Package_CIMEnumerations ;
  uml:id "EAID_333CE2A7_BC1E_48f5_8955_8705073ABD46" .

cim:RE_UnitMultiplier.micro a cim:RE_UnitMultiplier ;
  rdfs:label "micro" ;
  rdfs:comment "Micro 10**-6"@en ;
  rdfs:isDefinedBy :Package_CIMEnumerations ;
  uml:id "EAID_D5C77816_5F76_44ca_AE11_4404B1C626CE" .

cim:RE_UnitMultiplier.n a cim:RE_UnitMultiplier ;
  rdfs:label "n" ;
  rdfs:comment "Nano 10**-9"@en ;
  rdfs:isDefinedBy :Package_CIMEnumerations ;
  uml:id "EAID_A51AD183_AF2F_4128_95DB_53F4363F6E20" .

cim:RE_UnitMultiplier.none a cim:RE_UnitMultiplier ;
  rdfs:label "none" ;
  rdfs:isDefinedBy :Package_CIMEnumerations ;
  uml:id "EAID_3C34E45A_34BC_4055_8DB3_552E3F1DB230" .

cim:RE_UnitMultiplier.p a cim:RE_UnitMultiplier ;
  rdfs:label "p" ;
  rdfs:comment "Pico 10**-12"@en ;
  rdfs:isDefinedBy :Package_CIMEnumerations ;
  uml:id "EAID_DCAC6BAA_8A53_441b_AB8E_7211863F9C0B" .

cim:RE_UnitSymbol.A a cim:RE_UnitSymbol ;
  rdfs:label "A" ;
  rdfs:comment "Current in ampere"@en ;
  rdfs:isDefinedBy :Package_CIMEnumerations ;
  uml:id "EAID_1D066952_C39F_4ab3_A500_001D3487B377" .

cim:RE_UnitSymbol.F a cim:RE_UnitSymbol ;
  rdfs:label "F" ;
  rdfs:comment "Capacitance in farad"@en ;
  rdfs:isDefinedBy :Package_CIMEnumerations ;
  uml:id "EAID_9C4F2B00_7A94_47f1_AE53_8D57669E9234" .

cim:RE_UnitSymbol.H a cim:RE_UnitSymbol ;
  rdfs:label "H" ;
  rdfs:comment "Inductance in henry"@en ;
  rdfs:isDefinedBy :Package_CIMEnumerations ;
  uml:id "EAID_349F9A6B_85C9_48ef_A9A4_2178DCA64AAF" .

cim:RE_UnitSymbol.Hz a cim:RE_UnitSymbol ;
  rdfs:label "Hz" ;
  rdfs:comment "Frequency in hertz"@en ;
  rdfs:isDefinedBy :Package_CIMEnumerations ;
  uml:id "EAID_58CA784B_0269_4106_97FA_F5EB062AFFB9" .

cim:RE_UnitSymbol.J a cim:RE_UnitSymbol ;
  rdfs:label "J" ;
  rdfs:comment "Energy in joule"@en ;
  rdfs:isDefinedBy :Package_CIMEnumerations ;
  uml:id "EAID_C7326BBD_7290_481f_9500_1C58C3A0681F" .

cim:RE_UnitSymbol.N a cim:RE_UnitSymbol ;
  rdfs:label "N" ;
  rdfs:comment "Force in newton"@en ;
  rdfs:isDefinedBy :Package_CIMEnumerations ;
  uml:id "EAID_EB9F7450_2A34_41ad_A957_198C340CB7EC" .

cim:RE_UnitSymbol.Pa a cim:RE_UnitSymbol ;
  rdfs:label "Pa" ;
  rdfs:comment "Pressure in pascal (n/m2)"@en ;
  rdfs:isDefinedBy :Package_CIMEnumerations ;
  uml:id "EAID_8EE37224_377D_4e72_8043_C3FC38B2E352" .

cim:RE_UnitSymbol.S a cim:RE_UnitSymbol ;
  rdfs:label "S" ;
  rdfs:comment "Conductance in siemens"@en ;
  rdfs:isDefinedBy :Package_CIMEnumerations ;
  uml:id "EAID_330922ED_3925_477b_BFAF_D7535B654A0F" .

cim:RE_UnitSymbol.V a cim:RE_UnitSymbol ;
  rdfs:label "V" ;
  rdfs:comment "Voltage in volt"@en ;
  rdfs:isDefinedBy :Package_CIMEnumerations ;
  uml:id "EAID_C6839724_BD18_4045_A3BA_A580EC9F9B4B" .

cim:RE_UnitSymbol.VA a cim:RE_UnitSymbol ;
  rdfs:label "VA" ;
  rdfs:comment "Apparent power in volt ampere"@en ;
  rdfs:isDefinedBy :Package_CIMEnumerations ;
  uml:id "EAID_7A46A41D_3A37_4a42_A6AA_BF9BD2164E23" .

cim:RE_UnitSymbol.VAh a cim:RE_UnitSymbol ;
  rdfs:label "VAh" ;
  rdfs:comment "Apparent energy in volt ampere hours"@en ;
  rdfs:isDefinedBy :Package_CIMEnumerations ;
  uml:id "EAID_A0E46D67_DAE3_41dd_8BBE_1E0EE42F37EE" .

cim:RE_UnitSymbol.VAr a cim:RE_UnitSymbol ;
  rdfs:label "VAr" ;
  rdfs:comment "Reactive power in volt ampere reactive"@en ;
  rdfs:isDefinedBy :Package_CIMEnumerations ;
  uml:id "EAID_4E613429_EDA8_4115_94A0_B010172B04AE" .

cim:RE_UnitSymbol.VArh a cim:RE_UnitSymbol ;
  rdfs:label "VArh" ;
  rdfs:comment "Reactive energy in volt ampere reactive hours"@en ;
  rdfs:isDefinedBy :Package_CIMEnumerations ;
  uml:id "EAID_226C8BBE_FE49_4fdb_AC07_CA17B1C461AE" .

cim:RE_UnitSymbol.W a cim:RE_UnitSymbol ;
  rdfs:label "W" ;
  rdfs:comment "Active power in watt"@en ;
  rdfs:isDefinedBy :Package_CIMEnumerations ;
  uml:id "EAID_09BD8937_7E80_460f_9AC6_5B2BF8ADC9D5" .

cim:RE_UnitSymbol.Wh a cim:RE_UnitSymbol ;
  rdfs:label "Wh" ;
  rdfs:comment "Real energy in what hours"@en ;
  rdfs:isDefinedBy :Package_CIMEnumerations ;
  uml:id "EAID_64930AB6_FB66_4c1e_9917_F90C9526314A" .

cim:RE_UnitSymbol.deg a cim:RE_UnitSymbol ;
  rdfs:label "deg" ;
  rdfs:comment "Plane angle in degrees"@en ;
  rdfs:isDefinedBy :Package_CIMEnumerations ;
  uml:id "EAID_8ECA4E7A_9070_4265_9505_97D3146376BB" .

cim:RE_UnitSymbol.degC a cim:RE_UnitSymbol ;
  rdfs:label "degC" ;
  rdfs:comment "Relative temperature in degrees Celsius. In the SI unit system the symbol is ï¿½C. Electric charge is measured in coulomb that has the unit symbol C. To destinguish degree Celsius form coulomb the symbol used in the UML is degC. Reason for not using ï¿½C is the special character ï¿½ is difficult to manage in software."@en ;
  rdfs:isDefinedBy :Package_CIMEnumerations ;
  uml:id "EAID_EF2C967F_E4D4_4656_9A21_9267BDC24BCA" .

cim:RE_UnitSymbol.g a cim:RE_UnitSymbol ;
  rdfs:label "g" ;
  rdfs:comment "Mass in gram"@en ;
  rdfs:isDefinedBy :Package_CIMEnumerations ;
  uml:id "EAID_424CCF55_3D24_473a_82EC_A0446E2CA414" .

cim:RE_UnitSymbol.h a cim:RE_UnitSymbol ;
  rdfs:label "h" ;
  rdfs:comment "Time in hours"@en ;
  rdfs:isDefinedBy :Package_CIMEnumerations ;
  uml:id "EAID_96F30304_0F6F_4598_9929_9A4CECF6E22D" .

cim:RE_UnitSymbol.m a cim:RE_UnitSymbol ;
  rdfs:label "m" ;
  rdfs:comment "Length in meter"@en ;
  rdfs:isDefinedBy :Package_CIMEnumerations ;
  uml:id "EAID_D8A30C24_5F82_48f4_B86A_890D5C2F30A3" .

cim:RE_UnitSymbol.m2 a cim:RE_UnitSymbol ;
  rdfs:label "m2" ;
  rdfs:comment "Area in square meters"@en ;
  rdfs:isDefinedBy :Package_CIMEnumerations ;
  uml:id "EAID_9BBE63B4_C05B_4566_A763_263D08546340" .

cim:RE_UnitSymbol.m3 a cim:RE_UnitSymbol ;
  rdfs:label "m3" ;
  rdfs:comment "Volume in cubic meters"@en ;
  rdfs:isDefinedBy :Package_CIMEnumerations ;
  uml:id "EAID_EE9B9D81_A019_4894_99C6_C5632D448263" .

cim:RE_UnitSymbol.min a cim:RE_UnitSymbol ;
  rdfs:label "min" ;
  rdfs:comment "Time in minutes"@en ;
  rdfs:isDefinedBy :Package_CIMEnumerations ;
  uml:id "EAID_52EB81C6_1328_4835_9811_63F87A239CA5" .

cim:RE_UnitSymbol.none a cim:RE_UnitSymbol ;
  rdfs:label "none" ;
  rdfs:comment "Dimension less quantity, e.g. count, per unit, etc."@en ;
  rdfs:isDefinedBy :Package_CIMEnumerations ;
  uml:id "EAID_EA1B87C1_2C08_4775_90E8_00D871C9ADD3" .

cim:RE_UnitSymbol.ohm a cim:RE_UnitSymbol ;
  rdfs:label "ohm" ;
  rdfs:comment "Resistance in ohm"@en ;
  rdfs:isDefinedBy :Package_CIMEnumerations ;
  uml:id "EAID_6AE6208E_8576_47c0_A9DD_4AD4BC7C09C3" .

cim:RE_UnitSymbol.rad a cim:RE_UnitSymbol ;
  rdfs:label "rad" ;
  rdfs:comment "Plane angle in radians"@en ;
  rdfs:isDefinedBy :Package_CIMEnumerations ;
  uml:id "EAID_802E57FC_3F95_4304_A50B_3AA26E56E9A2" .

cim:RE_UnitSymbol.s a cim:RE_UnitSymbol ;
  rdfs:label "s" ;
  rdfs:comment "Time in seconds"@en ;
  rdfs:isDefinedBy :Package_CIMEnumerations ;
  uml:id "EAID_714C8194_3A05_407f_89EA_EA3D5568BD7A" .

cim:Reactance a rdfs:Datatype ;
  rdfs:label "Reactance" ;
  rdfs:comment "Reactance (imaginary part of impedance), at rated frequency."@en ;
  owl:equivalentClass xsd:float ;
  rdfs:isDefinedBy :Package_CIMDataTypes ;
  uml:hasMultiplier "none" ;
  uml:hasStereotype uml:cimdatatype ;
  uml:hasUnits "ohm" ;
  uml:id "EAID_E6647C55_B9C1_4641_96F0_A37531B351F8" .

cim:ReactancePerLength a rdfs:Datatype ;
  rdfs:label "ReactancePerLength" ;
  rdfs:comment "Reactance (imaginary part of impedance) per unit of length, at rated frequency."@en ;
  owl:equivalentClass xsd:float ;
  rdfs:isDefinedBy :Package_CIMDataTypes ;
  uml:hasMultiplier "none" ;
  uml:hasStereotype uml:cimdatatype ;
  uml:hasUnits "ohmPerm" ;
  uml:id "EAID_A7E9997F_4062_4cea_9A9B_9E8616B1B10B" .

cim:ReactivePower a rdfs:Datatype ;
  rdfs:label "ReactivePower" ;
  rdfs:comment "Product of RMS value of the voltage and the RMS value of the quadrature component of the current."@en ;
  owl:equivalentClass xsd:float ;
  rdfs:isDefinedBy :Package_CIMDataTypes ;
  uml:hasMultiplier "M" ;
  uml:hasStereotype uml:cimdatatype ;
  uml:hasUnits "VAr" ;
  uml:id "EAID_CC96E5EA_D0AB_40e4_B38C_0AFD3AC137A2" .

cim:RegulatingControlModeKind.activePower a cim:RegulatingControlModeKind ;
  rdfs:label "activePower" ;
  rdfs:comment "Active power is specified."@en ;
  rdfs:isDefinedBy :Package_CIMEnumerations ;
  uml:id "EAID_3A242210_5241_4aee_BDCC_B2EEC46D7526" .

cim:RegulatingControlModeKind.admittance a cim:RegulatingControlModeKind ;
  rdfs:label "admittance" ;
  rdfs:comment "Admittance is specified."@en ;
  rdfs:isDefinedBy :Package_CIMEnumerations ;
  uml:id "EAID_CC9BFCC8_FD49_4d34_8C86_6AB669472FBB" .

cim:RegulatingControlModeKind.currentFlow a cim:RegulatingControlModeKind ;
  rdfs:label "currentFlow" ;
  rdfs:comment "Current flow is specified."@en ;
  rdfs:isDefinedBy :Package_CIMEnumerations ;
  uml:id "EAID_DA6E8D1B_AAAB_443b_9D74_3CFD4D3CF2F7" .

cim:RegulatingControlModeKind.powerFactor a cim:RegulatingControlModeKind ;
  rdfs:label "powerFactor" ;
  rdfs:comment "Power factor is specified."@en ;
  rdfs:isDefinedBy :Package_CIMEnumerations ;
  uml:id "EAID_BBDBB729_3252_48bf_9021_4F9C7B27DABE" .

cim:RegulatingControlModeKind.reactivePower a cim:RegulatingControlModeKind ;
  rdfs:label "reactivePower" ;
  rdfs:comment "Reactive power is specified."@en ;
  rdfs:isDefinedBy :Package_CIMEnumerations ;
  uml:id "EAID_8F976702_2290_4ecc_8CC2_15D5D9E2B5C8" .

cim:RegulatingControlModeKind.temperature a cim:RegulatingControlModeKind ;
  rdfs:label "temperature" ;
  rdfs:comment "Control switches on/off based on the local temperature (i.e., a thermostat)."@en ;
  rdfs:isDefinedBy :Package_CIMEnumerations ;
  uml:id "EAID_ECDE8AEF_767A_4271_BC3E_9BCF890AC483" .

cim:RegulatingControlModeKind.timeScheduled a cim:RegulatingControlModeKind ;
  rdfs:label "timeScheduled" ;
  rdfs:comment "Control switches on/off by time of day. The times may change on the weekend, or in different seasons."@en ;
  rdfs:isDefinedBy :Package_CIMEnumerations ;
  uml:id "EAID_1F1704CF_ED40_4818_9990_F2DF43E570DC" .

cim:RegulatingControlModeKind.voltage a cim:RegulatingControlModeKind ;
  rdfs:label "voltage" ;
  rdfs:comment "Voltage is specified."@en ;
  rdfs:isDefinedBy :Package_CIMEnumerations ;
  uml:id "EAID_503A9670_BF42_4f3f_9B69_A219D154073D" .

cim:Resistance a rdfs:Datatype ;
  rdfs:label "Resistance" ;
  rdfs:comment "Resistance (real part of impedance)."@en ;
  owl:equivalentClass xsd:float ;
  rdfs:isDefinedBy :Package_CIMDataTypes ;
  uml:hasMultiplier "none" ;
  uml:hasStereotype uml:cimdatatype ;
  uml:hasUnits "ohm" ;
  uml:id "EAID_FA3E94AC_639D_4c8b_AB87_191BFC0FF0D9" .

cim:ResistancePerLength a rdfs:Datatype ;
  rdfs:label "ResistancePerLength" ;
  rdfs:comment "Resistance (real part of impedance) per unit of length."@en ;
  owl:equivalentClass xsd:float ;
  rdfs:isDefinedBy :Package_CIMDataTypes ;
  uml:hasMultiplier "none" ;
  uml:hasStereotype uml:cimdatatype ;
  uml:hasUnits "ohmPerm" ;
  uml:id "EAID_6C1F662A_01FC_4ac9_9E3C_79831BA6475C" .

cim:Seconds a rdfs:Datatype ;
  rdfs:label "Seconds" ;
  rdfs:comment "Time, in seconds"@en ;
  owl:equivalentClass xsd:float ;
  rdfs:isDefinedBy :Package_CIMDataTypes ;
  uml:hasMultiplier "none" ;
  uml:hasStereotype uml:cimdatatype ;
  uml:hasUnits "s" ;
  uml:id "EAID_A31852A6_6FB6_42f5_89BE_1436C133DF02" .

cim:SinglePhaseKind.A a cim:SinglePhaseKind ;
  rdfs:label "A" ;
  rdfs:comment "Phase A."@en ;
  rdfs:isDefinedBy :Package_CIMEnumerations ;
  uml:id "EAID_DB6D14A1_A992_40c2_9ADC_98E77A562976" .

cim:SinglePhaseKind.B a cim:SinglePhaseKind ;
  rdfs:label "B" ;
  rdfs:comment "Phase B."@en ;
  rdfs:isDefinedBy :Package_CIMEnumerations ;
  uml:id "EAID_9201A3D3_AED5_4e24_B6B9_DADA199BEB44" .

cim:SinglePhaseKind.C a cim:SinglePhaseKind ;
  rdfs:label "C" ;
  rdfs:comment "Phase C."@en ;
  rdfs:isDefinedBy :Package_CIMEnumerations ;
  uml:id "EAID_A16526E7_12C4_459f_AEFB_BF71DBA05A20" .

cim:SinglePhaseKind.N a cim:SinglePhaseKind ;
  rdfs:label "N" ;
  rdfs:comment "Neutral."@en ;
  rdfs:isDefinedBy :Package_CIMEnumerations ;
  uml:id "EAID_15D88944_D797_4fb7_B472_9B08783989DD" .

cim:SinglePhaseKind.s1 a cim:SinglePhaseKind ;
  rdfs:label "s1" ;
  rdfs:comment "Secondary phase 1."@en ;
  rdfs:isDefinedBy :Package_CIMEnumerations ;
  uml:id "EAID_2A8A3118_9520_451a_B36F_9FDA42EED05D" .

cim:SinglePhaseKind.s2 a cim:SinglePhaseKind ;
  rdfs:label "s2" ;
  rdfs:comment "Secondary phase 2."@en ;
  rdfs:isDefinedBy :Package_CIMEnumerations ;
  uml:id "EAID_A309AF87_34D9_4666_88BF_E181D87835CA" .

cim:Source.DEFAULTED a cim:Source ;
  rdfs:label "DEFAULTED" ;
  rdfs:comment "The value contains a default value."@en ;
  rdfs:isDefinedBy :Package_CIMEnumerations ;
  uml:id "EAID_370C51F9_6A1C_46d9_8249_B180DC1C8B19" .

cim:Source.PROCESS a cim:Source ;
  rdfs:label "PROCESS" ;
  rdfs:comment "The value is provided by input from the process I/O or being calculated from some function."@en ;
  rdfs:isDefinedBy :Package_CIMEnumerations ;
  uml:id "EAID_C84C8FE1_DD0B_4ad1_9029_FD7E5B67FC32" .

cim:Source.SUBSTITUTED a cim:Source ;
  rdfs:label "SUBSTITUTED" ;
  rdfs:comment "The value is provided by input of an operator or by an automatic source."@en ;
  rdfs:isDefinedBy :Package_CIMEnumerations ;
  uml:id "EAID_F4E73941_BB66_4305_9EA8_B143906FA010" .

cim:Susceptance a rdfs:Datatype ;
  rdfs:label "Susceptance" ;
  rdfs:comment "Imaginary part of admittance."@en ;
  owl:equivalentClass xsd:float ;
  rdfs:isDefinedBy :Package_CIMDataTypes ;
  uml:hasMultiplier "none" ;
  uml:hasStereotype uml:cimdatatype ;
  uml:hasUnits "S" ;
  uml:id "EAID_103215C2_533F_402a_8F81_CC945A4D81E2" .

cim:SusceptancePerLength a rdfs:Datatype ;
  rdfs:label "SusceptancePerLength" ;
  rdfs:comment "Imaginary part of admittance per unit of length."@en ;
  owl:equivalentClass xsd:float ;
  rdfs:isDefinedBy :Package_CIMDataTypes ;
  uml:hasMultiplier "none" ;
  uml:hasStereotype uml:cimdatatype ;
  uml:hasUnits "SPerm" ;
  uml:id "EAID_71A6BB9C_53CC_488a_A79F_CCA69267D61E" .

cim:SynchronousMachineKind.condenser a cim:SynchronousMachineKind ;
  rdfs:label "condenser" ;
  rdfs:isDefinedBy :Package_CIMEnumerations ;
  uml:id "EAID_00750BBA_4AD4_4e59_BCF9_83D1E5C5CB86" .

cim:SynchronousMachineKind.generator a cim:SynchronousMachineKind ;
  rdfs:label "generator" ;
  rdfs:isDefinedBy :Package_CIMEnumerations ;
  uml:id "EAID_627E55C1_C38A_4dbc_8F56_DCFE8AC55DDE" .

cim:SynchronousMachineKind.generatorOrCondenser a cim:SynchronousMachineKind ;
  rdfs:label "generatorOrCondenser" ;
  rdfs:isDefinedBy :Package_CIMEnumerations ;
  uml:id "EAID_D97A2F0C_8961_44a5_889D_1A5184FB8877" .

cim:SynchronousMachineKind.generatorOrCondenserOrMotor a cim:SynchronousMachineKind ;
  rdfs:label "generatorOrCondenserOrMotor" ;
  rdfs:isDefinedBy :Package_CIMEnumerations ;
  uml:id "EAID_F2DA14F7_3AEA_40ce_A8B0_1D48A1BB0C33" .

cim:SynchronousMachineKind.generatorOrMotor a cim:SynchronousMachineKind ;
  rdfs:label "generatorOrMotor" ;
  rdfs:isDefinedBy :Package_CIMEnumerations ;
  uml:id "EAID_3B8665CF_C9C2_406b_ABC7_F422D211FD74" .

cim:SynchronousMachineKind.motor a cim:SynchronousMachineKind ;
  rdfs:label "motor" ;
  rdfs:isDefinedBy :Package_CIMEnumerations ;
  uml:id "EAID_D5DD2C3F_51DB_422d_A374_37E1E485FFBB" .

cim:SynchronousMachineKind.motorOrCondenser a cim:SynchronousMachineKind ;
  rdfs:label "motorOrCondenser" ;
  rdfs:isDefinedBy :Package_CIMEnumerations ;
  uml:id "EAID_E375A69E_0415_4f6d_A3F0_054109E5F696" .

cim:SynchronousMachineOperatingMode.condenser a cim:SynchronousMachineOperatingMode ;
  rdfs:label "condenser" ;
  rdfs:isDefinedBy :Package_CIMEnumerations ;
  uml:id "EAID_6F8D9A9E_FDB1_4008_B152_034D447C1B16" .

cim:SynchronousMachineOperatingMode.generator a cim:SynchronousMachineOperatingMode ;
  rdfs:label "generator" ;
  rdfs:isDefinedBy :Package_CIMEnumerations ;
  uml:id "EAID_A7C24167_4F73_4f82_8EFC_C047BE2B1A89" .

cim:SynchronousMachineOperatingMode.motor a cim:SynchronousMachineOperatingMode ;
  rdfs:label "motor" ;
  rdfs:isDefinedBy :Package_CIMEnumerations ;
  uml:id "EAID_65FD9F19_65B2_4654_93EA_F3FEA630C765" .

cim:Temperature a rdfs:Datatype ;
  rdfs:label "Temperature" ;
  rdfs:comment "Value of temperature in degrees Celsius."@en ;
  owl:equivalentClass xsd:float ;
  rdfs:isDefinedBy :Package_CIMDataTypes ;
  uml:hasMultiplier "none" ;
  uml:hasStereotype uml:cimdatatype ;
  uml:hasUnits "degC" ;
  uml:id "EAID_93052F5B_A392_42f6_AD2B_BBD13DD080B6" .

cim:TransformerControlMode.reactive a cim:TransformerControlMode ;
  rdfs:label "reactive" ;
  rdfs:comment "Reactive power flow control"@en ;
  rdfs:isDefinedBy :Package_CIMEnumerations ;
  uml:id "EAID_F76A9BEF_6CA9_4073_BF18_10F8A39A3C54" .

cim:TransformerControlMode.volt a cim:TransformerControlMode ;
  rdfs:label "volt" ;
  rdfs:comment "Voltage control"@en ;
  rdfs:isDefinedBy :Package_CIMEnumerations ;
  uml:id "EAID_46309B1F_4C1C_468a_9D9A_CC189525BBFA" .

cim:UnitMultiplier.E a cim:UnitMultiplier ;
  rdfs:label "E" ;
  rdfs:comment "Exa 10**18."@en ;
  rdfs:isDefinedBy :Package_CIMEnumerations ;
  uml:id "EAID_C5C15442_BFDE_4707_9E9B_614F0960086A" .

cim:UnitMultiplier.G a cim:UnitMultiplier ;
  rdfs:label "G" ;
  rdfs:comment "Giga 10**9"@en ;
  rdfs:isDefinedBy :Package_CIMEnumerations ;
  uml:id "EAID_AFD1C533_8EFC_4ef1_86AA_320EE060BDAE" .

cim:UnitMultiplier.M a cim:UnitMultiplier ;
  rdfs:label "M" ;
  rdfs:comment "Mega 10**6"@en ;
  rdfs:isDefinedBy :Package_CIMEnumerations ;
  uml:id "EAID_E1B011DE_672C_4e2c_8FCB_9EC7FECE85B9" .

cim:UnitMultiplier.P a cim:UnitMultiplier ;
  rdfs:label "P" ;
  rdfs:comment "Peta 10**15"@en ;
  rdfs:isDefinedBy :Package_CIMEnumerations ;
  uml:id "EAID_051C3A9E_75DC_4df2_AA07_31E381BD7D51" .

cim:UnitMultiplier.T a cim:UnitMultiplier ;
  rdfs:label "T" ;
  rdfs:comment "Tera 10**12"@en ;
  rdfs:isDefinedBy :Package_CIMEnumerations ;
  uml:id "EAID_61A4565B_982A_44cb_B8E4_5DA4D5F2BDE5" .

cim:UnitMultiplier.Y a cim:UnitMultiplier ;
  rdfs:label "Y" ;
  rdfs:comment "Yotta 10**24"@en ;
  rdfs:isDefinedBy :Package_CIMEnumerations ;
  uml:id "EAID_AD5C72FE_4530_4239_A2FF_83193695B3AE" .

cim:UnitMultiplier.Z a cim:UnitMultiplier ;
  rdfs:label "Z" ;
  rdfs:comment "Zetta 10**21"@en ;
  rdfs:isDefinedBy :Package_CIMEnumerations ;
  uml:id "EAID_11BDF9ED_D8FD_431b_B0F5_77B3B4C899AC" .

cim:UnitMultiplier.a a cim:UnitMultiplier ;
  rdfs:label "a" ;
  rdfs:comment "atto 10**-18."@en ;
  rdfs:isDefinedBy :Package_CIMEnumerations ;
  uml:id "EAID_FE6505E5_A528_449e_B404_DB453AE4F04D" .

cim:UnitMultiplier.c a cim:UnitMultiplier ;
  rdfs:label "c" ;
  rdfs:comment "Centi 10**-2"@en ;
  rdfs:isDefinedBy :Package_CIMEnumerations ;
  uml:id "EAID_DD0B514D_88B5_44b2_8E1E_F38548EF1473" .

cim:UnitMultiplier.d a cim:UnitMultiplier ;
  rdfs:label "d" ;
  rdfs:comment "Deci 10**-1"@en ;
  rdfs:isDefinedBy :Package_CIMEnumerations ;
  uml:id "EAID_1D7A475A_3750_4608_936F_490FE8D92D3E" .

cim:UnitMultiplier.da a cim:UnitMultiplier ;
  rdfs:label "da" ;
  rdfs:comment "deca 10**1."@en ;
  rdfs:isDefinedBy :Package_CIMEnumerations ;
  uml:id "EAID_471A251F_92B6_4af8_9FCC_5202BD959D96" .

cim:UnitMultiplier.f a cim:UnitMultiplier ;
  rdfs:label "f" ;
  rdfs:comment "femto 10**-15."@en ;
  rdfs:isDefinedBy :Package_CIMEnumerations ;
  uml:id "EAID_AFEE121A_F906_46e1_8313_92514C1A4678" .

cim:UnitMultiplier.h a cim:UnitMultiplier ;
  rdfs:label "h" ;
  rdfs:comment "hecto 10**2."@en ;
  rdfs:isDefinedBy :Package_CIMEnumerations ;
  uml:id "EAID_65E1E0A8_6EC4_4d33_814B_865C6F119C90" .

cim:UnitMultiplier.k a cim:UnitMultiplier ;
  rdfs:label "k" ;
  rdfs:comment "Kilo 10**3"@en ;
  rdfs:isDefinedBy :Package_CIMEnumerations ;
  uml:id "EAID_E948AAE1_01BD_4043_BDB1_68635BF460F3" .

cim:UnitMultiplier.m a cim:UnitMultiplier ;
  rdfs:label "m" ;
  rdfs:comment "Milli 10**-3"@en ;
  rdfs:isDefinedBy :Package_CIMEnumerations ;
  uml:id "EAID_507BCDCB_B560_4b11_98E7_3FDB7F7FEE60" .

cim:UnitMultiplier.micro a cim:UnitMultiplier ;
  rdfs:label "micro" ;
  rdfs:comment "Micro 10**-6"@en ;
  rdfs:isDefinedBy :Package_CIMEnumerations ;
  uml:id "EAID_A240E6A3_C9CD_491c_8CF0_5F937DAF8133" .

cim:UnitMultiplier.n a cim:UnitMultiplier ;
  rdfs:label "n" ;
  rdfs:comment "Nano 10**-9"@en ;
  rdfs:isDefinedBy :Package_CIMEnumerations ;
  uml:id "EAID_002AEB7F_EFD4_4961_9EA4_10425961D0F2" .

cim:UnitMultiplier.none a cim:UnitMultiplier ;
  rdfs:label "none" ;
  rdfs:isDefinedBy :Package_CIMEnumerations ;
  uml:id "EAID_CE1AC3A2_D62E_4168_9909_E4298D28933D" .

cim:UnitMultiplier.p a cim:UnitMultiplier ;
  rdfs:label "p" ;
  rdfs:comment "Pico 10**-12"@en ;
  rdfs:isDefinedBy :Package_CIMEnumerations ;
  uml:id "EAID_816E050B_5E00_418d_A9DA_9CA703C98E30" .

cim:UnitMultiplier.y a cim:UnitMultiplier ;
  rdfs:label "y" ;
  rdfs:comment "yocto 10**-24."@en ;
  rdfs:isDefinedBy :Package_CIMEnumerations ;
  uml:id "EAID_F3FD1886_B7ED_4c9b_8747_9BD316B4E631" .

cim:UnitMultiplier.z a cim:UnitMultiplier ;
  rdfs:label "z" ;
  rdfs:comment "zepto 10**-21."@en ;
  rdfs:isDefinedBy :Package_CIMEnumerations ;
  uml:id "EAID_F2E5D8DC_AAA2_4e84_830B_C1260BAE9B3F" .

cim:UnitSymbol.A a cim:UnitSymbol ;
  rdfs:label "A" ;
  rdfs:comment "Current in Ampere."@en ;
  rdfs:isDefinedBy :Package_CIMEnumerations ;
  uml:id "EAID_73192209_46C4_4236_A93F_622B9B20B1D2" .

cim:UnitSymbol.A2 a cim:UnitSymbol ;
  rdfs:label "A2" ;
  rdfs:comment "Ampere squared (Aï¿½)."@en ;
  rdfs:isDefinedBy :Package_CIMEnumerations ;
  uml:id "EAID_18F91DF9_5F02_4fcc_8718_6F1B172B69A6" .

cim:UnitSymbol.A2h a cim:UnitSymbol ;
  rdfs:label "A2h" ;
  rdfs:comment "ampere-squared hour, Ampere-squared hour."@en ;
  rdfs:isDefinedBy :Package_CIMEnumerations ;
  uml:id "EAID_01289D24_5F6D_41ec_94BF_393D18E0BDF6" .

cim:UnitSymbol.A2s a cim:UnitSymbol ;
  rdfs:label "A2s" ;
  rdfs:comment "Ampere squared time in square ampere (Aï¿½s)."@en ;
  rdfs:isDefinedBy :Package_CIMEnumerations ;
  uml:id "EAID_EABC3521_23CB_4f06_8DF2_FCB922207D3D" .

cim:UnitSymbol.APerA a cim:UnitSymbol ;
  rdfs:label "APerA" ;
  rdfs:comment "Current, Ratio of Amperages  Note: Users may need to supply a prefix such as ï¿½mï¿½ to show rates such as ï¿½mA/Aï¿½."@en ;
  rdfs:isDefinedBy :Package_CIMEnumerations ;
  uml:id "EAID_0981015A_8462_486a_B3F8_BDE9BF366589" .

cim:UnitSymbol.APerm a cim:UnitSymbol ;
  rdfs:label "APerm" ;
  rdfs:comment "A/m, magnetic field strength, Ampere per metre."@en ;
  rdfs:isDefinedBy :Package_CIMEnumerations ;
  uml:id "EAID_D3199EFD_A62A_4880_BAD2_C8C7DBB980D3" .

cim:UnitSymbol.Ah a cim:UnitSymbol ;
  rdfs:label "Ah" ;
  rdfs:comment "Ampere-hours, Ampere-hours."@en ;
  rdfs:isDefinedBy :Package_CIMEnumerations ;
  uml:id "EAID_CE9B8EC3_3129_42df_87A0_36D042ABD54B" .

cim:UnitSymbol.As a cim:UnitSymbol ;
  rdfs:label "As" ;
  rdfs:comment "Ampere seconds (Aï¿½s)."@en ;
  rdfs:isDefinedBy :Package_CIMEnumerations ;
  uml:id "EAID_49C928A6_F4C8_4393_B349_B7C3E333DCAF" .

cim:UnitSymbol.Bq a cim:UnitSymbol ;
  rdfs:label "Bq" ;
  rdfs:comment "Radioactivity in Becquerel (1/s)."@en ;
  rdfs:isDefinedBy :Package_CIMEnumerations ;
  uml:id "EAID_30B53BA7_AE34_4baa_B893_2C10F799CFA1" .

cim:UnitSymbol.Btu a cim:UnitSymbol ;
  rdfs:label "Btu" ;
  rdfs:comment "Energy, British Thermal Unit."@en ;
  rdfs:isDefinedBy :Package_CIMEnumerations ;
  uml:id "EAID_1B4C1E78_59D4_4d29_A7A1_71CBC49EE405" .

cim:UnitSymbol.C a cim:UnitSymbol ;
  rdfs:label "C" ;
  rdfs:comment "Electric charge in Coulomb (Aï¿½s)."@en ;
  rdfs:isDefinedBy :Package_CIMEnumerations ;
  uml:id "EAID_C61A2A7C_DF02_44c5_9FC1_A47B7645816E" .

cim:UnitSymbol.CPerkg a cim:UnitSymbol ;
  rdfs:label "CPerkg" ;
  rdfs:comment "exposure (x rays), Coulomb per kilogram."@en ;
  rdfs:isDefinedBy :Package_CIMEnumerations ;
  uml:id "EAID_BE648D60_3104_4798_9AF2_ADD5F3BECC9A" .

cim:UnitSymbol.CPerm2 a cim:UnitSymbol ;
  rdfs:label "CPerm2" ;
  rdfs:comment "surface charge density, Coulomb per square metre."@en ;
  rdfs:isDefinedBy :Package_CIMEnumerations ;
  uml:id "EAID_3283D3E6_1A08_4008_BDCB_DCA8752664A4" .

cim:UnitSymbol.CPerm3 a cim:UnitSymbol ;
  rdfs:label "CPerm3" ;
  rdfs:comment "electric charge density, Coulomb per cubic metre."@en ;
  rdfs:isDefinedBy :Package_CIMEnumerations ;
  uml:id "EAID_8F77778C_0BD6_446b_B67C_10683180E189" .

cim:UnitSymbol.F a cim:UnitSymbol ;
  rdfs:label "F" ;
  rdfs:comment "Electric capacitance in Farad (C/V)."@en ;
  rdfs:isDefinedBy :Package_CIMEnumerations ;
  uml:id "EAID_D70AA740_B956_43a8_99CF_6DB3A5AA09B1" .

cim:UnitSymbol.FPerm a cim:UnitSymbol ;
  rdfs:label "FPerm" ;
  rdfs:comment "permittivity, Farad per metre."@en ;
  rdfs:isDefinedBy :Package_CIMEnumerations ;
  uml:id "EAID_C04572EA_C3F3_4517_99AE_C2CEA71B58C8" .

cim:UnitSymbol.G a cim:UnitSymbol ;
  rdfs:label "G" ;
  rdfs:comment "Magnetic flux density, Gauss (1 G = 10-4 T)."@en ;
  rdfs:isDefinedBy :Package_CIMEnumerations ;
  uml:id "EAID_FE8F4D96_0B8D_4ffb_88F9_6443451F7424" .

cim:UnitSymbol.Gy a cim:UnitSymbol ;
  rdfs:label "Gy" ;
  rdfs:comment "Absorbed dose in Gray (J/kg)."@en ;
  rdfs:isDefinedBy :Package_CIMEnumerations ;
  uml:id "EAID_8CE82932_8CA9_4160_9446_17BED2B1E815" .

cim:UnitSymbol.GyPers a cim:UnitSymbol ;
  rdfs:label "GyPers" ;
  rdfs:comment "absorbed dose rate, Gray per second."@en ;
  rdfs:isDefinedBy :Package_CIMEnumerations ;
  uml:id "EAID_78EF1199_DA54_4191_ADE0_E5D68B8F605A" .

cim:UnitSymbol.H a cim:UnitSymbol ;
  rdfs:label "H" ;
  rdfs:comment "Electric inductance in Henry (Wb/A)."@en ;
  rdfs:isDefinedBy :Package_CIMEnumerations ;
  uml:id "EAID_8040E2D3_A5E3_4bf8_B171_DC7FA9E864B9" .

cim:UnitSymbol.HPerm a cim:UnitSymbol ;
  rdfs:label "HPerm" ;
  rdfs:comment "permeability, Henry per metre."@en ;
  rdfs:isDefinedBy :Package_CIMEnumerations ;
  uml:id "EAID_0AFE859F_EC8D_4f7d_B7DA_B9770716017B" .

cim:UnitSymbol.Hz a cim:UnitSymbol ;
  rdfs:label "Hz" ;
  rdfs:comment "Frequency in Hertz (1/s)."@en ;
  rdfs:isDefinedBy :Package_CIMEnumerations ;
  uml:id "EAID_12FFE4AD_4859_47dd_A5F9_3AD564FCD8FC" .

cim:UnitSymbol.HzPerHz a cim:UnitSymbol ;
  rdfs:label "HzPerHz" ;
  rdfs:comment "Frequency, Rate of frequency change  Note: Users may need to supply a prefix such as ï¿½mï¿½ to show rates such as ï¿½mHz/Hzï¿½."@en ;
  rdfs:isDefinedBy :Package_CIMEnumerations ;
  uml:id "EAID_34F2F478_6864_4ddc_9F2E_C31BAF85AC60" .

cim:UnitSymbol.HzPers a cim:UnitSymbol ;
  rdfs:label "HzPers" ;
  rdfs:comment "Rate of change of frequency in Hertz per second."@en ;
  rdfs:isDefinedBy :Package_CIMEnumerations ;
  uml:id "EAID_AEEED7A8_50C6_4856_ACF4_A280D57EB110" .

cim:UnitSymbol.J a cim:UnitSymbol ;
  rdfs:label "J" ;
  rdfs:comment "Energy in joule (Nï¿½m = Cï¿½V = Wï¿½s)."@en ;
  rdfs:isDefinedBy :Package_CIMEnumerations ;
  uml:id "EAID_4FE8744A_7C5F_4fc7_8FFB_5B9A05F0EF19" .

cim:UnitSymbol.JPerK a cim:UnitSymbol ;
  rdfs:label "JPerK" ;
  rdfs:comment "Heat capacity in Joule/Kelvin."@en ;
  rdfs:isDefinedBy :Package_CIMEnumerations ;
  uml:id "EAID_FF36C817_7511_422c_A716_6C89E08ACBC4" .

cim:UnitSymbol.JPerkg a cim:UnitSymbol ;
  rdfs:label "JPerkg" ;
  rdfs:comment "Specific energy, Joule / kg."@en ;
  rdfs:isDefinedBy :Package_CIMEnumerations ;
  uml:id "EAID_9AF99907_30CB_43b3_91AA_CB01E39EEBA1" .

cim:UnitSymbol.JPerkgK a cim:UnitSymbol ;
  rdfs:label "JPerkgK" ;
  rdfs:comment "Specific heat capacity, specific entropy, Joule per kilogram Kelvin."@en ;
  rdfs:isDefinedBy :Package_CIMEnumerations ;
  uml:id "EAID_39ADD645_66F8_4b70_96D8_1D4EC7778020" .

cim:UnitSymbol.JPerm2 a cim:UnitSymbol ;
  rdfs:label "JPerm2" ;
  rdfs:comment "Insulation energy density, Joule per square metre or watt second per square metre."@en ;
  rdfs:isDefinedBy :Package_CIMEnumerations ;
  uml:id "EAID_212F940C_F1E4_4eaa_B1D3_5102896EEB35" .

cim:UnitSymbol.JPerm3 a cim:UnitSymbol ;
  rdfs:label "JPerm3" ;
  rdfs:comment "energy density, Joule per cubic metre."@en ;
  rdfs:isDefinedBy :Package_CIMEnumerations ;
  uml:id "EAID_3C842C47_4B64_4c2e_9427_46ADCDCE35F0" .

cim:UnitSymbol.JPermol a cim:UnitSymbol ;
  rdfs:label "JPermol" ;
  rdfs:comment "molar energy, Joule per mole."@en ;
  rdfs:isDefinedBy :Package_CIMEnumerations ;
  uml:id "EAID_353C895C_47E1_4914_B6E1_BD5BCAB94594" .

cim:UnitSymbol.JPermolK a cim:UnitSymbol ;
  rdfs:label "JPermolK" ;
  rdfs:comment "molar entropy, molar heat capacity, Joule per mole kelvin."@en ;
  rdfs:isDefinedBy :Package_CIMEnumerations ;
  uml:id "EAID_F882002C_6A67_4257_BDBE_6CCC013B9AB3" .

cim:UnitSymbol.JPers a cim:UnitSymbol ;
  rdfs:label "JPers" ;
  rdfs:comment "Energy rate joule per second (J/s),"@en ;
  rdfs:isDefinedBy :Package_CIMEnumerations ;
  uml:id "EAID_634EDCB8_AD8B_41e9_90BE_5505F97851D9" .

cim:UnitSymbol.K a cim:UnitSymbol ;
  rdfs:label "K" ;
  rdfs:comment "Temperature in Kelvin."@en ;
  rdfs:isDefinedBy :Package_CIMEnumerations ;
  uml:id "EAID_1C7019D4_4C0C_4563_BD39_4341656535C3" .

cim:UnitSymbol.KPers a cim:UnitSymbol ;
  rdfs:label "KPers" ;
  rdfs:comment "Temperature change rate in Kelvin per second."@en ;
  rdfs:isDefinedBy :Package_CIMEnumerations ;
  uml:id "EAID_9A2A4DC0_BF90_466e_B784_29EA09352F82" .

cim:UnitSymbol.M a cim:UnitSymbol ;
  rdfs:label "M" ;
  rdfs:comment "Length, nautical mile (1 M = 1852 m)."@en ;
  rdfs:isDefinedBy :Package_CIMEnumerations ;
  uml:id "EAID_968D12C1_180C_4b26_B5DF_012BD53DED80" .

cim:UnitSymbol.Mx a cim:UnitSymbol ;
  rdfs:label "Mx" ;
  rdfs:comment "Magnetic flux, Maxwell (1 Mx = 10-8 Wb)."@en ;
  rdfs:isDefinedBy :Package_CIMEnumerations ;
  uml:id "EAID_D1C8B88C_D6A3_4717_946B_867577DE8009" .

cim:UnitSymbol.N a cim:UnitSymbol ;
  rdfs:label "N" ;
  rdfs:comment "Force in Newton (kgï¿½m/sï¿½)."@en ;
  rdfs:isDefinedBy :Package_CIMEnumerations ;
  uml:id "EAID_8A741E4F_51FC_4b84_A786_4A9D8C113F9D" .

cim:UnitSymbol.NPerm a cim:UnitSymbol ;
  rdfs:label "NPerm" ;
  rdfs:comment "Surface tension, Newton per metre."@en ;
  rdfs:isDefinedBy :Package_CIMEnumerations ;
  uml:id "EAID_C4D5B098_8516_4a09_9438_021D4673AF64" .

cim:UnitSymbol.Nm a cim:UnitSymbol ;
  rdfs:label "Nm" ;
  rdfs:comment "Moment of force, Newton metre."@en ;
  rdfs:isDefinedBy :Package_CIMEnumerations ;
  uml:id "EAID_81CE58A8_CB0D_4985_95F9_AD61BF9564C2" .

cim:UnitSymbol.Oe a cim:UnitSymbol ;
  rdfs:label "Oe" ;
  rdfs:comment "Magnetic field, ï¿½rsted (1 Oe = (103/4p) A/m)."@en ;
  rdfs:isDefinedBy :Package_CIMEnumerations ;
  uml:id "EAID_B2481968_BFB0_4b4e_B558_1B5D0ECBEABA" .

cim:UnitSymbol.Pa a cim:UnitSymbol ;
  rdfs:label "Pa" ;
  rdfs:comment "Pressure in Pascal (N/mï¿½). Note: the absolute or relative measurement of pressure is implied with this entry. See below for more explicit forms."@en ;
  rdfs:isDefinedBy :Package_CIMEnumerations ;
  uml:id "EAID_91C62CD5_316C_4133_B60C_10B358D0151D" .

cim:UnitSymbol.PaPers a cim:UnitSymbol ;
  rdfs:label "PaPers" ;
  rdfs:comment "Pressure change rate in Pascal per second."@en ;
  rdfs:isDefinedBy :Package_CIMEnumerations ;
  uml:id "EAID_021658D5_DF8F_4227_ADB8_65714453802B" .

cim:UnitSymbol.Pas a cim:UnitSymbol ;
  rdfs:label "Pas" ;
  rdfs:comment "Dynamic viscosity, Pascal second."@en ;
  rdfs:isDefinedBy :Package_CIMEnumerations ;
  uml:id "EAID_D232804D_4191_48f5_B5E7_B71B50AD52DE" .

cim:UnitSymbol.Q a cim:UnitSymbol ;
  rdfs:label "Q" ;
  rdfs:comment "Quantity power, Q."@en ;
  rdfs:isDefinedBy :Package_CIMEnumerations ;
  uml:id "EAID_1BB7A76B_00E0_4d58_AD95_5DCF130E8324" .

cim:UnitSymbol.Qh a cim:UnitSymbol ;
  rdfs:label "Qh" ;
  rdfs:comment "Quantity energy, Qh."@en ;
  rdfs:isDefinedBy :Package_CIMEnumerations ;
  uml:id "EAID_1770F83A_9153_45e4_91DD_DC53260E2843" .

cim:UnitSymbol.S a cim:UnitSymbol ;
  rdfs:label "S" ;
  rdfs:comment "Conductance in Siemens."@en ;
  rdfs:isDefinedBy :Package_CIMEnumerations ;
  uml:id "EAID_957E82E6_ECC7_4bad_857B_40D8EFB98461" .

cim:UnitSymbol.SPerm a cim:UnitSymbol ;
  rdfs:label "SPerm" ;
  rdfs:comment "Conductance per length (F/m)."@en ;
  rdfs:isDefinedBy :Package_CIMEnumerations ;
  uml:id "EAID_53A6D4F2_8E3C_4abb_9F90_D3384CD9F08E" .

cim:UnitSymbol.Sv a cim:UnitSymbol ;
  rdfs:label "Sv" ;
  rdfs:comment "Dose equivalent in Sievert (J/kg)."@en ;
  rdfs:isDefinedBy :Package_CIMEnumerations ;
  uml:id "EAID_14CB198F_E1D3_4622_950B_5553B10C2852" .

cim:UnitSymbol.T a cim:UnitSymbol ;
  rdfs:label "T" ;
  rdfs:comment "Magnetic flux density in Tesla (Wb/m2)."@en ;
  rdfs:isDefinedBy :Package_CIMEnumerations ;
  uml:id "EAID_2EC7E58C_2672_45ac_B70D_B9DB36DC1BBB" .

cim:UnitSymbol.V a cim:UnitSymbol ;
  rdfs:label "V" ;
  rdfs:comment "Electric potential in Volt (W/A)."@en ;
  rdfs:isDefinedBy :Package_CIMEnumerations ;
  uml:id "EAID_3FB55A80_415D_4a6b_8A30_C75CD420B222" .

cim:UnitSymbol.V2 a cim:UnitSymbol ;
  rdfs:label "V2" ;
  rdfs:comment "Volt squared (Wï¿½/Aï¿½)."@en ;
  rdfs:isDefinedBy :Package_CIMEnumerations ;
  uml:id "EAID_F50AD8B5_9E99_41fe_BB86_CBC5CA9491B4" .

cim:UnitSymbol.V2h a cim:UnitSymbol ;
  rdfs:label "V2h" ;
  rdfs:comment "volt-squared hour, Volt-squared-hours."@en ;
  rdfs:isDefinedBy :Package_CIMEnumerations ;
  uml:id "EAID_5A34C44C_74CD_4810_B21A_FC8C343AC7C8" .

cim:UnitSymbol.VA a cim:UnitSymbol ;
  rdfs:label "VA" ;
  rdfs:comment "Apparent power in Volt Ampere (See also real power and reactive power.)"@en ;
  rdfs:isDefinedBy :Package_CIMEnumerations ;
  uml:id "EAID_D143576A_D481_4b1f_BDBD_8F388295FFAE" .

cim:UnitSymbol.VAh a cim:UnitSymbol ;
  rdfs:label "VAh" ;
  rdfs:comment "Apparent energy in Volt Ampere hours."@en ;
  rdfs:isDefinedBy :Package_CIMEnumerations ;
  uml:id "EAID_3C54998F_DB57_4682_8152_68D311DD9089" .

cim:UnitSymbol.VAr a cim:UnitSymbol ;
  rdfs:label "VAr" ;
  rdfs:comment """Reactive power in Volt Ampere reactive. The ï¿½reactiveï¿½ or ï¿½imaginaryï¿½ component of electrical power (VIsin(phi)). (See also real power and apparent power).
      Note: Different meter designs use different methods to arrive at their results. Some meters may compute reactive power as an arithmetic value, while others compute the value vectorially. The data consumer should determine the method in use and the suitability of the measurement for the intended purpose."""@en ;
  rdfs:isDefinedBy :Package_CIMEnumerations ;
  uml:id "EAID_DCEBA4F8_0358_41de_A358_F1B17E674523" .

cim:UnitSymbol.VArh a cim:UnitSymbol ;
  rdfs:label "VArh" ;
  rdfs:comment "Reactive energy in Volt Ampere reactive hours."@en ;
  rdfs:isDefinedBy :Package_CIMEnumerations ;
  uml:id "EAID_46D8AE45_E355_49a2_B804_3ADAC25E50D1" .

cim:UnitSymbol.VPerHz a cim:UnitSymbol ;
  rdfs:label "VPerHz" ;
  rdfs:comment "Magnetic flux in Volt per Hertz."@en ;
  rdfs:isDefinedBy :Package_CIMEnumerations ;
  uml:id "EAID_07982CB2_AB66_430f_81F7_89B4401DAA26" .

cim:UnitSymbol.VPerV a cim:UnitSymbol ;
  rdfs:label "VPerV" ;
  rdfs:comment "Voltage, Ratio of voltages Note: Users may need to supply a prefix such as ï¿½mï¿½ to show rates such as ï¿½mV/Vï¿½."@en ;
  rdfs:isDefinedBy :Package_CIMEnumerations ;
  uml:id "EAID_2FA931F4_B97C_4478_AA52_CB5B05B1C38A" .

cim:UnitSymbol.VPerVA a cim:UnitSymbol ;
  rdfs:label "VPerVA" ;
  rdfs:comment "Power factor, PF, the ratio of the active power to the apparent power. Note: The sign convention used for power factor will differ between IEC meters and EEI (ANSI) meters. It is assumed that the data consumers understand the type of meter being used and agree on the sign convention in use at any given utility."@en ;
  rdfs:isDefinedBy :Package_CIMEnumerations ;
  uml:id "EAID_84F0EE0E_944C_4c28_AFC7_966E1E8C6ACB" .

cim:UnitSymbol.VPerVAr a cim:UnitSymbol ;
  rdfs:label "VPerVAr" ;
  rdfs:comment "Power factor, PF, the ratio of the active power to the apparent power. Note: The sign convention used for power factor will differ between IEC meters and EEI (ANSI) meters. It is assumed that the data consumers understand the type of meter being used and agree on the sign convention in use at any given utility."@en ;
  rdfs:isDefinedBy :Package_CIMEnumerations ;
  uml:id "EAID_BD05EC25_B9FA_4e2a_A953_D23FEA80E1C8" .

cim:UnitSymbol.VPerm a cim:UnitSymbol ;
  rdfs:label "VPerm" ;
  rdfs:comment "electric field strength, Volt per metre."@en ;
  rdfs:isDefinedBy :Package_CIMEnumerations ;
  uml:id "EAID_AB063AEA_81C2_410c_B41C_B345D7F1868B" .

cim:UnitSymbol.Vh a cim:UnitSymbol ;
  rdfs:label "Vh" ;
  rdfs:comment "Volt-hour, Volt hours."@en ;
  rdfs:isDefinedBy :Package_CIMEnumerations ;
  uml:id "EAID_731A8202_1BD4_44a0_B8E7_C82A6F1B47F4" .

cim:UnitSymbol.Vs a cim:UnitSymbol ;
  rdfs:label "Vs" ;
  rdfs:comment "Volt second (Ws/A)."@en ;
  rdfs:isDefinedBy :Package_CIMEnumerations ;
  uml:id "EAID_50759FC7_EB2D_47b3_833C_7F6B1458D251" .

cim:UnitSymbol.W a cim:UnitSymbol ;
  rdfs:label "W" ;
  rdfs:comment "Real power in Watt (J/s). Electrical power may have real and reactive components. The real portion of electrical power (Iï¿½R or VIcos(phi)), is expressed in Watts. (See also apparent power and reactive power.)"@en ;
  rdfs:isDefinedBy :Package_CIMEnumerations ;
  uml:id "EAID_C160944D_C9F0_4871_9B2C_2320C1F7C1A2" .

cim:UnitSymbol.WPerA a cim:UnitSymbol ;
  rdfs:label "WPerA" ;
  rdfs:comment "Active power per current flow, watt per Ampere."@en ;
  rdfs:isDefinedBy :Package_CIMEnumerations ;
  uml:id "EAID_F55D6160_9960_4178_BB40_4BC85AFF91E5" .

cim:UnitSymbol.WPerHz a cim:UnitSymbol ;
  rdfs:label "WPerm2" ;
  rdfs:comment "Active Power Per Frequency? Watt per hertz."@en ;
  rdfs:isDefinedBy :Package_CIMEnumerations ;
  uml:id "EAID_93EAE4BB_9CE4_41e8_9730_D957269533C9" .

cim:UnitSymbol.WPerW a cim:UnitSymbol ;
  rdfs:label "WPerW" ;
  rdfs:comment "Signal Strength, Ratio of power  Note: Users may need to supply a prefix such as ï¿½mï¿½ to show rates such as ï¿½mW/Wï¿½."@en ;
  rdfs:isDefinedBy :Package_CIMEnumerations ;
  uml:id "EAID_23406637_6D26_4426_BD20_1F8B2C5AA515" .

cim:UnitSymbol.WPerm2 a cim:UnitSymbol ;
  rdfs:label "WPerm2" ;
  rdfs:comment "Heat flux density, irradiance, Watt per square metre."@en ;
  rdfs:isDefinedBy :Package_CIMEnumerations ;
  uml:id "EAID_93EAE4BB_9CE4_41e8_9730_D957269533C9" .

cim:UnitSymbol.WPerm2sr a cim:UnitSymbol ;
  rdfs:label "WPerm2sr" ;
  rdfs:comment "radiance, Watt per square metre steradian."@en ;
  rdfs:isDefinedBy :Package_CIMEnumerations ;
  uml:id "EAID_047346B8_71C8_4fda_85A2_6FE1D43D6431" .

cim:UnitSymbol.WPermK a cim:UnitSymbol ;
  rdfs:label "WPermK" ;
  rdfs:comment "Thermal conductivity in Watt/metre Kelvin."@en ;
  rdfs:isDefinedBy :Package_CIMEnumerations ;
  uml:id "EAID_86E9DE8F_B4C7_48b4_8848_6A9B854FC76C" .

cim:UnitSymbol.WPers a cim:UnitSymbol ;
  rdfs:label "WPers" ;
  rdfs:comment "Ramp rate in Watt per second."@en ;
  rdfs:isDefinedBy :Package_CIMEnumerations ;
  uml:id "EAID_F0181C52_D05F_4e50_94AA_C5D348AAF734" .

cim:UnitSymbol.WPersr a cim:UnitSymbol ;
  rdfs:label "WPersr" ;
  rdfs:comment "Radiant intensity, Watt per steradian."@en ;
  rdfs:isDefinedBy :Package_CIMEnumerations ;
  uml:id "EAID_FDF9DAF2_2C0C_4ded_A78F_9CC8068BE2D5" .

cim:UnitSymbol.Wb a cim:UnitSymbol ;
  rdfs:label "Wb" ;
  rdfs:comment "Magnetic flux in Weber (Vï¿½s)."@en ;
  rdfs:isDefinedBy :Package_CIMEnumerations ;
  uml:id "EAID_BAD96D9D_91A8_480b_B918_798774EEECBB" .

cim:UnitSymbol.Wh a cim:UnitSymbol ;
  rdfs:label "Wh" ;
  rdfs:comment "Real energy in Watt hours."@en ;
  rdfs:isDefinedBy :Package_CIMEnumerations ;
  uml:id "EAID_A239C761_B67B_4ccb_832E_F299590120AB" .

cim:UnitSymbol.anglemin a cim:UnitSymbol ;
  rdfs:label "anglemin" ;
  rdfs:comment "Plane angle, minute."@en ;
  rdfs:isDefinedBy :Package_CIMEnumerations ;
  uml:id "EAID_AE607533_42D1_4b54_8BA2_B842D9B8A5CD" .

cim:UnitSymbol.anglesec a cim:UnitSymbol ;
  rdfs:label "anglesec" ;
  rdfs:comment "Plane angle, second."@en ;
  rdfs:isDefinedBy :Package_CIMEnumerations ;
  uml:id "EAID_A9E672D6_E895_4ae8_BD5C_9216FE5D1208" .

cim:UnitSymbol.bar a cim:UnitSymbol ;
  rdfs:label "bar" ;
  rdfs:comment "Pressure, bar (1 bar = 100 kPa)."@en ;
  rdfs:isDefinedBy :Package_CIMEnumerations ;
  uml:id "EAID_FAC447D1_CA76_4824_97C8_BC02A71FABF7" .

cim:UnitSymbol.cd a cim:UnitSymbol ;
  rdfs:label "cd" ;
  rdfs:comment "Luminous intensity in candela."@en ;
  rdfs:isDefinedBy :Package_CIMEnumerations ;
  uml:id "EAID_86492824_BA54_4e78_BEA8_DF08A1519540" .

cim:UnitSymbol.charPers a cim:UnitSymbol ;
  rdfs:label "charPers" ;
  rdfs:comment "Data rate (baud) in characters per second."@en ;
  rdfs:isDefinedBy :Package_CIMEnumerations ;
  uml:id "EAID_D03D75BB_9A84_4f44_8DC1_AB7254097464" .

cim:UnitSymbol.character a cim:UnitSymbol ;
  rdfs:label "character" ;
  rdfs:comment "Number of characters."@en ;
  rdfs:isDefinedBy :Package_CIMEnumerations ;
  uml:id "EAID_8B996FC0_89EB_4157_8F63_99A18429B8A7" .

cim:UnitSymbol.cosPhi a cim:UnitSymbol ;
  rdfs:label "cosPhi" ;
  rdfs:comment """Power factor, dimensionless.
      Note 1: This definition of power factor only holds for balanced systems. See the alternative definition under code 153.
      Note 2ï¿½: Beware of differing sign conventions in use between the IEC and EEI. It is assumed that the data consumer understands the type of meter in use and the sign convention in use by the utility."""@en ;
  rdfs:isDefinedBy :Package_CIMEnumerations ;
  uml:id "EAID_9A475C35_1BB1_4d24_A1E0_61C8A0DE6542" .

cim:UnitSymbol.count a cim:UnitSymbol ;
  rdfs:label "count" ;
  rdfs:comment "Amount of substance, Counter value."@en ;
  rdfs:isDefinedBy :Package_CIMEnumerations ;
  uml:id "EAID_BFFB42D5_CAE3_49f7_9130_69385D62E5D0" .

cim:UnitSymbol.d a cim:UnitSymbol ;
  rdfs:label "d" ;
  rdfs:comment "Time, day = 24 h = 86400 s."@en ;
  rdfs:isDefinedBy :Package_CIMEnumerations ;
  uml:id "EAID_9DE425D1_8CB8_4b2e_BCDA_D9990ED74533" .

cim:UnitSymbol.dB a cim:UnitSymbol ;
  rdfs:label "dB" ;
  rdfs:comment "Sound pressure level in decibel. Note:  multiplier ï¿½dï¿½ is included in this unit symbol for compatibility with IEC 61850-7-3."@en ;
  rdfs:isDefinedBy :Package_CIMEnumerations ;
  uml:id "EAID_33CC17A0_5D8D_44e2_B72E_9668E65C3AE2" .

cim:UnitSymbol.dBm a cim:UnitSymbol ;
  rdfs:label "dBm" ;
  rdfs:comment "Power level (logrithmic ratio of signal strength , Bel-mW), normalized to 1mW. Note:  multiplier ï¿½dï¿½ is included in this unit symbol for compatibility with IEC 61850-7-3."@en ;
  rdfs:isDefinedBy :Package_CIMEnumerations ;
  uml:id "EAID_45FE77FA_3D1C_4f61_9328_44099CDB1396" .

cim:UnitSymbol.deg a cim:UnitSymbol ;
  rdfs:label "deg" ;
  rdfs:comment "Plane angle in degrees."@en ;
  rdfs:isDefinedBy :Package_CIMEnumerations ;
  uml:id "EAID_79DF68B3_CFBC_462f_BB36_9D491F5F3D83" .

cim:UnitSymbol.degC a cim:UnitSymbol ;
  rdfs:label "degC" ;
  rdfs:comment """Relative temperature in degrees Celsius.
      In the SI unit system the symbol is ï¿½C. Electric charge is measured in coulomb that has the unit symbol C. To distinguish degree Celsius form coulomb the symbol used in the UML is degC. Reason for not using ï¿½C is the special character ï¿½ is difficult to manage in software."""@en ;
  rdfs:isDefinedBy :Package_CIMEnumerations ;
  uml:id "EAID_2BA135D2_0950_48d2_976B_A142C4FB4BD5" .

cim:UnitSymbol.ft3 a cim:UnitSymbol ;
  rdfs:label "ft3" ;
  rdfs:comment "Volume, cubic foot."@en ;
  rdfs:isDefinedBy :Package_CIMEnumerations ;
  uml:id "EAID_EE3DE7DA_7747_4df4_AA96_CB826C159A37" .

cim:UnitSymbol.gPerg a cim:UnitSymbol ;
  rdfs:label "gPerg" ;
  rdfs:comment "Concentration, The ratio of the mass of a solute divided by the mass of  the solution. Note: Users may need use a prefix such a ï¿½ï¿½ï¿½ to express a quantity such as ï¿½ï¿½g/gï¿½."@en ;
  rdfs:isDefinedBy :Package_CIMEnumerations ;
  uml:id "EAID_4FE2C6F4_252B_478b_81B6_B8A37C2040EA" .

cim:UnitSymbol.gal a cim:UnitSymbol ;
  rdfs:label "gal" ;
  rdfs:comment "Volume, US gallon (1 gal = 231 in3 = 128 fl ounce)."@en ;
  rdfs:isDefinedBy :Package_CIMEnumerations ;
  uml:id "EAID_075573F5_3B3E_413a_A3EE_6EEAD392ACF2" .

cim:UnitSymbol.h a cim:UnitSymbol ;
  rdfs:label "h" ;
  rdfs:comment "Time, hour = 60 min = 3600 s."@en ;
  rdfs:isDefinedBy :Package_CIMEnumerations ;
  uml:id "EAID_2FF7FF26_CE3D_43a3_99E4_7188416EC342" .

cim:UnitSymbol.ha a cim:UnitSymbol ;
  rdfs:label "ha" ;
  rdfs:comment "Area, hectare."@en ;
  rdfs:isDefinedBy :Package_CIMEnumerations ;
  uml:id "EAID_5DAD9F50_364E_4ff1_BC2C_B761442B63C0" .

cim:UnitSymbol.kat a cim:UnitSymbol ;
  rdfs:label "kat" ;
  rdfs:comment "Catalytic activity, katal = mol / s."@en ;
  rdfs:isDefinedBy :Package_CIMEnumerations ;
  uml:id "EAID_834E4B66_2AB3_4795_BDDA_F41BBA345492" .

cim:UnitSymbol.katPerm3 a cim:UnitSymbol ;
  rdfs:label "katPerm3" ;
  rdfs:comment "catalytic activity concentration, katal per cubic metre."@en ;
  rdfs:isDefinedBy :Package_CIMEnumerations ;
  uml:id "EAID_6221E81C_4094_4544_A256_101BFF4D1FC5" .

cim:UnitSymbol.kg a cim:UnitSymbol ;
  rdfs:label "kg" ;
  rdfs:comment "Mass in kilogram.  Note: multiplier ï¿½kï¿½ is included in this unit symbol for compatibility with IEC 61850-7-3."@en ;
  rdfs:isDefinedBy :Package_CIMEnumerations ;
  uml:id "EAID_DFBF6B76_BA8D_48f1_B895_3C1F69D191BC" .

cim:UnitSymbol.kgPerJ a cim:UnitSymbol ;
  rdfs:label "kgPerJ" ;
  rdfs:comment "Weigh per energy in kilogram/joule (kg/J). Note: multiplier ï¿½kï¿½ is included in this unit symbol for compatibility with IEC 61850-7-3."@en ;
  rdfs:isDefinedBy :Package_CIMEnumerations ;
  uml:id "EAID_CC8F1FA5_7B24_44c6_A882_50C0713C04A5" .

cim:UnitSymbol.kgPerm3 a cim:UnitSymbol ;
  rdfs:label "kgPerm3" ;
  rdfs:comment "Density in kilogram/cubic metre (kg/mï¿½). Note: multiplier ï¿½kï¿½ is included in this unit symbol for compatibility with IEC 61850-7-3."@en ;
  rdfs:isDefinedBy :Package_CIMEnumerations ;
  uml:id "EAID_501BEC8C_B847_44aa_BD7B_E606CCDBA737" .

cim:UnitSymbol.kgm a cim:UnitSymbol ;
  rdfs:label "kgm" ;
  rdfs:comment "Moment of mass in kilogram metre (kgï¿½m) (first moment of mass). Note: multiplier ï¿½kï¿½ is included in this unit symbol for compatibility with IEC 61850-7-3."@en ;
  rdfs:isDefinedBy :Package_CIMEnumerations ;
  uml:id "EAID_1DE9FA6B_0179_4e12_B5C4_6ABEB1FC4002" .

cim:UnitSymbol.kgm2 a cim:UnitSymbol ;
  rdfs:label "kgm2" ;
  rdfs:comment "Moment of mass in kilogram square metre (kgï¿½mï¿½) (Second moment of mass, commonly called the moment of inertia). Note: multiplier ï¿½kï¿½ is included in this unit symbol for compatibility with IEC 61850-7-3."@en ;
  rdfs:isDefinedBy :Package_CIMEnumerations ;
  uml:id "EAID_61A641E6_AACB_4084_8033_1F0424D09B3A" .

cim:UnitSymbol.kn a cim:UnitSymbol ;
  rdfs:label "kn" ;
  rdfs:comment "Speed, knot (1 kn = 1852/3600) m/s."@en ;
  rdfs:isDefinedBy :Package_CIMEnumerations ;
  uml:id "EAID_F100EA66_B1BA_4d19_B04F_94A815273DA8" .

cim:UnitSymbol.l a cim:UnitSymbol ;
  rdfs:label "l" ;
  rdfs:comment "Volume, litre = dm3 = m3/1000."@en ;
  rdfs:isDefinedBy :Package_CIMEnumerations ;
  uml:id "EAID_D946A4B2_75F4_456d_8A7B_60D75D8C8C54" .

cim:UnitSymbol.lPerh a cim:UnitSymbol ;
  rdfs:label "lPerh" ;
  rdfs:comment "Volumetric flow rate, litre per hour."@en ;
  rdfs:isDefinedBy :Package_CIMEnumerations ;
  uml:id "EAID_A2D6FCDF_C6C0_4b29_A162_3851CFD8CDFA" .

cim:UnitSymbol.lPerl a cim:UnitSymbol ;
  rdfs:label "lPerl" ;
  rdfs:comment "Concentration, The ratio of the volume of a solute divided by the volume of  the solution. Note: Users may need use a prefix such a ï¿½ï¿½ï¿½ to express a quantity such as ï¿½ï¿½L/Lï¿½."@en ;
  rdfs:isDefinedBy :Package_CIMEnumerations ;
  uml:id "EAID_1734D386_C2FA_4d27_B33B_F56A5B13F07D" .

cim:UnitSymbol.lPers a cim:UnitSymbol ;
  rdfs:label "lPers" ;
  rdfs:comment "Volumetric flow rate in litre per second."@en ;
  rdfs:isDefinedBy :Package_CIMEnumerations ;
  uml:id "EAID_EFE6BF1C_3882_4194_84CF_DB5A333DC816" .

cim:UnitSymbol.lm a cim:UnitSymbol ;
  rdfs:label "lm" ;
  rdfs:comment "Luminous flux in lumen (cdï¿½sr)."@en ;
  rdfs:isDefinedBy :Package_CIMEnumerations ;
  uml:id "EAID_CA24CD8D_1AAB_4e25_A5F3_9CE4FF76D150" .

cim:UnitSymbol.lx a cim:UnitSymbol ;
  rdfs:label "lx" ;
  rdfs:comment "Illuminance in lux (lm/mï¿½)."@en ;
  rdfs:isDefinedBy :Package_CIMEnumerations ;
  uml:id "EAID_66FD58AD_46BC_40cc_87F2_60012016945E" .

cim:UnitSymbol.m a cim:UnitSymbol ;
  rdfs:label "m" ;
  rdfs:comment "Length in meter."@en ;
  rdfs:isDefinedBy :Package_CIMEnumerations ;
  uml:id "EAID_E115BEB5_4F2D_4394_AF62_EB222FCD4431" .

cim:UnitSymbol.m2 a cim:UnitSymbol ;
  rdfs:label "m2" ;
  rdfs:comment "Area in square metre (mï¿½)."@en ;
  rdfs:isDefinedBy :Package_CIMEnumerations ;
  uml:id "EAID_244449A7_27DD_43b1_8A51_C79EFCA98953" .

cim:UnitSymbol.m2Pers a cim:UnitSymbol ;
  rdfs:label "m2Pers" ;
  rdfs:comment "Viscosity in metre square / second (mï¿½/s)."@en ;
  rdfs:isDefinedBy :Package_CIMEnumerations ;
  uml:id "EAID_DF3DC5F4_EA0C_4ceb_A28F_32BAD9DFFACD" .

cim:UnitSymbol.m3 a cim:UnitSymbol ;
  rdfs:label "m3" ;
  rdfs:comment "Volume in cubic metre (mï¿½)."@en ;
  rdfs:isDefinedBy :Package_CIMEnumerations ;
  uml:id "EAID_51129F02_2AD7_4cf4_A1B2_0429467866FA" .

cim:UnitSymbol.m3Compensated a cim:UnitSymbol ;
  rdfs:label "m3Compensated" ;
  rdfs:comment "Volume, cubic metre, with the value compensated for weather effects."@en ;
  rdfs:isDefinedBy :Package_CIMEnumerations ;
  uml:id "EAID_33690AF4_D81B_47f5_89FE_462996022C7E" .

cim:UnitSymbol.m3Perh a cim:UnitSymbol ;
  rdfs:label "m3Perh" ;
  rdfs:comment "Volumetric flow rate, cubic metre per hour."@en ;
  rdfs:isDefinedBy :Package_CIMEnumerations ;
  uml:id "EAID_96A81015_4806_4f34_8569_AA1432D6B2C8" .

cim:UnitSymbol.m3Perkg a cim:UnitSymbol ;
  rdfs:label "m3Perkg" ;
  rdfs:comment "Specific volume, cubic metre per kilogram, v."@en ;
  rdfs:isDefinedBy :Package_CIMEnumerations ;
  uml:id "EAID_A8364DE1_5E2D_490e_B99A_0D455165E39C" .

cim:UnitSymbol.m3Pers a cim:UnitSymbol ;
  rdfs:label "m3Pers" ;
  rdfs:comment "Volumetric flow rate in cubic metres per second (mï¿½/s)."@en ;
  rdfs:isDefinedBy :Package_CIMEnumerations ;
  uml:id "EAID_71D34D30_EE1F_491c_A3CA_1537AFCAE549" .

cim:UnitSymbol.m3Uncompensated a cim:UnitSymbol ;
  rdfs:label "m3Uncompensated" ;
  rdfs:comment "Volume, cubic metre, with the value uncompensated for weather effects."@en ;
  rdfs:isDefinedBy :Package_CIMEnumerations ;
  uml:id "EAID_6EF4A0F2_BA42_4486_B9A9_377C712B992E" .

cim:UnitSymbol.mPerm3 a cim:UnitSymbol ;
  rdfs:label "mPerm3" ;
  rdfs:comment "Fuel efficiency in metre per cubic metre (m/mï¿½)."@en ;
  rdfs:isDefinedBy :Package_CIMEnumerations ;
  uml:id "EAID_23C866AE_1454_4cac_B175_5BB2B115F859" .

cim:UnitSymbol.mPers a cim:UnitSymbol ;
  rdfs:label "mPers" ;
  rdfs:comment "Velocity in metre per second (m/s)."@en ;
  rdfs:isDefinedBy :Package_CIMEnumerations ;
  uml:id "EAID_14B945E9_F748_46eb_8316_7E7554218281" .

cim:UnitSymbol.mPers2 a cim:UnitSymbol ;
  rdfs:label "mPers2" ;
  rdfs:comment "Acceleration in metre per second squared (m/sï¿½)."@en ;
  rdfs:isDefinedBy :Package_CIMEnumerations ;
  uml:id "EAID_EA7DFD97_B06D_49dc_8726_EF0AF90505EE" .

cim:UnitSymbol.min a cim:UnitSymbol ;
  rdfs:label "min" ;
  rdfs:comment "Time, minute  = 60 s."@en ;
  rdfs:isDefinedBy :Package_CIMEnumerations ;
  uml:id "EAID_3711F440_EF3C_4c2d_8E90_CFC579ED94D1" .

cim:UnitSymbol.mmHg a cim:UnitSymbol ;
  rdfs:label "mmHg" ;
  rdfs:comment "Pressure, millimeter of mercury (1 mmHg is approximately 133.3 Pa)."@en ;
  rdfs:isDefinedBy :Package_CIMEnumerations ;
  uml:id "EAID_2AF0F2E6_FE07_4d0f_96C0_53B160516548" .

cim:UnitSymbol.mol a cim:UnitSymbol ;
  rdfs:label "mol" ;
  rdfs:comment "Amount of substance in mole."@en ;
  rdfs:isDefinedBy :Package_CIMEnumerations ;
  uml:id "EAID_60EE99CE_44B4_4eea_A380_C57B5A599751" .

cim:UnitSymbol.molPerkg a cim:UnitSymbol ;
  rdfs:label "molPerkg" ;
  rdfs:comment "Concentration, Molality, the amount of solute in moles and the amount of solvent in kilograms."@en ;
  rdfs:isDefinedBy :Package_CIMEnumerations ;
  uml:id "EAID_6393AB83_C6B3_4a9f_9014_4922A983270E" .

cim:UnitSymbol.molPerm3 a cim:UnitSymbol ;
  rdfs:label "molPerm3" ;
  rdfs:comment "Concentration, The amount of substance concentration, (c), the amount of solvent in moles divided by the volume of solution in mï¿½."@en ;
  rdfs:isDefinedBy :Package_CIMEnumerations ;
  uml:id "EAID_75B287C7_9AE3_4d28_8ECD_68CF7049BE6E" .

cim:UnitSymbol.molPermol a cim:UnitSymbol ;
  rdfs:label "molPermol" ;
  rdfs:comment "Concentration, Molar fraction (?), the ratio of the molar amount of a solute divided by the molar amount of the solution."@en ;
  rdfs:isDefinedBy :Package_CIMEnumerations ;
  uml:id "EAID_2E332E4E_01A2_44b3_805D_026A1C392DD7" .

cim:UnitSymbol.none a cim:UnitSymbol ;
  rdfs:label "none" ;
  rdfs:comment "Dimension less quantity, e.g. count, per unit, etc."@en ;
  rdfs:isDefinedBy :Package_CIMEnumerations ;
  uml:id "EAID_D2CE6FE3_01D7_4dd1_B8F7_FF90BE636625" .

cim:UnitSymbol.ohm a cim:UnitSymbol ;
  rdfs:label "ohm" ;
  rdfs:comment "Electric resistance in ohm (V/A)."@en ;
  rdfs:isDefinedBy :Package_CIMEnumerations ;
  uml:id "EAID_0D7094F7_0879_4d34_B08B_DEBC8C333F47" .

cim:UnitSymbol.ohmPerm a cim:UnitSymbol ;
  rdfs:label "ohmPerm" ;
  rdfs:comment "Electric resistance per length in ohm per metre ((V/A)/m)."@en ;
  rdfs:isDefinedBy :Package_CIMEnumerations ;
  uml:id "EAID_7FF254A7_BED8_4c65_995C_C60F5F99FF54" .

cim:UnitSymbol.ohmm a cim:UnitSymbol ;
  rdfs:label "ohmm" ;
  rdfs:comment "resistivity, Ohm metre, (rho)."@en ;
  rdfs:isDefinedBy :Package_CIMEnumerations ;
  uml:id "EAID_AC95BDC8_E2FA_47bc_A37A_04D7248D068B" .

cim:UnitSymbol.onePerHz a cim:UnitSymbol ;
  rdfs:label "onePerHz" ;
  rdfs:comment "Reciprocal of frequency (1/Hz)."@en ;
  rdfs:isDefinedBy :Package_CIMEnumerations ;
  uml:id "EAID_E416F8A6_355A_4667_A64E_E8BA5416F12A" .

cim:UnitSymbol.onePerm a cim:UnitSymbol ;
  rdfs:label "onePerm" ;
  rdfs:comment "Wavenumber, reciprocal metre,  (1/m)."@en ;
  rdfs:isDefinedBy :Package_CIMEnumerations ;
  uml:id "EAID_30EFB7ED_268D_4077_87DC_FAD3D4D1D20E" .

cim:UnitSymbol.ppm a cim:UnitSymbol ;
  rdfs:label "ppm" ;
  rdfs:comment "Concentration in parts per million."@en ;
  rdfs:isDefinedBy :Package_CIMEnumerations ;
  uml:id "EAID_BE0ED943_A3E0_477d_947B_05F076A2A5FD" .

cim:UnitSymbol.rad a cim:UnitSymbol ;
  rdfs:label "rad" ;
  rdfs:comment "Plane angle in radian (m/m)."@en ;
  rdfs:isDefinedBy :Package_CIMEnumerations ;
  uml:id "EAID_E6692373_B332_4cd8_AE2D_D17186894BB3" .

cim:UnitSymbol.radPers a cim:UnitSymbol ;
  rdfs:label "radPers" ;
  rdfs:comment "Angular velocity in radians per second (rad/s)."@en ;
  rdfs:isDefinedBy :Package_CIMEnumerations ;
  uml:id "EAID_A44B7E88_AD3F_4765_894A_8C4E32EAC533" .

cim:UnitSymbol.radPers2 a cim:UnitSymbol ;
  rdfs:label "radPers2" ;
  rdfs:comment "Angular acceleration, radian per second squared."@en ;
  rdfs:isDefinedBy :Package_CIMEnumerations ;
  uml:id "EAID_79216E4F_F72F_44ef_9AAE_4BBE9441712A" .

cim:UnitSymbol.rev a cim:UnitSymbol ;
  rdfs:label "rev" ;
  rdfs:comment "Amount of rotation, Revolutions."@en ;
  rdfs:isDefinedBy :Package_CIMEnumerations ;
  uml:id "EAID_6F1AA7AC_7267_46c1_9A0E_86B9095B2B6B" .

cim:UnitSymbol.rotPers a cim:UnitSymbol ;
  rdfs:label "rotPers" ;
  rdfs:comment "Rotations per second (1/s). See also Hz (1/s)."@en ;
  rdfs:isDefinedBy :Package_CIMEnumerations ;
  uml:id "EAID_ECAF4A79_071B_4634_B2B2_DF2CB571C6DB" .

cim:UnitSymbol.s a cim:UnitSymbol ;
  rdfs:label "s" ;
  rdfs:comment "Time in seconds."@en ;
  rdfs:isDefinedBy :Package_CIMEnumerations ;
  uml:id "EAID_6114A519_3046_45a6_8A51_0DCFB465BCE6" .

cim:UnitSymbol.sPers a cim:UnitSymbol ;
  rdfs:label "sPers" ;
  rdfs:comment "Time, Ratio of time Note: Users may need to supply a prefix such as ï¿½ï¿½ï¿½ to show rates such as ï¿½ï¿½s/sï¿½"@en ;
  rdfs:isDefinedBy :Package_CIMEnumerations ;
  uml:id "EAID_EC6B9D0A_9C93_4a3f_BF4C_28E0D4F71EF5" .

cim:UnitSymbol.sr a cim:UnitSymbol ;
  rdfs:label "sr" ;
  rdfs:comment "Solid angle in steradian (m2/m2)."@en ;
  rdfs:isDefinedBy :Package_CIMEnumerations ;
  uml:id "EAID_08E268BA_FF87_444c_86E8_73A7EC4FF8D2" .

cim:UnitSymbol.therm a cim:UnitSymbol ;
  rdfs:label "therm" ;
  rdfs:comment "Energy, Therm."@en ;
  rdfs:isDefinedBy :Package_CIMEnumerations ;
  uml:id "EAID_4CA0BAFD_8B17_41ec_9753_0942B31959E8" .

cim:UnitSymbol.tonne a cim:UnitSymbol ;
  rdfs:label "tonne" ;
  rdfs:comment "mass, ï¿½tonneï¿½ or ï¿½metric  tonï¿½ (1000 kg = 1 Mg)."@en ;
  rdfs:isDefinedBy :Package_CIMEnumerations ;
  uml:id "EAID_A053EE28_60BE_4459_89CF_0EF5CB8FCE30" .

cim:Voltage a rdfs:Datatype ;
  rdfs:label "Voltage" ;
  rdfs:comment "Electrical voltage."@en ;
  owl:equivalentClass xsd:float ;
  rdfs:isDefinedBy :Package_CIMDataTypes ;
  uml:hasMultiplier "k" ;
  uml:hasStereotype uml:cimdatatype ;
  uml:hasUnits "V" ;
  uml:id "EAID_21C26D0F_BD78_444c_A025_61515F1D67B7" .

cim:VoltagePerReactivePower a rdfs:Datatype ;
  rdfs:label "VoltagePerReactivePower" ;
  rdfs:comment "Voltage variation with reactive power"@en ;
  owl:equivalentClass xsd:float ;
  rdfs:isDefinedBy :Package_CIMDataTypes ;
  uml:hasStereotype uml:cimdatatype ;
  uml:hasUnits "VPerVAr" ;
  uml:id "EAID_1DF64161_6CDF_4681_A40A_FAE80E1B8AD9" .

cim:WindGenUnitKind.offshore a cim:WindGenUnitKind ;
  rdfs:label "offshore" ;
  rdfs:comment "The wind generating unit is located offshore."@en ;
  rdfs:isDefinedBy :Package_CIMEnumerations ;
  uml:id "EAID_6AA2C69E_87FC_4e2e_B774_DBA24BA423A8" .

cim:WindGenUnitKind.onshore a cim:WindGenUnitKind ;
  rdfs:label "onshore" ;
  rdfs:comment "The wind generating unit is located onshore."@en ;
  rdfs:isDefinedBy :Package_CIMEnumerations ;
  uml:id "EAID_72FE0A3C_10D8_46e1_9512_E12C33892EE6" .

cim:WindingConnection.A a cim:WindingConnection ;
  rdfs:label "A" ;
  rdfs:comment "Autotransformer common winding"@en ;
  rdfs:isDefinedBy :Package_CIMEnumerations ;
  uml:id "EAID_D7E730D7_F1E1_4b1f_A052_C985EB91EFBC" .

cim:WindingConnection.D a cim:WindingConnection ;
  rdfs:label "D" ;
  rdfs:comment "Delta"@en ;
  rdfs:isDefinedBy :Package_CIMEnumerations ;
  uml:id "EAID_A4A9CBDC_3182_48b4_9709_2458B1B84066" .

cim:WindingConnection.I a cim:WindingConnection ;
  rdfs:label "I" ;
  rdfs:comment "Independent winding, for single-phase connections"@en ;
  rdfs:isDefinedBy :Package_CIMEnumerations ;
  uml:id "EAID_42EC06DE_A1F1_414b_85A6_55B3A11A14EC" .

cim:WindingConnection.Y a cim:WindingConnection ;
  rdfs:label "Y" ;
  rdfs:comment "Wye"@en ;
  rdfs:isDefinedBy :Package_CIMEnumerations ;
  uml:id "EAID_8DE87FC8_1289_49fa_9738_92F17BE0E78A" .

cim:WindingConnection.Yn a cim:WindingConnection ;
  rdfs:label "Yn" ;
  rdfs:comment "Wye, with neutral brought out for grounding."@en ;
  rdfs:isDefinedBy :Package_CIMEnumerations ;
  uml:id "EAID_662B6476_DA64_4379_93BE_06B3DAC31C2B" .

cim:WindingConnection.Z a cim:WindingConnection ;
  rdfs:label "Z" ;
  rdfs:comment "ZigZag"@en ;
  rdfs:isDefinedBy :Package_CIMEnumerations ;
  uml:id "EAID_4C2D41A1_4F47_4561_9CB1_0F8C4C2A35B6" .

cim:WindingConnection.Zn a cim:WindingConnection ;
  rdfs:label "Zn" ;
  rdfs:comment "ZigZag, with neutral brought out for grounding."@en ;
  rdfs:isDefinedBy :Package_CIMEnumerations ;
  uml:id "EAID_CBED0332_D6A9_465c_9F81_3BADD87D81BD" .

cim:WireInsulationKind.asbestosAndVarnishedCambric a cim:WireInsulationKind ;
  rdfs:label "asbestosAndVarnishedCambric" ;
  rdfs:isDefinedBy :Package_CIMEnumerations ;
  uml:id "EAID_E2D397FE_53C0_4362_96E5_163900C3C661" .

cim:WireInsulationKind.beltedPilc a cim:WireInsulationKind ;
  rdfs:label "beltedPilc" ;
  rdfs:isDefinedBy :Package_CIMEnumerations ;
  uml:id "EAID_D234E706_517B_4452_8C7A_209068C4AB5B" .

cim:WireInsulationKind.butyl a cim:WireInsulationKind ;
  rdfs:label "butyl" ;
  rdfs:isDefinedBy :Package_CIMEnumerations ;
  uml:id "EAID_E12301A9_8968_4235_AD10_01C5D076D9C6" .

cim:WireInsulationKind.crosslinkedPolyethylene a cim:WireInsulationKind ;
  rdfs:label "crosslinkedPolyethylene" ;
  rdfs:isDefinedBy :Package_CIMEnumerations ;
  uml:id "EAID_F8F5FADE_221E_47db_9CCF_BF45B3961468" .

cim:WireInsulationKind.ethylenePropyleneRubber a cim:WireInsulationKind ;
  rdfs:label "ethylenePropyleneRubber" ;
  rdfs:isDefinedBy :Package_CIMEnumerations ;
  uml:id "EAID_FAB16BFF_E26A_4ac2_A4EF_5D87ED0D6D8A" .

cim:WireInsulationKind.highMolecularWeightPolyethylene a cim:WireInsulationKind ;
  rdfs:label "highMolecularWeightPolyethylene" ;
  rdfs:isDefinedBy :Package_CIMEnumerations ;
  uml:id "EAID_2A5AC730_5EAA_4dbe_89F7_6926C40CE3AA" .

cim:WireInsulationKind.highPressureFluidFilled a cim:WireInsulationKind ;
  rdfs:label "highPressureFluidFilled" ;
  rdfs:isDefinedBy :Package_CIMEnumerations ;
  uml:id "EAID_31782C28_3342_4e7e_9C16_C767EA054D93" .

cim:WireInsulationKind.lowCapacitanceRubber a cim:WireInsulationKind ;
  rdfs:label "lowCapacitanceRubber" ;
  rdfs:isDefinedBy :Package_CIMEnumerations ;
  uml:id "EAID_961CFE6D_312A_4c78_8787_DD6FF530792B" .

cim:WireInsulationKind.oilPaper a cim:WireInsulationKind ;
  rdfs:label "oilPaper" ;
  rdfs:isDefinedBy :Package_CIMEnumerations ;
  uml:id "EAID_9AE08072_2A33_43af_BE3F_064F8C0B6D16" .

cim:WireInsulationKind.other a cim:WireInsulationKind ;
  rdfs:label "other" ;
  rdfs:isDefinedBy :Package_CIMEnumerations ;
  uml:id "EAID_D633B342_9CA4_4a3c_9018_925E2D8FF1C2" .

cim:WireInsulationKind.ozoneResistantRubber a cim:WireInsulationKind ;
  rdfs:label "ozoneResistantRubber" ;
  rdfs:isDefinedBy :Package_CIMEnumerations ;
  uml:id "EAID_2EB63137_31CC_4de7_836B_7CDF6703A9C7" .

cim:WireInsulationKind.rubber a cim:WireInsulationKind ;
  rdfs:label "rubber" ;
  rdfs:isDefinedBy :Package_CIMEnumerations ;
  uml:id "EAID_2EBA837D_F669_4613_BAEC_5E4EFE0C4E56" .

cim:WireInsulationKind.siliconRubber a cim:WireInsulationKind ;
  rdfs:label "siliconRubber" ;
  rdfs:isDefinedBy :Package_CIMEnumerations ;
  uml:id "EAID_0FEAA298_EF99_4777_998D_84196014FD5B" .

cim:WireInsulationKind.treeResistantHighMolecularWeightPolyethylene a cim:WireInsulationKind ;
  rdfs:label "treeResistantHighMolecularWeightPolyethylene" ;
  rdfs:isDefinedBy :Package_CIMEnumerations ;
  uml:id "EAID_45F5CFFD_B559_451e_8ED1_31ADA97E7135" .

cim:WireInsulationKind.treeRetardantCrosslinkedPolyethylene a cim:WireInsulationKind ;
  rdfs:label "treeRetardantCrosslinkedPolyethylene" ;
  rdfs:isDefinedBy :Package_CIMEnumerations ;
  uml:id "EAID_EDAD013B_EA92_4565_A0D3_5637926526EB" .

cim:WireInsulationKind.unbeltedPilc a cim:WireInsulationKind ;
  rdfs:label "unbeltedPilc" ;
  rdfs:isDefinedBy :Package_CIMEnumerations ;
  uml:id "EAID_B452862B_3CC6_4a8c_8D29_87A2CB7E52AB" .

cim:WireInsulationKind.varnishedCambricCloth a cim:WireInsulationKind ;
  rdfs:label "varnishedCambricCloth" ;
  rdfs:isDefinedBy :Package_CIMEnumerations ;
  uml:id "EAID_33D24022_A36E_4d80_97FA_6A87221C94A2" .

cim:WireInsulationKind.varnishedDacronGlass a cim:WireInsulationKind ;
  rdfs:label "varnishedDacronGlass" ;
  rdfs:isDefinedBy :Package_CIMEnumerations ;
  uml:id "EAID_47E2D409_4615_446d_B62A_1AE66872A80D" .

cim:WireMaterialKind.aaac a cim:WireMaterialKind ;
  rdfs:label "aaac" ;
  rdfs:comment "Aluminum-alloy conductor steel reinforced."@en ;
  rdfs:isDefinedBy :Package_CIMEnumerations ;
  uml:id "EAID_268ED1E9_EC67_4f18_A7DC_0955C9A0AD4D" .

cim:WireMaterialKind.acsr a cim:WireMaterialKind ;
  rdfs:label "acsr" ;
  rdfs:comment "Aluminum conductor steel reinforced."@en ;
  rdfs:isDefinedBy :Package_CIMEnumerations ;
  uml:id "EAID_0FC14A5C_8C14_4a1c_8F99_767018668A79" .

cim:WireMaterialKind.aluminum a cim:WireMaterialKind ;
  rdfs:label "aluminum" ;
  rdfs:isDefinedBy :Package_CIMEnumerations ;
  uml:id "EAID_4B18AEEA_0183_47c7_A880_8130E7DCEFD3" .

cim:WireMaterialKind.aluminumAlloy a cim:WireMaterialKind ;
  rdfs:label "aluminumAlloy" ;
  rdfs:isDefinedBy :Package_CIMEnumerations ;
  uml:id "EAID_0BBB476F_EF99_49fc_8D0B_253412E863A8" .

cim:WireMaterialKind.aluminumAlloySteel a cim:WireMaterialKind ;
  rdfs:label "aluminumAlloySteel" ;
  rdfs:isDefinedBy :Package_CIMEnumerations ;
  uml:id "EAID_E856F4E7_A25B_46c1_A00D_8C9E3E20C11D" .

cim:WireMaterialKind.aluminumSteel a cim:WireMaterialKind ;
  rdfs:label "aluminumSteel" ;
  rdfs:isDefinedBy :Package_CIMEnumerations ;
  uml:id "EAID_1026B016_6E05_4dc6_9C09_4DDB5109DBDA" .

cim:WireMaterialKind.copper a cim:WireMaterialKind ;
  rdfs:label "copper" ;
  rdfs:isDefinedBy :Package_CIMEnumerations ;
  uml:id "EAID_C437F22C_25F5_441e_91FA_1DF52B52982A" .

cim:WireMaterialKind.other a cim:WireMaterialKind ;
  rdfs:label "other" ;
  rdfs:isDefinedBy :Package_CIMEnumerations ;
  uml:id "EAID_D11DA662_4961_4a31_A0D7_4F15BB1653EC" .

cim:WireMaterialKind.steel a cim:WireMaterialKind ;
  rdfs:label "steel" ;
  rdfs:isDefinedBy :Package_CIMEnumerations ;
  uml:id "EAID_B41B166A_4EC4_4b8b_B3E5_020CB40F2C5B" .

cim:WireUsageKind.distribution a cim:WireUsageKind ;
  rdfs:label "distribution" ;
  rdfs:isDefinedBy :Package_CIMEnumerations ;
  uml:id "EAID_B3883D2E_FE70_404f_A707_BC1F61D33C69" .

cim:WireUsageKind.other a cim:WireUsageKind ;
  rdfs:label "other" ;
  rdfs:isDefinedBy :Package_CIMEnumerations ;
  uml:id "EAID_6C7040CB_2E2C_495d_8A01_449C074F2543" .

cim:WireUsageKind.secondary a cim:WireUsageKind ;
  rdfs:label "secondary" ;
  rdfs:isDefinedBy :Package_CIMEnumerations ;
  uml:id "EAID_7E55E71F_42CA_4aa4_9EC2_82A7F9648E86" .

cim:WireUsageKind.transmission a cim:WireUsageKind ;
  rdfs:label "transmission" ;
  rdfs:isDefinedBy :Package_CIMEnumerations ;
  uml:id "EAID_BF36BBDB_FC1D_4924_86A9_D9F754285E55" .

md:URI a rdfs:Datatype ;
  rdfs:label "URI" ;
  rdfs:comment "URI is a string following the rules defined by the W3C/IETF URI Planning Interest Group in a set of RFCs of which one is RFC 3305."@en ;
  rdfs:isDefinedBy :Package_ModelDescription ;
  uml:hasStereotype uml:primitive ;
  uml:id "EAID_FD27B00A_FB5C_4944_9ECA_58BD201E9B7F" .

uml:aggregateOf a uml:Stereotype ;
  rdfs:label "Aggregate Of" .

uml:attribute a uml:Stereotype ;
  rdfs:label "Attribute" .

uml:base a uml:Stereotype ;
  rdfs:label "Base" .

uml:byreference a uml:Stereotype ;
  rdfs:label "By Reference" .

uml:cdpsm a uml:Stereotype ;
  rdfs:label "cdpsm" ;
  uml:id "EAID_C845457D_5C10_429c_BB35_B765639087B0" .

uml:cimdatatype a uml:Stereotype ;
  rdfs:label "CIMDatatype" ;
  uml:id "EAID_DBA1FFD8_1484_4fc2_B66A_E6348B3A6A89" .

uml:compositeOf a uml:Stereotype ;
  rdfs:label "Composite Of" .

uml:compound a uml:Stereotype ;
  rdfs:label "Compound", "Compound Datatype" ;
  uml:id "EAID_1FBEF2D1_91AA_467d_AE9C_F353EB44AB64" .

uml:concrete a uml:Stereotype ;
  rdfs:label "Concrete" .

uml:contextualmodel a uml:Stereotype ;
  rdfs:label "ContextualModel" ;
  uml:id "EAID_565DE0C5_3550_4288_948B_FC5DBF209C05", "EAID_8DCF8F70_C3E5_4cef_84F9_B992F351B950" .

uml:datatype a uml:Stereotype ;
  rdfs:label "Datatype" .

uml:deprecated a uml:Stereotype ;
  rdfs:label "deprecated" ;
  uml:id "EAID_04E85A9B_E8D0_4f2c_AD38_6B560201A24B" .

uml:entsoe a uml:Stereotype ;
  rdfs:label "Entsoe" ;
  uml:id "EAID_89EB1BFD_4630_4704_AC74_B6FE25F8E434", "EAID_C6232DC4_C7C7_4c11_B75A_30616E266B5F" .

uml:enum a uml:Stereotype ;
  rdfs:label "enum" ;
  uml:id "EAID_2DB4C97D_A73C_4e3d_945B_DC11C242BB0B", "EAID_DFA7F18C_C4F9_4c58_815D_FA0C06B4C911" .

uml:enumeration a uml:Stereotype ;
  rdfs:label "Enumeration", "enumeration" ;
  uml:id "XTRA_stereotype_enumeration" .

uml:extendedby a uml:Stereotype ;
  rdfs:label "Extended By" .

uml:extension a uml:Stereotype ;
  rdfs:label "Extension Class", "extension" ;
  uml:id "EAID_7B6F9213_3CDC_4eba_ACE8_8122449C906A", "EAID_815CAB4A_AE9F_4c03_A0B2_D8C611380488", "EAID_D8E80C48_F67E_44ea_B1BD_33DD155D9CB1" .

uml:ofAggregate a uml:Stereotype ;
  rdfs:label "Of Aggregate" .

uml:ofComposite a uml:Stereotype ;
  rdfs:label "Of Composite" .

uml:preserve a uml:Stereotype ;
  rdfs:label "Preserve" .

uml:primitive a uml:Stereotype ;
  rdfs:label "Primitive" ;
  uml:id "EAID_2CBBE568_189E_4185_ABB5_8CA72ACAB81A", "EAID_D264CE2A_6D6E_49a4_A842_EF38A16736E4" .

uml:union a uml:Stereotype ;
  rdfs:label "Union" .

uml:xmlattribute a uml:Stereotype ;
  rdfs:label "XML Attribute" .

uml:xmlelement a uml:Stereotype ;
  rdfs:label "XML Element" .

xsd:date rdfs:label "Date" ;
  uml:id "eaxmiid3" .

xsd:dateTime rdfs:label "DateTime" ;
  uml:id "eaxmiid1" .

xsd:integer rdfs:label "Integer" ;
  uml:id "eaxmiid4" .

xsd:string rdfs:label "String" ;
  uml:id "eaxmiid0" .


